BoogieLang/Ast_Cfg_Transformation.thy
@@ -82,6 +82,12 @@ qed
 lemma strictly_smaller_helper2: "j'' < j' \<Longrightarrow> j = Suc j' \<Longrightarrow> j'' < j"
   by simp
 
+lemma strictly_smaller_helper3: "j'' < j' \<Longrightarrow> j''' < j'' \<Longrightarrow> j = Suc j' \<Longrightarrow> j''' < j"
+  by simp
+
+lemma strictly_smaller_helper4: "j' = Suc (Suc j'') \<Longrightarrow> k < j'' \<Longrightarrow> j = Suc j' \<Longrightarrow> k < j"
+  by simp
+
 lemma steps_trans_helper:
   assumes "A,M,\<Lambda>,\<Gamma>,\<Omega>,T \<turnstile>(bb0, cont0, Normal ns1'') -n\<longrightarrow>^j' (reached_bb, reached_cont, reached_state)"
   shows "rtranclp (red_bigblock A M \<Lambda> \<Gamma> \<Omega> T) (bb0, cont0, Normal ns1'') (reached_bb, reached_cont, reached_state)"
@@ -90,14 +96,41 @@ proof -
   from assms(1) show ?thesis by (simp add: relpowp_imp_rtranclp)
 qed
 
+lemma seq_skip:
+  assumes "A,M,\<Lambda>,\<Gamma>,\<Omega>,T \<turnstile>(bb0, (KSeq bb_next cont0), Normal ns3) -n\<longrightarrow>^l (reached_bb, reached_cont, reached_state)"
+      and "bb0 = BigBlock None [] None None"
+  shows "(valid_configuration A \<Lambda> \<Gamma> \<Omega> posts reached_bb reached_cont reached_state) \<or> 
+            (\<exists> l1. (A,M,\<Lambda>,\<Gamma>,\<Omega>,T \<turnstile>(bb_next, cont0, Normal ns3) -n\<longrightarrow>^l1 (reached_bb, reached_cont, reached_state)) \<and> (l = Suc l1) )"
+  using assms
+proof (cases l)
+  case 0
+  then show ?thesis by (metis Ast.valid_configuration_def assms(1) get_state.simps is_final.simps(5) relpowp_0_E state.distinct(1))
+next
+  case 1: (Suc l1)
+  then show ?thesis 
+  proof -
+    from 1 assms obtain inter_bb inter_cont inter_state where
+      step1: "(red_bigblock A M \<Lambda> \<Gamma> \<Omega> T (BigBlock None [] None None, (KSeq bb_next cont0), Normal ns3) (inter_bb, inter_cont, inter_state))" and 
+      rest: "A,M,\<Lambda>,\<Gamma>,\<Omega>,T \<turnstile>(inter_bb, inter_cont, inter_state) -n\<longrightarrow>^l1 (reached_bb, reached_cont, reached_state)" 
+      by (metis (no_types, opaque_lifting) prod_cases3 relpowp_Suc_D2)
+    from this have "(inter_bb, inter_cont, inter_state) = (bb_next, (cont0), Normal ns3)"
+    proof cases
+      case RedSkip thus ?thesis by auto
+    qed auto
+    hence "(A,M,\<Lambda>,\<Gamma>,\<Omega>,T \<turnstile>(bb_next, cont0, Normal ns3) -n\<longrightarrow>^l1 (reached_bb, reached_cont, reached_state)) \<and> (l = Suc l1)" using rest \<open>l = Suc l1\<close> by simp
+    then show ?thesis by blast
+  qed
+qed
+
 lemma endblock_skip:
-  assumes "A,M,\<Lambda>,\<Gamma>,\<Omega>,T \<turnstile>(BigBlock None [] None None, KEndBlock (KSeq bb_next cont0), Normal ns3) -n\<longrightarrow>^l (reached_bb, reached_cont, reached_state)"
-  shows "(valid_configuration A \<Lambda> \<Gamma> \<Omega> [] reached_bb reached_cont reached_state) \<or> 
+  assumes "A,M,\<Lambda>,\<Gamma>,\<Omega>,T \<turnstile>(bb0, KEndBlock (KSeq bb_next cont0), Normal ns3) -n\<longrightarrow>^l (reached_bb, reached_cont, reached_state)"
+      and "bb0 = BigBlock None [] None None" 
+  shows "(valid_configuration A \<Lambda> \<Gamma> \<Omega> posts reached_bb reached_cont reached_state) \<or> 
             (\<exists> l2. (A,M,\<Lambda>,\<Gamma>,\<Omega>,T \<turnstile>(bb_next, cont0, Normal ns3) -n\<longrightarrow>^l2 (reached_bb, reached_cont, reached_state)) \<and> (l = Suc (Suc l2)) )"
   using assms
 proof (cases l)
   case 0
-  then show ?thesis by (metis Ast.valid_configuration_def assms get_state.simps is_final.simps(6) relpowp_fun_conv state.simps(3))
+  then show ?thesis by (metis Ast.valid_configuration_def assms(1) get_state.simps is_final.simps(6) relpowp_fun_conv state.simps(3))
 next
   case 1: (Suc l1)
   then show ?thesis 
@@ -131,14 +164,97 @@ next
   qed
 qed
 
+lemma correctness_propagates_through_empty:
+  assumes "\<forall>m s. (A,M,\<Lambda>,\<Gamma>,\<Omega>,G \<turnstile>(Inl n0, Normal ns1) -n\<rightarrow>* (m, s)) \<longrightarrow> s \<noteq> Failure"
+      and "node_to_block G ! n0 = []"
+      and "List.member (out_edges G ! n0) n1"
+    shows "\<And> m s. (A,M,\<Lambda>,\<Gamma>,\<Omega>,G \<turnstile>(Inl n1, Normal ns1) -n\<rightarrow>* (m, s)) \<Longrightarrow> s \<noteq> Failure"
+proof -
+  fix m1 s1
+  have a1: "(A,M,\<Lambda>,\<Gamma>,\<Omega> \<turnstile> \<langle>[], Normal ns1\<rangle> [\<rightarrow>] (Normal ns1))" by (rule RedCmdListNil)
+  show "(A,M,\<Lambda>,\<Gamma>,\<Omega>,G \<turnstile>(Inl n1, Normal ns1) -n\<rightarrow>* (m1, s1)) \<Longrightarrow> s1 \<noteq> Failure" 
+  proof -
+    assume "(A,M,\<Lambda>,\<Gamma>,\<Omega>,G \<turnstile>(Inl n1, Normal ns1) -n\<rightarrow>* (m1, s1))"
+    thus "s1 \<noteq> Failure" by (metis a1 assms(1-3) dag_verifies_propagate)
+  qed
+qed
+
+lemma wrapper_to_endblock:
+  assumes "A,M,\<Lambda>,\<Gamma>,\<Omega>,T \<turnstile>(bb0, cont0, Normal ns) -n\<longrightarrow>^l (reached_bb, reached_cont, reached_state)"
+      and "bb0 = BigBlock name [] (Some (WhileWrapper loop)) None"
+  shows "(valid_configuration A \<Lambda> \<Gamma> \<Omega> posts reached_bb reached_cont reached_state) \<or> 
+         (\<exists> l1. (A,M,\<Lambda>,\<Gamma>,\<Omega>,T \<turnstile>((BigBlock name [] (Some loop) None), KEndBlock cont0, Normal ns) -n\<longrightarrow>^l1 (reached_bb, reached_cont, reached_state)) \<and> (l = Suc l1))"
+  using assms
+proof (cases l)
+  case 0
+  hence "(reached_bb, reached_cont, reached_state) = (bb0, cont0, Normal ns)" using assms(1) by simp
+  then show ?thesis by (simp add: Ast.valid_configuration_def assms(2))
+next
+  case 1: (Suc l1)
+  then show ?thesis 
+  proof -
+    from 1 assms obtain inter_bb inter_cont inter_state where
+      step1: "(red_bigblock A M \<Lambda> \<Gamma> \<Omega> T (bb0, cont0, Normal ns) (inter_bb, inter_cont, inter_state))" and 
+      rest: "A,M,\<Lambda>,\<Gamma>,\<Omega>,T \<turnstile>(inter_bb, inter_cont, inter_state) -n\<longrightarrow>^l1 (reached_bb, reached_cont, reached_state)" 
+      by (metis (no_types, opaque_lifting) prod_cases3 relpowp_Suc_D2)
+    from this have "(inter_bb, inter_cont, inter_state) = (BigBlock name [] (Some loop) None, KEndBlock cont0, Normal ns)"
+    proof cases
+      case RedParsedWhileWrapper thus ?thesis using assms(2) by auto
+    qed (auto simp add: assms(2))
+    hence "(A,M,\<Lambda>,\<Gamma>,\<Omega>,T \<turnstile>(BigBlock name [] (Some loop) None, KEndBlock cont0, Normal ns) -n\<longrightarrow>^l1 (reached_bb, reached_cont, reached_state)) \<and> (l = Suc l1)" 
+      using rest \<open>l = Suc l1\<close> assms(2) by simp
+    then show ?thesis by blast
+  qed
+qed
+
+lemma ending3:
+  assumes "A,M,\<Lambda>,\<Gamma>,\<Omega>,T \<turnstile>(bb, cont0, Normal ns1'') -n\<longrightarrow>^j (reached_bb, reached_cont, reached_state)" 
+      and "bb = BigBlock name [] (Some (WhileWrapper loop)) None"
+      and "\<And>m3 s3. (A,M,\<Lambda>,\<Gamma>,\<Omega>,G \<turnstile>(Inl n, Normal ns1'') -n\<rightarrow>* (m3, s3)) \<Longrightarrow> s3 \<noteq> Failure"
+      and "\<And> j''. 
+            j = Suc j'' \<Longrightarrow>
+            A,M,\<Lambda>,\<Gamma>,\<Omega>,T \<turnstile>(BigBlock name [] (Some loop) None, KEndBlock cont0, Normal ns1'') -n\<longrightarrow>^j'' (reached_bb, reached_cont, reached_state) \<Longrightarrow>
+           (\<And>m' s'. A,M,\<Lambda>,\<Gamma>,\<Omega>,G \<turnstile>(Inl n, Normal ns1'') -n\<rightarrow>* (m', s') \<Longrightarrow> s' \<noteq> Failure) \<Longrightarrow>
+           (valid_configuration A \<Lambda> \<Gamma> \<Omega> posts reached_bb reached_cont reached_state)"
+    shows "valid_configuration A \<Lambda> \<Gamma> \<Omega> posts reached_bb reached_cont reached_state"
+proof -
+  from assms(1-2) have disj_a:
+    "(valid_configuration A \<Lambda> \<Gamma> \<Omega> posts reached_bb reached_cont reached_state) \<or> 
+       (\<exists> l1. (A,M,\<Lambda>,\<Gamma>,\<Omega>,T \<turnstile>(BigBlock name [] (Some loop) None, KEndBlock cont0, Normal ns1'') -n\<longrightarrow>^l1 (reached_bb, reached_cont, reached_state)) \<and> (j = Suc l1) )" 
+    by (simp add: wrapper_to_endblock)
+  thus ?thesis
+  proof cases
+    assume "(valid_configuration A \<Lambda> \<Gamma> \<Omega> posts reached_bb reached_cont reached_state)" thus ?thesis by simp
+  next 
+    assume "\<not> ((valid_configuration A \<Lambda> \<Gamma> \<Omega> posts reached_bb reached_cont reached_state))"
+    hence "(\<exists> l2. (A,M,\<Lambda>,\<Gamma>,\<Omega>,T \<turnstile>(BigBlock name [] (Some loop) None, KEndBlock cont0, Normal ns1'') -n\<longrightarrow>^l2 (reached_bb, reached_cont, reached_state)) \<and> (j = Suc l2) )" 
+      using disj_a by blast
+    thus ?thesis
+    proof -
+      obtain l2_conc where conc_trace: "(A,M,\<Lambda>,\<Gamma>,\<Omega>,T \<turnstile>(BigBlock name [] (Some loop) None, KEndBlock cont0, Normal ns1'') -n\<longrightarrow>^l2_conc (reached_bb, reached_cont, reached_state))" and 
+                           succ_rel: "(j = Suc l2_conc)"
+        using \<open>\<exists>l2. (A,M,\<Lambda>,\<Gamma>,\<Omega>,T \<turnstile>(BigBlock name [] (Some loop) None, KEndBlock cont0, Normal ns1'') -n\<longrightarrow>^l2 (reached_bb, reached_cont, reached_state)) \<and> j = Suc l2\<close> by blast
+      show ?thesis
+        apply (rule assms(4))
+          apply (rule succ_rel)
+         apply (rule conc_trace)
+        apply (rule assms(3))
+        apply (simp)
+        done
+    qed
+  qed
+qed
+
+
 lemma endblock_skip_wrapper:
-  assumes "A,M,\<Lambda>,\<Gamma>,\<Omega>,T \<turnstile>(BigBlock None [] None None, KEndBlock (KSeq (BigBlock name [] (Some (WhileWrapper str)) tr) cont0), Normal ns3) -n\<longrightarrow>^l (reached_bb, reached_cont, reached_state)"
-  shows "(valid_configuration A \<Lambda> \<Gamma> \<Omega> [] reached_bb reached_cont reached_state) \<or> 
+  assumes "A,M,\<Lambda>,\<Gamma>,\<Omega>,T \<turnstile>(bb0, KEndBlock (KSeq (BigBlock name [] (Some (WhileWrapper str)) tr) cont0), Normal ns3) -n\<longrightarrow>^l (reached_bb, reached_cont, reached_state)"
+      and "bb0 = BigBlock None [] None None"
+  shows "(valid_configuration A \<Lambda> \<Gamma> \<Omega> posts reached_bb reached_cont reached_state) \<or> 
          (\<exists> l3. (A,M,\<Lambda>,\<Gamma>,\<Omega>,T \<turnstile>((BigBlock name [] (Some str) tr), KEndBlock cont0, Normal ns3) -n\<longrightarrow>^l3 (reached_bb, reached_cont, reached_state)) \<and> (l = Suc (Suc (Suc l3))) )"
   using assms
 proof (cases l)
   case 0
-  then show ?thesis by (metis Ast.valid_configuration_def assms get_state.simps is_final.simps(6) relpowp_fun_conv state.simps(3))
+  then show ?thesis by (metis Ast.valid_configuration_def assms(1) get_state.simps is_final.simps(6) relpowp_fun_conv state.simps(3))
 next
   case 1: (Suc l1)
   then show ?thesis 
@@ -201,37 +317,39 @@ next
   qed
 qed
 
+
 text \<open>Local lemmas: The following are lemmas proving local relations between various kinds of ast-bigblocks and cfg-blocks\<close>
 
 text \<open>Local relation between an ast-bigblock starting with a non-empty set of simple commands and a cfg-block containing the same simple commands\<close>
 lemma block_local_rel_generic:
-  assumes block_rel: "ast_cfg_rel guard invs (BigBlock name cs1 any_str any_tr) cs2"
-  and "cs1 \<noteq> Nil"
-  and "cs2 \<noteq> Nil"
+  assumes block_rel: "ast_cfg_rel guard invs bb cs2"
   and "guard = None"
   and "invs = []"
-  and Red_bb_to: "red_bigblock A M \<Lambda> \<Gamma> \<Omega> T ((BigBlock name cs1 any_str any_tr), cont0, (Normal ns1)) (reached_bb, reached_cont, reached_state)" 
-  and Red_impl: "(\<And> s2'.((red_cmd_list A M \<Lambda> \<Gamma> \<Omega> cs2 (Normal ns1) s2') \<Longrightarrow> (s2' \<noteq> Failure)))" 
+  and Red_bb_to: "red_bigblock A M \<Lambda> \<Gamma> \<Omega> T (bb, cont0, (Normal ns1)) (reached_bb, reached_cont, reached_state)" 
+  and Red_impl: "(\<And> s2'.((red_cmd_list A M \<Lambda> \<Gamma> \<Omega> cs2 (Normal ns1) s2') \<Longrightarrow> (s2' \<noteq> Failure)))"
+  and "bb = (BigBlock name cs1 any_str any_tr)"
+  and "cs1 \<noteq> Nil"
+  and "cs2 \<noteq> Nil"
   shows "reached_state \<noteq> Failure  \<and>
          (\<forall>ns1'. reached_state = Normal ns1' \<longrightarrow> (A,M,\<Lambda>,\<Gamma>,\<Omega> \<turnstile> \<langle>cs2, Normal ns1\<rangle> [\<rightarrow>] Normal ns1'))" 
   using assms
 proof (induction arbitrary: ns1)
-  case (Rel_Main_test name cs1 any_str any_tr)
+  case (Rel_Main_test bb name cs1 any_str any_tr)
   thus ?case
   proof (cases cs1)
     case Nil
-    then show ?thesis using Rel_Main_test(2) by simp
+    then show ?thesis using \<open>cs1 \<noteq> Nil\<close> by simp
   next
     case (Cons a list)
     then have "red_bigblock A M \<Lambda> \<Gamma> \<Omega> T ((BigBlock name (a#list) any_str any_tr), cont0, (Normal ns1)) (reached_bb, reached_cont, reached_state)" 
-      using Rel_Main_test(5) by simp
+      using Rel_Main_test by blast
     then have "A,M,\<Lambda>,\<Gamma>,\<Omega> \<turnstile> \<langle>(a#list), Normal ns1\<rangle> [\<rightarrow>] reached_state" using Rel_Main_test(5) 
     proof cases
       case RedSimpleCmds thus ?thesis by (simp add: RedSimpleCmds)
     qed
     then have "A,M,\<Lambda>,\<Gamma>,\<Omega> \<turnstile> \<langle>cs1, Normal ns1\<rangle> [\<rightarrow>] reached_state" using Cons by simp
     
-    then show ?thesis using Rel_Main_test(6) by auto
+    then show ?thesis using Rel_Main_test by auto
   qed 
 qed auto
 
@@ -239,41 +357,43 @@ text \<open>Local relation between (an ast-bigblock starting with a non-empty se
                and (is the first ast-bigblock in the then-branch of an if-statement or is the first ast-bigblock in the body of a while-loop)) 
        and a cfg-block containing the same simple commands\<close>
 lemma block_local_rel_guard_true:
-  assumes block_rel: "ast_cfg_rel None [] (BigBlock name cs1 any_str any_tr) cs2"
-  and "cs1 \<noteq> Nil"
-  and "cs2 \<noteq> Nil"
+  assumes block_rel: "ast_cfg_rel None [] bb cs2"
   and "c = Assume block_guard"
   and trace_is_possible: "A,\<Lambda>,\<Gamma>,\<Omega> \<turnstile> \<langle>block_guard, ns1\<rangle> \<Down> LitV (LBool True)"
-  and Red_bb_to: "red_bigblock A M \<Lambda> \<Gamma> \<Omega> T ((BigBlock name cs1 any_str any_tr), cont0, (Normal ns1)) (reached_bb, reached_cont, reached_state)" 
-  and Red_impl: "(\<And> s2'.((red_cmd_list A M \<Lambda> \<Gamma> \<Omega> (c#cs2) (Normal ns1) s2') \<Longrightarrow> (s2' \<noteq> Failure)))" 
+  and Red_bb_to: "red_bigblock A M \<Lambda> \<Gamma> \<Omega> T (bb, cont0, (Normal ns1)) (reached_bb, reached_cont, reached_state)" 
+  and Red_impl: "(\<And> s2'.((red_cmd_list A M \<Lambda> \<Gamma> \<Omega> (cs3) (Normal ns1) s2') \<Longrightarrow> (s2' \<noteq> Failure)))" 
+  and "bb = (BigBlock name cs1 any_str any_tr)"
+  and "cs1 \<noteq> Nil"
+  and "cs2 \<noteq> Nil"
+  and "cs3 = (c#cs2)"
   shows "reached_state \<noteq> Failure  \<and>
-         (\<forall>ns1'. reached_state = Normal ns1' \<longrightarrow> (A,M,\<Lambda>,\<Gamma>,\<Omega> \<turnstile> \<langle>(c#cs2), Normal ns1\<rangle> [\<rightarrow>] Normal ns1'))" 
+         (\<forall>ns1'. reached_state = Normal ns1' \<longrightarrow> (A,M,\<Lambda>,\<Gamma>,\<Omega> \<turnstile> \<langle>cs3, Normal ns1\<rangle> [\<rightarrow>] Normal ns1'))" 
   using assms 
 proof cases
   case Rel_Main_test
   have Red_impl_extended: "(\<And> s2'.((red_cmd_list A M \<Lambda> \<Gamma> \<Omega> cs2 (Normal ns1) s2') \<Longrightarrow> (s2' \<noteq> Failure)))" 
-    using trace_is_possible \<open>c = Assume block_guard\<close> Red_impl RedAssumeOk RedCmdListCons by blast
+    using trace_is_possible \<open>c = Assume block_guard\<close> Red_impl RedAssumeOk RedCmdListCons \<open>cs3 = c#cs2\<close> by blast
   hence snd_step_to_end: "reached_state \<noteq> Failure  \<and> (\<forall>ns1'. reached_state = Normal ns1' \<longrightarrow> (A,M,\<Lambda>,\<Gamma>,\<Omega> \<turnstile> \<langle>cs2, Normal ns1\<rangle> [\<rightarrow>] Normal ns1'))"
-    using Red_bb_to assms(2-3) block_local_rel_generic block_rel 
-    by blast 
+    using Red_bb_to assms(6-8) block_local_rel_generic block_rel by metis
   have push_one_cmd: "A,M,\<Lambda>,\<Gamma>,\<Omega> \<turnstile> \<langle>c, Normal ns1\<rangle> \<rightarrow> Normal ns1" 
     using \<open>c = Assume block_guard\<close> trace_is_possible 
     by (simp only: RedAssumeOk)
-  then show ?thesis using snd_step_to_end  by (simp add: RedCmdListCons)
+  then show ?thesis using snd_step_to_end by (simp add: RedCmdListCons \<open>cs3 = c#cs2\<close>)
 qed auto
 
 text \<open>Local relation between (an ast-bigblock starting with a non-empty set of simple commands 
                and (is the first ast-bigblock in the else-branch of an if-statement or is the first ast-bigblock after a while-loop)) 
        and a cfg-block containing the same simple commands\<close>
 lemma block_local_rel_guard_false:
-  assumes block_rel: "ast_cfg_rel None [] (BigBlock name cs1 any_str any_tr) cs2"
-  and "cs1 \<noteq> Nil"
-  and "cs2 \<noteq> Nil"
+  assumes block_rel: "ast_cfg_rel None [] bb cs2"
   and "(UnOp Not block_guard) \<sim> b "
   and "c = Assume b"
   and trace_is_possible: "A,\<Lambda>,\<Gamma>,\<Omega> \<turnstile> \<langle>(UnOp Not block_guard), ns1\<rangle> \<Down> LitV (LBool True)"
-  and Red_bb_to: "red_bigblock A M \<Lambda> \<Gamma> \<Omega> T ((BigBlock name cs1 any_str any_tr), cont0, (Normal ns1)) (reached_bb, reached_cont, reached_state)" 
+  and Red_bb_to: "red_bigblock A M \<Lambda> \<Gamma> \<Omega> T (bb, cont0, (Normal ns1)) (reached_bb, reached_cont, reached_state)" 
   and Red_impl: "(\<And> s2'.((red_cmd_list A M \<Lambda> \<Gamma> \<Omega> (c#cs2) (Normal ns1) s2') \<Longrightarrow> (s2' \<noteq> Failure)))" 
+  and "bb = (BigBlock name cs1 any_str any_tr)"
+  and "cs1 \<noteq> Nil"
+  and "cs2 \<noteq> Nil"
   shows "reached_state \<noteq> Failure  \<and>
          (\<forall>ns1'. reached_state = Normal ns1' \<longrightarrow> (A,M,\<Lambda>,\<Gamma>,\<Omega> \<turnstile> \<langle>(c#cs2), Normal ns1\<rangle> [\<rightarrow>] Normal ns1'))" 
   using assms 
@@ -282,8 +402,7 @@ proof cases
   have Red_impl_extended: "(\<And> s2'.((red_cmd_list A M \<Lambda> \<Gamma> \<Omega> cs2 (Normal ns1) s2') \<Longrightarrow> (s2' \<noteq> Failure)))" 
     using trace_is_possible \<open>c = Assume b\<close> \<open>(UnOp Not block_guard) \<sim> b\<close> equiv_preserves_value  Red_impl RedAssumeOk RedCmdListCons by metis
   hence snd_step_to_end: "reached_state \<noteq> Failure  \<and> (\<forall>ns1'. reached_state = Normal ns1' \<longrightarrow> (A,M,\<Lambda>,\<Gamma>,\<Omega> \<turnstile> \<langle>cs2, Normal ns1\<rangle> [\<rightarrow>] Normal ns1'))"
-    using Red_bb_to assms(2-3) block_local_rel_generic block_rel 
-    by blast 
+    using Red_bb_to assms(7-9) block_local_rel_generic block_rel by metis
   have equiv: "A,\<Lambda>,\<Gamma>,\<Omega> \<turnstile> \<langle>b, ns1\<rangle> \<Down> BoolV True" 
     using trace_is_possible equiv_preserves_value \<open>(UnOp Not block_guard) \<sim> b\<close>
     by metis
@@ -295,35 +414,36 @@ qed auto
 
 text \<open>Local relation between a loop-only(no simple commands) ast-bigblock and a corresponding cfg-block containing assertions of the loop invariants\<close>
 lemma block_local_rel_loop_head:
-  assumes block_rel: "ast_cfg_rel None assert_invs (BigBlock name [] (Some (ParsedWhile loop_guard invs (bb0#body_bbs))) any_tr) assertions"
+  assumes block_rel: "ast_cfg_rel None assert_invs bb assertions"
+  and "bb =  (BigBlock name [] (Some (ParsedWhile loop_guard invs (bb0#body_bbs))) any_tr)"
   and "assert_invs = map inv_into_assertion invs"
-  and Red_bb: "red_bigblock A M \<Lambda> \<Gamma> \<Omega> T ((BigBlock name [] (Some (ParsedWhile loop_guard invs (bb0#body_bbs))) any_tr), cont0, (Normal ns1)) (reached_bb, reached_cont, reached_state)" 
+  and Red_bb: "red_bigblock A M \<Lambda> \<Gamma> \<Omega> T (bb, cont0, (Normal ns1)) (reached_bb, reached_cont, reached_state)" 
   and Red_impl: "(\<And> s2'.((red_cmd_list A M \<Lambda> \<Gamma> \<Omega> assertions (Normal ns1) s2') \<Longrightarrow> (s2' \<noteq> Failure)))"
   shows "reached_state \<noteq> Failure  \<and>
          (\<forall>ns1'. reached_state = Normal ns1' \<longrightarrow> (A,M,\<Lambda>,\<Gamma>,\<Omega> \<turnstile> \<langle>assertions, Normal ns1\<rangle> [\<rightarrow>] Normal ns1'))" 
   using assms
 proof cases
   case Rel_Invs
-  hence "assertions = map inv_into_assertion invs" using assms(2) by simp
+  hence "assertions = map inv_into_assertion invs" using assms(3) by simp
   from Red_bb show ?thesis
   proof cases
-    case RedParsedWhileTrue thus ?thesis using \<open>assertions = (map inv_into_assertion invs)\<close>  by (simp add: asserts_hold_if_invs_hold)
+    case RedParsedWhileTrue thus ?thesis using \<open>assertions = (map inv_into_assertion invs)\<close>  by (simp add: asserts_hold_if_invs_hold assms(2))
   next
-    case RedParsedWhileFalse thus ?thesis using \<open>assertions = (map inv_into_assertion invs)\<close>  by (simp add: asserts_hold_if_invs_hold)
+    case RedParsedWhileFalse thus ?thesis using \<open>assertions = (map inv_into_assertion invs)\<close>  by (simp add: asserts_hold_if_invs_hold assms(2))
   next
-    case RedParsedWhile_InvFail thus ?thesis using Red_impl \<open>assertions = map inv_into_assertion invs\<close> one_inv_fails_assertions by blast
-  qed auto
+    case RedParsedWhile_InvFail thus ?thesis using Red_impl \<open>assertions = map inv_into_assertion invs\<close> one_inv_fails_assertions assms(2) by blast
+  qed (auto simp add: assms(2))
 next
   case Rel_Main_test
-  hence "assertions = map inv_into_assertion invs" using assms(2) by simp
+  hence "assertions = map inv_into_assertion invs" using assms(2-3) by simp
   from Red_bb show ?thesis
   proof cases
-    case RedParsedWhileTrue thus ?thesis using \<open>assertions = (map inv_into_assertion invs)\<close>  by (simp add: asserts_hold_if_invs_hold)
+    case RedParsedWhileTrue thus ?thesis using \<open>assertions = (map inv_into_assertion invs)\<close>  by (simp add: asserts_hold_if_invs_hold assms(2))
   next
-    case RedParsedWhileFalse thus ?thesis using \<open>assertions = (map inv_into_assertion invs)\<close>  by (simp add: asserts_hold_if_invs_hold)
+    case RedParsedWhileFalse thus ?thesis using \<open>assertions = (map inv_into_assertion invs)\<close>  by (simp add: asserts_hold_if_invs_hold assms(2))
   next
-    case RedParsedWhile_InvFail thus ?thesis using Red_impl \<open>assertions = map inv_into_assertion invs\<close> one_inv_fails_assertions by blast
-  qed auto
+    case RedParsedWhile_InvFail thus ?thesis using Red_impl \<open>assertions = map inv_into_assertion invs\<close> one_inv_fails_assertions assms(2) by blast
+  qed (auto simp add: assms(2))
 qed
 
 text \<open>Global lemmas: The following are lemmas proving global relations between various kinds of ast-bigblocks and cfg-blocks\<close>
@@ -334,39 +454,40 @@ text \<open>'ending', 'ending2' and 'correctness_propagates_through_assumption' 
        we're proving a global lemma for the head of a loop that is followed by another loop (not nested).\<close>
 lemma ending:
   assumes "j = Suc j'" 
-      and "A,M,\<Lambda>,\<Gamma>,\<Omega>,T \<turnstile>(BigBlock None [] None None, KEndBlock (KSeq bigblock_next KStop), Normal ns1'') -n\<longrightarrow>^j' (reached_bb, reached_cont, reached_state)" 
+      and "A,M,\<Lambda>,\<Gamma>,\<Omega>,T \<turnstile>(bb, KEndBlock (KSeq bigblock_next cont0), Normal ns1'') -n\<longrightarrow>^j' (reached_bb, reached_cont, reached_state)" 
+      and "bb = BigBlock None [] None None"
       and "\<And>m3 s3. (A,M,\<Lambda>,\<Gamma>,\<Omega>,G \<turnstile>(Inl n, Normal ns1'') -n\<rightarrow>* (m3, s3)) \<Longrightarrow> s3 \<noteq> Failure"
       and "A,\<Lambda>,\<Gamma>,\<Omega> \<turnstile> \<langle>guard,ns1''\<rangle> \<Down> BoolV False" 
       and "\<And> j''. 
             j' = Suc (Suc j'') \<Longrightarrow>
-            A,M,\<Lambda>,\<Gamma>,\<Omega>,T \<turnstile>(bigblock_next, KStop, Normal ns1'') -n\<longrightarrow>^j'' (reached_bb, reached_cont, reached_state) \<Longrightarrow>
+            A,M,\<Lambda>,\<Gamma>,\<Omega>,T \<turnstile>(bigblock_next, cont0, Normal ns1'') -n\<longrightarrow>^j'' (reached_bb, reached_cont, reached_state) \<Longrightarrow>
            (\<And>m' s'. A,M,\<Lambda>,\<Gamma>,\<Omega>,G \<turnstile>(Inl n, Normal ns1'') -n\<rightarrow>* (m', s') \<Longrightarrow> s' \<noteq> Failure) \<Longrightarrow>
-           (A,\<Lambda>,\<Gamma>,\<Omega> \<turnstile> \<langle>UnOp Not guard,ns1''\<rangle> \<Down> BoolV True) \<Longrightarrow> (valid_configuration A \<Lambda> \<Gamma> \<Omega> [] reached_bb reached_cont reached_state)"
-    shows "valid_configuration A \<Lambda> \<Gamma> \<Omega> [] reached_bb reached_cont reached_state"
+           (A,\<Lambda>,\<Gamma>,\<Omega> \<turnstile> \<langle>UnOp Not guard,ns1''\<rangle> \<Down> BoolV True) \<Longrightarrow> (valid_configuration A \<Lambda> \<Gamma> \<Omega> posts reached_bb reached_cont reached_state)"
+    shows "valid_configuration A \<Lambda> \<Gamma> \<Omega> posts reached_bb reached_cont reached_state"
 proof -
-  from assms(2) have disj_a:
-    "(valid_configuration A \<Lambda> \<Gamma> \<Omega> [] reached_bb reached_cont reached_state) \<or> 
-       (\<exists> l2. (A,M,\<Lambda>,\<Gamma>,\<Omega>,T \<turnstile>(bigblock_next, KStop, Normal ns1'') -n\<longrightarrow>^l2 (reached_bb, reached_cont, reached_state)) \<and> (j' = Suc (Suc l2)) )" 
+  from assms(2-3) have disj_a:
+    "(valid_configuration A \<Lambda> \<Gamma> \<Omega> posts reached_bb reached_cont reached_state) \<or> 
+       (\<exists> l2. (A,M,\<Lambda>,\<Gamma>,\<Omega>,T \<turnstile>(bigblock_next, cont0, Normal ns1'') -n\<longrightarrow>^l2 (reached_bb, reached_cont, reached_state)) \<and> (j' = Suc (Suc l2)) )" 
     by (simp add: endblock_skip)
   thus ?thesis
   proof cases
-    assume "(valid_configuration A \<Lambda> \<Gamma> \<Omega> [] reached_bb reached_cont reached_state)" thus ?thesis by simp
+    assume "(valid_configuration A \<Lambda> \<Gamma> \<Omega> posts reached_bb reached_cont reached_state)" thus ?thesis by simp
   next 
-    assume "\<not> ((valid_configuration A \<Lambda> \<Gamma> \<Omega> [] reached_bb reached_cont reached_state))"
-    hence "(\<exists> l2. (A,M,\<Lambda>,\<Gamma>,\<Omega>,T \<turnstile>(bigblock_next, KStop, Normal ns1'') -n\<longrightarrow>^l2 (reached_bb, reached_cont, reached_state)) \<and> (j' = Suc (Suc l2)) )" 
+    assume "\<not> ((valid_configuration A \<Lambda> \<Gamma> \<Omega> posts reached_bb reached_cont reached_state))"
+    hence "(\<exists> l2. (A,M,\<Lambda>,\<Gamma>,\<Omega>,T \<turnstile>(bigblock_next, cont0, Normal ns1'') -n\<longrightarrow>^l2 (reached_bb, reached_cont, reached_state)) \<and> (j' = Suc (Suc l2)) )" 
       using disj_a by blast
     thus ?thesis
     proof -
-      obtain l2_conc where conc_trace: "(A,M,\<Lambda>,\<Gamma>,\<Omega>,T \<turnstile>(bigblock_next, KStop, Normal ns1'') -n\<longrightarrow>^l2_conc (reached_bb, reached_cont, reached_state))" and 
+      obtain l2_conc where conc_trace: "(A,M,\<Lambda>,\<Gamma>,\<Omega>,T \<turnstile>(bigblock_next, cont0, Normal ns1'') -n\<longrightarrow>^l2_conc (reached_bb, reached_cont, reached_state))" and 
                            succ_rel: "(j' = Suc (Suc l2_conc))"
-        using \<open>\<exists>l2. (A,M,\<Lambda>,\<Gamma>,\<Omega>,T \<turnstile>(bigblock_next, KStop, Normal ns1'') -n\<longrightarrow>^l2 (reached_bb, reached_cont, reached_state)) \<and> j' = Suc (Suc l2)\<close> by blast
+        using \<open>\<exists>l2. (A,M,\<Lambda>,\<Gamma>,\<Omega>,T \<turnstile>(bigblock_next, cont0, Normal ns1'') -n\<longrightarrow>^l2 (reached_bb, reached_cont, reached_state)) \<and> j' = Suc (Suc l2)\<close> by blast
       show ?thesis
-        apply (rule assms(5))
+        apply (rule assms(6))
            apply (rule succ_rel)
           apply (rule conc_trace)
-         apply (rule assms(3))
+         apply (rule assms(4))
          apply (simp)
-        using assms(4) false_equals_not_true 
+        using assms(5) false_equals_not_true 
         by blast
     qed
   qed
@@ -390,12 +511,29 @@ proof -
   qed
 qed
 
+lemma correctness_propagates_through_assumption2:
+  assumes "\<forall>m s. (A,M,\<Lambda>,\<Gamma>,\<Omega>,G \<turnstile>(Inl n0, Normal ns1) -n\<rightarrow>* (m, s)) \<longrightarrow> s \<noteq> Failure"
+      and "node_to_block G ! n0 = [Assume guard]"
+      and "A,\<Lambda>,\<Gamma>,\<Omega> \<turnstile> \<langle>guard, ns1\<rangle> \<Down> BoolV True"
+      and "List.member (out_edges G ! n0) n1"
+    shows "\<And> m s. (A,M,\<Lambda>,\<Gamma>,\<Omega>,G \<turnstile>(Inl n1, Normal ns1) -n\<rightarrow>* (m, s)) \<Longrightarrow> s \<noteq> Failure"
+proof -
+  fix m1 s1
+  have a1: "(A,M,\<Lambda>,\<Gamma>,\<Omega> \<turnstile> \<langle>[Assume guard], Normal ns1\<rangle> [\<rightarrow>] (Normal ns1))" by (meson RedAssumeOk assms(3) red_cmd_list.simps)
+  show "(A,M,\<Lambda>,\<Gamma>,\<Omega>,G \<turnstile>(Inl n1, Normal ns1) -n\<rightarrow>* (m1, s1)) \<Longrightarrow> s1 \<noteq> Failure" 
+  proof -
+    assume "(A,M,\<Lambda>,\<Gamma>,\<Omega>,G \<turnstile>(Inl n1, Normal ns1) -n\<rightarrow>* (m1, s1))"
+    thus "s1 \<noteq> Failure" using a1 assms(1-2) assms(4) dag_verifies_propagate by blast 
+  qed
+qed
+
 lemma ending2:
   assumes "j = Suc j'"
-      and "A,M,\<Lambda>,\<Gamma>,\<Omega>,T \<turnstile>(BigBlock None [] None None,
+      and "A,M,\<Lambda>,\<Gamma>,\<Omega>,T \<turnstile>(bb,
                       KEndBlock (KSeq (BigBlock None [] (Some (WhileWrapper (ParsedWhile next_guard next_invs (next_body_bb#body_bbs)))) None) cont1),
                       Normal ns1'') -n\<longrightarrow>^j'
            (reached_bb, reached_cont, reached_state)"
+      and "bb = BigBlock None [] None None"
       and corr: "\<forall>m3 s3. (A,M,\<Lambda>,\<Gamma>,\<Omega>,G \<turnstile>(Inl n, Normal ns1'') -n\<rightarrow>* (m3, s3)) \<longrightarrow> s3 \<noteq> Failure"
       and guard_false: "A,\<Lambda>,\<Gamma>,\<Omega> \<turnstile> \<langle>guard, ns1''\<rangle> \<Down> BoolV False" 
       and "node_to_block G ! n = [Assume c]" 
@@ -409,20 +547,20 @@ lemma ending2:
           A,M,\<Lambda>,\<Gamma>,\<Omega>,T \<turnstile>((BigBlock None [] (Some (ParsedWhile next_guard next_invs (next_body_bb#body_bbs))) None), KEndBlock cont1, Normal ns1'') -n\<longrightarrow>^j''' 
               (reached_bb, reached_cont, reached_state) \<Longrightarrow>
           (\<And>m' s'. A,M,\<Lambda>,\<Gamma>,\<Omega>,G \<turnstile>(Inl n1, Normal ns1'') -n\<rightarrow>* (m', s') \<Longrightarrow> s' \<noteq> Failure) \<Longrightarrow> 
-          (Ast.valid_configuration A \<Lambda> \<Gamma> \<Omega> [] reached_bb reached_cont reached_state)"
-    shows "(Ast.valid_configuration A \<Lambda> \<Gamma> \<Omega> [] reached_bb reached_cont reached_state)"
+          (Ast.valid_configuration A \<Lambda> \<Gamma> \<Omega> posts reached_bb reached_cont reached_state)"
+    shows "(Ast.valid_configuration A \<Lambda> \<Gamma> \<Omega> posts reached_bb reached_cont reached_state)"
   using assms
 proof -
-  from assms(2) have disj_a:
-    "(valid_configuration A \<Lambda> \<Gamma> \<Omega> [] reached_bb reached_cont reached_state) \<or> 
+  from assms(2-3) have disj_a:
+    "(valid_configuration A \<Lambda> \<Gamma> \<Omega> posts reached_bb reached_cont reached_state) \<or> 
        (\<exists> l3. (A,M,\<Lambda>,\<Gamma>,\<Omega>,T \<turnstile> ((BigBlock None [] (Some (ParsedWhile next_guard next_invs (next_body_bb#body_bbs))) None), KEndBlock cont1, Normal ns1'') 
               -n\<longrightarrow>^l3 (reached_bb, reached_cont, reached_state)) \<and> (j' = Suc (Suc (Suc l3))) )"
     by (simp add: endblock_skip_wrapper)
   thus ?thesis
   proof cases
-    assume "(valid_configuration A \<Lambda> \<Gamma> \<Omega> [] reached_bb reached_cont reached_state)" thus ?thesis by simp
+    assume "(valid_configuration A \<Lambda> \<Gamma> \<Omega> posts reached_bb reached_cont reached_state)" thus ?thesis by simp
   next 
-    assume "\<not> ((valid_configuration A \<Lambda> \<Gamma> \<Omega> [] reached_bb reached_cont reached_state))"
+    assume "\<not> ((valid_configuration A \<Lambda> \<Gamma> \<Omega> posts reached_bb reached_cont reached_state))"
     hence skipped_endblock: 
                   "(\<exists> l3. (A,M,\<Lambda>,\<Gamma>,\<Omega>,T \<turnstile>((BigBlock None [] (Some (ParsedWhile next_guard next_invs (next_body_bb#body_bbs))) None), KEndBlock cont1, Normal ns1'') 
                    -n\<longrightarrow>^l3 (reached_bb, reached_cont, reached_state)) \<and> (j' = Suc (Suc (Suc l3))) )" 
@@ -433,6 +571,118 @@ proof -
            conc_trace: "(A,M,\<Lambda>,\<Gamma>,\<Omega>,T \<turnstile>((BigBlock None [] (Some (ParsedWhile next_guard next_invs (next_body_bb#body_bbs))) None), KEndBlock cont1, Normal ns1'') 
                         -n\<longrightarrow>^l3_conc (reached_bb, reached_cont, reached_state))" and 
            succ_rel: "(j' = Suc (Suc (Suc l3_conc))) " 
+        using skipped_endblock by blast
+      show ?thesis
+        apply (rule assms(9))
+             apply (rule succ_rel)
+            apply (simp add: assms)
+           apply (rule assms(7))
+          apply (rule assms(8))
+         apply (rule conc_trace)
+        apply (rule correctness_propagates_through_assumption)
+             apply (rule corr)
+            apply (rule assms(6))
+           apply (rule assms(7))
+          apply (rule guard_false)
+         apply (rule assms(8))
+        apply simp
+        done
+    qed
+  qed
+qed
+
+lemma ending_then:
+  assumes "A,M,\<Lambda>,\<Gamma>,\<Omega>,T \<turnstile>(bb, KSeq bb_next cont1, Normal ns1'') -n\<longrightarrow>^j (reached_bb, reached_cont, reached_state)"
+      and "bb = BigBlock None [] None None"
+      and guard_true: "A,\<Lambda>,\<Gamma>,\<Omega> \<turnstile> \<langle>guard, ns1''\<rangle> \<Down> BoolV True" 
+      and "node_to_block G ! n = cs2"
+      and "cs2 = [Assume guard]"
+      and "List.member (out_edges(G) ! n) n1"
+      and corr: "\<forall>m3 s3. (A,M,\<Lambda>,\<Gamma>,\<Omega>,G \<turnstile>(Inl n, Normal ns1'') -n\<rightarrow>* (m3, s3)) \<longrightarrow> s3 \<noteq> Failure"
+      and "\<And> j''.
+          j = (Suc j'') \<Longrightarrow>
+          node_to_block G ! n = cs2 \<Longrightarrow>
+          List.member (out_edges(G) ! n) n1 \<Longrightarrow>
+          A,M,\<Lambda>,\<Gamma>,\<Omega>,T \<turnstile>(bb_next, cont1, Normal ns1'') -n\<longrightarrow>^j'' (reached_bb, reached_cont, reached_state) \<Longrightarrow>
+          (\<And>m' s'. A,M,\<Lambda>,\<Gamma>,\<Omega>,G \<turnstile>(Inl n1, Normal ns1'') -n\<rightarrow>* (m', s') \<Longrightarrow> s' \<noteq> Failure) \<Longrightarrow> 
+          (Ast.valid_configuration A \<Lambda> \<Gamma> \<Omega> posts reached_bb reached_cont reached_state)"
+    shows "(Ast.valid_configuration A \<Lambda> \<Gamma> \<Omega> posts reached_bb reached_cont reached_state)"
+  using assms
+proof -
+  from assms(1-2) have disj_a:
+    "(valid_configuration A \<Lambda> \<Gamma> \<Omega> posts reached_bb reached_cont reached_state) \<or> 
+       (\<exists> l1. (A,M,\<Lambda>,\<Gamma>,\<Omega>,T \<turnstile> (bb_next, cont1, Normal ns1'') -n\<longrightarrow>^l1 (reached_bb, reached_cont, reached_state)) \<and> (j = Suc l1) )"
+    by (simp add: seq_skip)
+  thus ?thesis
+  proof cases
+    assume "(valid_configuration A \<Lambda> \<Gamma> \<Omega> posts reached_bb reached_cont reached_state)" thus ?thesis by simp
+  next 
+    assume "\<not> ((valid_configuration A \<Lambda> \<Gamma> \<Omega> posts reached_bb reached_cont reached_state))"
+    hence skipped_endblock: 
+                  "(\<exists> l1. (A,M,\<Lambda>,\<Gamma>,\<Omega>,T \<turnstile>(bb_next, cont1, Normal ns1'') 
+                   -n\<longrightarrow>^l1 (reached_bb, reached_cont, reached_state)) \<and> (j = Suc l1) )" 
+      using disj_a by blast
+    thus ?thesis
+    proof -
+      obtain l1_conc where 
+           conc_trace: "(A,M,\<Lambda>,\<Gamma>,\<Omega>,T \<turnstile>(bb_next, cont1, Normal ns1'') -n\<longrightarrow>^l1_conc (reached_bb, reached_cont, reached_state))" and 
+           succ_rel: "(j = Suc l1_conc) " 
+        using skipped_endblock by blast
+      show ?thesis
+        apply (rule assms(8))
+             apply (rule succ_rel)
+            apply (simp add: assms)
+           apply (rule assms(6))
+         apply (rule conc_trace)
+        apply (rule correctness_propagates_through_assumption2)
+            apply (rule corr)
+           apply (simp add: assms(4))
+           apply (rule assms(5))
+          apply (rule guard_true)
+         apply (rule assms(6))
+        apply simp
+        done
+    qed
+  qed
+qed
+
+lemma ending_else:
+  assumes "A,M,\<Lambda>,\<Gamma>,\<Omega>,T \<turnstile>(bb, KSeq bb_next cont1, Normal ns1'') -n\<longrightarrow>^j (reached_bb, reached_cont, reached_state)"
+      and "bb = BigBlock None [] None None"
+      and corr: "\<forall>m3 s3. (A,M,\<Lambda>,\<Gamma>,\<Omega>,G \<turnstile>(Inl n, Normal ns1'') -n\<rightarrow>* (m3, s3)) \<longrightarrow> s3 \<noteq> Failure"
+      and guard_false: "A,\<Lambda>,\<Gamma>,\<Omega> \<turnstile> \<langle>guard, ns1''\<rangle> \<Down> BoolV False" 
+      and "node_to_block G ! n = [Assume c]" 
+      and "(UnOp Not guard) \<sim> c"
+      and "List.member (out_edges(G) ! n) n1"
+      and "\<And> j''.
+          j = (Suc j'') \<Longrightarrow>
+          node_to_block G ! n = [Assume c] \<Longrightarrow>
+          (UnOp Not guard) \<sim> c \<Longrightarrow>
+          List.member (out_edges(G) ! n) n1 \<Longrightarrow>
+          A,M,\<Lambda>,\<Gamma>,\<Omega>,T \<turnstile>(bb_next, cont1, Normal ns1'') -n\<longrightarrow>^j'' (reached_bb, reached_cont, reached_state) \<Longrightarrow>
+          (\<And>m' s'. A,M,\<Lambda>,\<Gamma>,\<Omega>,G \<turnstile>(Inl n1, Normal ns1'') -n\<rightarrow>* (m', s') \<Longrightarrow> s' \<noteq> Failure) \<Longrightarrow> 
+          (Ast.valid_configuration A \<Lambda> \<Gamma> \<Omega> posts reached_bb reached_cont reached_state)"
+    shows "(Ast.valid_configuration A \<Lambda> \<Gamma> \<Omega> posts reached_bb reached_cont reached_state)"
+  using assms
+proof -
+  from assms(1-2) have disj_a:
+    "(valid_configuration A \<Lambda> \<Gamma> \<Omega> posts reached_bb reached_cont reached_state) \<or> 
+       (\<exists> l1. (A,M,\<Lambda>,\<Gamma>,\<Omega>,T \<turnstile> (bb_next, cont1, Normal ns1'') -n\<longrightarrow>^l1 (reached_bb, reached_cont, reached_state)) \<and> (j = Suc l1) )"
+    by (simp add: seq_skip)
+  thus ?thesis
+  proof cases
+    assume "(valid_configuration A \<Lambda> \<Gamma> \<Omega> posts reached_bb reached_cont reached_state)" thus ?thesis by simp
+  next 
+    assume "\<not> ((valid_configuration A \<Lambda> \<Gamma> \<Omega> posts reached_bb reached_cont reached_state))"
+    hence skipped_endblock: 
+                  "(\<exists> l1. (A,M,\<Lambda>,\<Gamma>,\<Omega>,T \<turnstile>(bb_next, cont1, Normal ns1'') 
+                   -n\<longrightarrow>^l1 (reached_bb, reached_cont, reached_state)) \<and> (j = Suc l1) )" 
+      using disj_a by blast
+    thus ?thesis
+    proof -
+      obtain l1_conc where 
+           conc_trace: "(A,M,\<Lambda>,\<Gamma>,\<Omega>,T \<turnstile>(bb_next, cont1, Normal ns1'') -n\<longrightarrow>^l1_conc (reached_bb, reached_cont, reached_state))" and 
+           succ_rel: "(j = Suc l1_conc) " 
         using skipped_endblock by blast
       show ?thesis
         apply (rule assms(8))
@@ -453,102 +703,149 @@ proof -
   qed
 qed
 
+
 text \<open>Global lemma for an ast-bigblock with a non-empty set of simple commands which concludes the program and is immediately after a loop.\<close>
 lemma generic_ending_block_after_loop_global_rel:
-  assumes syn_rel: "ast_cfg_rel None [] (BigBlock name cs1 None any_tr) cs2"
+  assumes syn_rel: "ast_cfg_rel None [] bb cs2"
+  and "bb = (BigBlock name cs1 None any_tr)"
   and "(any_tr = None) \<or> (any_tr = (Some (Return val1)))"
-  and "cs1 \<noteq> Nil"
-  and "cs2 \<noteq> Nil"
-  and "node_to_block G ! n = (c#cs2)" 
+  and "node_to_block G ! n = (cs3)"
+  and "cs3 = c#cs2"
   and "c = Assume b"
   and "(UnOp Not guard) \<sim> b"
   and trace_is_possible: "A,\<Lambda>,\<Gamma>,\<Omega> \<turnstile> \<langle>UnOp Not guard, ns1\<rangle> \<Down> BoolV True"
-  and j_step_ast_trace: "A,M,\<Lambda>,\<Gamma>,\<Omega>,T \<turnstile> ((BigBlock name cs1 None any_tr), KStop, (Normal ns1)) -n\<longrightarrow>^j (reached_bb, reached_cont, reached_state)"
+  and j_step_ast_trace: "A,M,\<Lambda>,\<Gamma>,\<Omega>,T \<turnstile> (bb, KStop, (Normal ns1)) -n\<longrightarrow>^j (reached_bb, reached_cont, reached_state)"
   and cfg_is_correct: "\<And> m' s'. (red_cfg_multi A M \<Lambda> \<Gamma> \<Omega> G ((Inl n),(Normal ns1)) (m',s')) \<Longrightarrow> (s' \<noteq> Failure)"
   shows "(valid_configuration A \<Lambda> \<Gamma> \<Omega> [] reached_bb reached_cont reached_state)" 
   using assms
-proof (cases j)
-  case 0
-  from this j_step_ast_trace have "(reached_bb, reached_cont, reached_state) = ((BigBlock name cs1 None any_tr), KStop, (Normal ns1))" by simp
-  then show ?thesis by (simp add: valid_configuration_def expr_all_sat_def)
-next
-  case (Suc j')
-  from this j_step_ast_trace obtain inter_bb inter_cont inter_state where
-    step: "A,M,\<Lambda>,\<Gamma>,\<Omega>,T \<turnstile> \<langle>((BigBlock name cs1 None any_tr), KStop, (Normal ns1))\<rangle> \<longrightarrow> (inter_bb, inter_cont, inter_state)" and
-    rest: "A,M,\<Lambda>,\<Gamma>,\<Omega>,T \<turnstile> (inter_bb, inter_cont, inter_state) -n\<longrightarrow>^j' (reached_bb, reached_cont, reached_state)"
-    by (metis prod_cases3 relpowp_Suc_D2) 
-  then show ?thesis 
-  proof (cases any_tr)
-    case None
-    from step this have concrete_inter: "(inter_bb, inter_cont, inter_state) = (BigBlock name [] None None, KStop, inter_state)"
-    proof cases
-      case RedSimpleCmds thus ?thesis using None by (auto simp add: RedSimpleCmds)
-    qed auto
-
-    have Red_impl: "(\<And> s2'.((red_cmd_list A M \<Lambda> \<Gamma> \<Omega> (c#cs2) (Normal ns1) s2') \<Longrightarrow> (s2' \<noteq> Failure)))" 
-      using dag_verifies_propagate_2  assms(5) cfg_is_correct by blast 
-
-    from step have "inter_state \<noteq> Failure"
-    proof cases
-      case RedSimpleCmds thus ?thesis using Red_impl trace_is_possible
-        by (metis assms(4) assms(7) assms(6) block_local_rel_guard_false step syn_rel)
-    qed auto
-
-    hence valid_inter: "(valid_configuration A \<Lambda> \<Gamma> \<Omega> [] inter_bb inter_cont inter_state)" 
-      unfolding valid_configuration_def expr_all_sat_def
-      using concrete_inter get_state.simps is_final.simps by simp
-
-    have "is_final (inter_bb, inter_cont, inter_state)" using concrete_inter by simp 
-    then show ?thesis by (metis Pair_inject concrete_inter final_is_static_propagate relpowp_imp_rtranclp rest valid_inter)
-  next
-    case (Some transfer)
-    then show ?thesis
-    proof (cases transfer)
-      case (Goto x1)
-      then show ?thesis using Some assms(2) by blast
+proof (cases cs2)
+  case Nil
+  hence "cs1 = []" using ast_cfg_rel.cases syn_rel assms(2) by blast 
+  thus ?thesis
+    proof (cases any_tr)
+      case None
+      then have "is_final ((BigBlock name cs1 None any_tr), KStop, (Normal ns1))" using \<open>cs1 = []\<close> by auto 
+      moreover have "(valid_configuration A \<Lambda> \<Gamma> \<Omega> [] (BigBlock name cs1 None any_tr) KStop (Normal ns1))" by (simp add: Ast.valid_configuration_def expr_all_sat_def)
+      ultimately show ?thesis by (metis None \<open>cs1 = []\<close> final_is_static_propagate j_step_ast_trace prod.sel(1) prod.sel(2) relpowp_imp_rtranclp assms(2))
     next
-      case (Return ret)
-      from step this Some have concrete_inter: "(inter_bb, inter_cont, inter_state) = (BigBlock name [] None (Some (Return ret)), KStop, inter_state)"
+      case (Some a)
+      then show ?thesis
+      proof (cases j)
+        case 0
+        from this j_step_ast_trace assms(2) have "(reached_bb, reached_cont, reached_state) = ((BigBlock name cs1 None any_tr), KStop, (Normal ns1))" by simp
+        then show ?thesis by (simp add: valid_configuration_def expr_all_sat_def)
+      next
+        case (Suc j')
+        thus ?thesis 
+        proof (cases a)
+          case (Return x2) 
+          from Suc j_step_ast_trace assms(2) obtain inter_bb inter_cont inter_state where
+            step0: "A,M,\<Lambda>,\<Gamma>,\<Omega>,T \<turnstile> \<langle>((BigBlock name cs1 None any_tr), KStop, (Normal ns1))\<rangle> \<longrightarrow> (inter_bb, inter_cont, inter_state)" and
+            rest0: "A,M,\<Lambda>,\<Gamma>,\<Omega>,T \<turnstile> (inter_bb, inter_cont, inter_state) -n\<longrightarrow>^j' (reached_bb, reached_cont, reached_state)"
+            by (metis prod_cases3 relpowp_Suc_D2) 
+          then have inter_conc: "(inter_bb, inter_cont, inter_state) = ((BigBlock name [] None None), KStop, Normal ns1)" 
+            using \<open>cs1 = []\<close> Return Some
+          proof cases
+            case RedReturn thus ?thesis by blast
+          qed auto
+          then have "is_final (inter_bb, inter_cont, inter_state)" by simp
+          then have "(valid_configuration A \<Lambda> \<Gamma> \<Omega> [] inter_bb inter_cont inter_state)" using inter_conc valid_configuration_def
+            by (metis expr_all_sat_def get_state.simps list.pred_inject(1) state.simps(3))
+          then show ?thesis
+            by (metis \<open>is_final (inter_bb, inter_cont, inter_state)\<close> final_is_static_propagate inter_conc prod.sel(1) prod.sel(2) relpowp_imp_rtranclp rest0)
+        next
+          case (Goto x3)
+          thus ?thesis using assms(3) Some by blast
+      qed
+    qed
+  qed
+next
+  case (Cons)
+  hence "cs1 \<noteq> []" using syn_rel assms(2) ast_cfg_rel.simps by blast
+  thus ?thesis 
+  proof (cases j)
+    case 0
+    from this j_step_ast_trace assms(2) have "(reached_bb, reached_cont, reached_state) = ((BigBlock name cs1 None any_tr), KStop, (Normal ns1))" by simp
+    then show ?thesis by (simp add: valid_configuration_def expr_all_sat_def)
+  next
+    case (Suc j')
+    from this j_step_ast_trace assms(2) obtain inter_bb inter_cont inter_state where
+      step: "A,M,\<Lambda>,\<Gamma>,\<Omega>,T \<turnstile> \<langle>((BigBlock name cs1 None any_tr), KStop, (Normal ns1))\<rangle> \<longrightarrow> (inter_bb, inter_cont, inter_state)" and
+      rest: "A,M,\<Lambda>,\<Gamma>,\<Omega>,T \<turnstile> (inter_bb, inter_cont, inter_state) -n\<longrightarrow>^j' (reached_bb, reached_cont, reached_state)"
+      by (metis prod_cases3 relpowp_Suc_D2) 
+    then show ?thesis 
+    proof (cases any_tr)
+      case None
+      from step this have concrete_inter: "(inter_bb, inter_cont, inter_state) = (BigBlock name [] None None, KStop, inter_state)"
       proof cases
-        case RedSimpleCmds thus ?thesis using Return Some by blast
-      qed (auto simp add: assms(3))
+        case RedSimpleCmds thus ?thesis using None by (auto simp add: RedSimpleCmds)
+      qed auto
   
       have Red_impl: "(\<And> s2'.((red_cmd_list A M \<Lambda> \<Gamma> \<Omega> (c#cs2) (Normal ns1) s2') \<Longrightarrow> (s2' \<noteq> Failure)))" 
-        using dag_verifies_propagate_2  assms(5) cfg_is_correct by blast 
+        using dag_verifies_propagate_2 assms cfg_is_correct by blast 
   
       from step have "inter_state \<noteq> Failure"
       proof cases
         case RedSimpleCmds thus ?thesis using Red_impl trace_is_possible
-          by (metis assms(4) assms(7) assms(6) block_local_rel_guard_false step syn_rel)
+          by (metis assms(5-7) assms(2) block_local_rel_guard_false local.Cons local.step neq_Nil_conv syn_rel)
       qed auto
-      then show ?thesis 
-      proof (cases inter_state)
-        case (Normal x1)
-        then show ?thesis
-        proof (cases j')
-          case 0
-          then show ?thesis using concrete_inter by (metis Ast.valid_configuration_def \<open>inter_state \<noteq> Failure\<close> get_state.simps is_final.simps(4) relpowp_0_E rest)
-        next
-          case (Suc j'')
-          from this rest obtain inter_bb2 inter_cont2 inter_state2 where
-            snd_step: "A,M,\<Lambda>,\<Gamma>,\<Omega>,T \<turnstile> \<langle>(inter_bb, inter_cont, inter_state)\<rangle> \<longrightarrow> (inter_bb2, inter_cont2, inter_state2)" and
-            snd_rest: "A,M,\<Lambda>,\<Gamma>,\<Omega>,T \<turnstile> (inter_bb2, inter_cont2, inter_state2) -n\<longrightarrow>^j'' (reached_bb, reached_cont, reached_state)"
-            by (metis get_state.cases relpowp_Suc_E2)
-          then have inter2_conc: "(inter_bb2, inter_cont2, inter_state2) = ((BigBlock name [] None None), KStop, inter_state)" 
-            using concrete_inter \<open>inter_state \<noteq> Failure\<close> Normal
-          proof cases
-            case RedReturn thus ?thesis using concrete_inter \<open>inter_state \<noteq> Failure\<close> Normal by blast
-          qed auto
-          hence "is_final (inter_bb2, inter_cont2, inter_state2)" by simp
+  
+      hence valid_inter: "(valid_configuration A \<Lambda> \<Gamma> \<Omega> [] inter_bb inter_cont inter_state)" 
+        unfolding valid_configuration_def expr_all_sat_def
+        using concrete_inter get_state.simps is_final.simps by simp
+  
+      have "is_final (inter_bb, inter_cont, inter_state)" using concrete_inter by simp 
+      then show ?thesis by (metis Pair_inject concrete_inter final_is_static_propagate relpowp_imp_rtranclp rest valid_inter)
+    next
+      case (Some transfer)
+      then show ?thesis
+      proof (cases transfer)
+        case (Goto x1)
+        then show ?thesis using Some assms(3) by blast
+      next
+        case (Return ret)
+        from step this Some have concrete_inter: "(inter_bb, inter_cont, inter_state) = (BigBlock name [] None (Some (Return ret)), KStop, inter_state)"
+        proof cases
+          case RedSimpleCmds thus ?thesis using Return Some by blast
+        qed (auto simp add: Cons \<open>cs1 \<noteq> []\<close>)
+    
+        have Red_impl: "(\<And> s2'.((red_cmd_list A M \<Lambda> \<Gamma> \<Omega> (c#cs2) (Normal ns1) s2') \<Longrightarrow> (s2' \<noteq> Failure)))" 
+          using dag_verifies_propagate_2 assms cfg_is_correct by blast 
+    
+        from step have "inter_state \<noteq> Failure"
+        proof cases
+          case RedSimpleCmds thus ?thesis using Red_impl trace_is_possible
+            by (metis assms(1-2) assms(5-8) block_local_rel_guard_false local.Cons local.step neq_Nil_conv syn_rel)
+        qed auto
+        then show ?thesis 
+        proof (cases inter_state)
+          case (Normal x1)
           then show ?thesis
-            by (metis Ast.valid_configuration_def inter2_conc \<open>inter_state \<noteq> Failure\<close> expr_all_sat_def final_is_static_propagate get_state.simps list.pred_inject(1) rtranclp_power snd_rest)
+          proof (cases j')
+            case 0
+            then show ?thesis using concrete_inter by (metis Ast.valid_configuration_def \<open>inter_state \<noteq> Failure\<close> get_state.simps is_final.simps(4) relpowp_0_E rest)
+          next
+            case (Suc j'')
+            from this rest obtain inter_bb2 inter_cont2 inter_state2 where
+              snd_step: "A,M,\<Lambda>,\<Gamma>,\<Omega>,T \<turnstile> \<langle>(inter_bb, inter_cont, inter_state)\<rangle> \<longrightarrow> (inter_bb2, inter_cont2, inter_state2)" and
+              snd_rest: "A,M,\<Lambda>,\<Gamma>,\<Omega>,T \<turnstile> (inter_bb2, inter_cont2, inter_state2) -n\<longrightarrow>^j'' (reached_bb, reached_cont, reached_state)"
+              by (metis get_state.cases relpowp_Suc_E2)
+            then have inter2_conc: "(inter_bb2, inter_cont2, inter_state2) = ((BigBlock name [] None None), KStop, inter_state)" 
+              using concrete_inter \<open>inter_state \<noteq> Failure\<close> Normal
+            proof cases
+              case RedReturn thus ?thesis using concrete_inter \<open>inter_state \<noteq> Failure\<close> Normal by blast
+            qed auto
+            hence "is_final (inter_bb2, inter_cont2, inter_state2)" by simp
+            then show ?thesis
+              by (metis Ast.valid_configuration_def inter2_conc \<open>inter_state \<noteq> Failure\<close> expr_all_sat_def final_is_static_propagate get_state.simps list.pred_inject(1) rtranclp_power snd_rest)
+          qed
+        next
+          case Failure
+          then show ?thesis using \<open>inter_state \<noteq> Failure\<close> by simp
+        next
+          case Magic
+          then show ?thesis by (metis Ast.valid_configuration_def \<open>inter_state \<noteq> Failure\<close> get_state.simps magic_propagates rest state.simps(5))
         qed
-      next
-        case Failure
-        then show ?thesis using \<open>inter_state \<noteq> Failure\<close> by simp
-      next
-        case Magic
-        then show ?thesis by (metis Ast.valid_configuration_def \<open>inter_state \<noteq> Failure\<close> get_state.simps magic_propagates rest state.simps(5))
       qed
     qed
   qed
@@ -557,96 +854,141 @@ qed
 
 text \<open>Global lemma for an ast-bigblock with a non-empty set of simple commands which concludes the program.\<close>
 lemma generic_ending_block_global_rel:
-  assumes syn_rel: "ast_cfg_rel None [] (BigBlock name cs1 None any_tr) cs2"
-  and j_step_ast_trace: "A,M,\<Lambda>,\<Gamma>,\<Omega>,T \<turnstile> ((BigBlock name cs1 None any_tr), KStop, (Normal ns1)) -n\<longrightarrow>^j (reached_bb, reached_cont, reached_state)"
+  assumes syn_rel: "ast_cfg_rel None [] bb cs2"
+  and j_step_ast_trace: "A,M,\<Lambda>,\<Gamma>,\<Omega>,T \<turnstile> (bb, KStop, (Normal ns1)) -n\<longrightarrow>^j (reached_bb, reached_cont, reached_state)"
+  and "bb = (BigBlock name cs1 None any_tr)"
   and "(any_tr = None) \<or> (any_tr = (Some (Return val1)))"
-  and "cs1 \<noteq> Nil"
-  and "cs2 \<noteq> Nil"
   and "node_to_block G ! n = cs2"
   and cfg_is_correct: "\<And> m' s'. (red_cfg_multi A M \<Lambda> \<Gamma> \<Omega> G ((Inl n),(Normal ns1)) (m',s')) \<Longrightarrow> (s' \<noteq> Failure)" 
 shows "(valid_configuration A \<Lambda> \<Gamma> \<Omega> [] reached_bb reached_cont reached_state)"
   using assms
-proof (cases j)
-  case 0
-  from this j_step_ast_trace have "(reached_bb, reached_cont, reached_state) = ((BigBlock name cs1 None any_tr), KStop, (Normal ns1))" by simp
-  then show ?thesis by (simp add: valid_configuration_def expr_all_sat_def)
-next
-  case (Suc j')
-  from this j_step_ast_trace obtain inter_bb inter_cont inter_state where
-    step: "A,M,\<Lambda>,\<Gamma>,\<Omega>,T \<turnstile> \<langle>((BigBlock name cs1 None any_tr), KStop, (Normal ns1))\<rangle> \<longrightarrow> (inter_bb, inter_cont, inter_state)" and
-    rest: "A,M,\<Lambda>,\<Gamma>,\<Omega>,T \<turnstile> (inter_bb, inter_cont, inter_state) -n\<longrightarrow>^j' (reached_bb, reached_cont, reached_state)"
-    by (metis prod_cases3 relpowp_Suc_D2) 
-  then show ?thesis 
-  proof (cases any_tr)
-    case None
-    from step this have concrete_inter: "(inter_bb, inter_cont, inter_state) = (BigBlock name [] None None, KStop, inter_state)"
-    proof cases
-      case RedSimpleCmds thus ?thesis using None by (auto simp add: RedSimpleCmds)
-    qed auto
-
-    have Red_impl: "(\<And> s2'.((red_cmd_list A M \<Lambda> \<Gamma> \<Omega> cs2 (Normal ns1) s2') \<Longrightarrow> (s2' \<noteq> Failure)))"
-      using assms(6) cfg_is_correct dag_verifies_propagate_2 by blast
-
-    from step have "inter_state \<noteq> Failure"
-    proof cases
-      case RedSimpleCmds thus ?thesis using Red_impl assms(5) block_local_rel_generic local.step syn_rel by blast
-    qed auto
-
-    hence valid_inter: "(valid_configuration A \<Lambda> \<Gamma> \<Omega> [] inter_bb inter_cont inter_state)" 
-      unfolding valid_configuration_def expr_all_sat_def
-      using concrete_inter get_state.simps is_final.simps by simp
-
-    have "is_final (inter_bb, inter_cont, inter_state)" using concrete_inter by simp 
-    then show ?thesis by (metis Pair_inject concrete_inter final_is_static_propagate relpowp_imp_rtranclp rest valid_inter)
-  next
-    case (Some transfer)
-    then show ?thesis
-    proof (cases transfer)
-      case (Goto x1)
-      then show ?thesis using Some assms(3) by blast
+proof (cases cs2)
+  case Nil 
+  hence "cs1 = []" using ast_cfg_rel.cases syn_rel assms(3) by blast 
+  thus ?thesis
+    proof (cases any_tr)
+      case None
+      then have "is_final ((BigBlock name cs1 None any_tr), KStop, (Normal ns1))" using \<open>cs1 = []\<close> by auto 
+      moreover have "(valid_configuration A \<Lambda> \<Gamma> \<Omega> [] (BigBlock name cs1 None any_tr) KStop (Normal ns1))" by (simp add: Ast.valid_configuration_def expr_all_sat_def)
+      ultimately show ?thesis by (metis assms(3) None \<open>cs1 = []\<close> final_is_static_propagate j_step_ast_trace prod.sel(1) prod.sel(2) relpowp_imp_rtranclp)
     next
-      case (Return ret)
-      from step this Some have concrete_inter: "(inter_bb, inter_cont, inter_state) = (BigBlock name [] None (Some (Return ret)), KStop, inter_state)"
+      case (Some a)
+      then show ?thesis
+      proof (cases j)
+        case 0
+        from this j_step_ast_trace assms(3) have "(reached_bb, reached_cont, reached_state) = ((BigBlock name cs1 None any_tr), KStop, (Normal ns1))" by simp
+        then show ?thesis by (simp add: valid_configuration_def expr_all_sat_def)
+      next
+        case (Suc j')
+        thus ?thesis 
+        proof (cases a)
+          case (Return x2) 
+          from Suc j_step_ast_trace assms(3) obtain inter_bb inter_cont inter_state where
+            step0: "A,M,\<Lambda>,\<Gamma>,\<Omega>,T \<turnstile> \<langle>((BigBlock name cs1 None any_tr), KStop, (Normal ns1))\<rangle> \<longrightarrow> (inter_bb, inter_cont, inter_state)" and
+            rest0: "A,M,\<Lambda>,\<Gamma>,\<Omega>,T \<turnstile> (inter_bb, inter_cont, inter_state) -n\<longrightarrow>^j' (reached_bb, reached_cont, reached_state)"
+            by (metis prod_cases3 relpowp_Suc_D2) 
+          then have inter_conc: "(inter_bb, inter_cont, inter_state) = ((BigBlock name [] None None), KStop, Normal ns1)" 
+            using \<open>cs1 = []\<close> Return Some
+          proof cases
+            case RedReturn thus ?thesis by blast
+          qed auto
+          then have "is_final (inter_bb, inter_cont, inter_state)" by simp
+          then have "(valid_configuration A \<Lambda> \<Gamma> \<Omega> [] inter_bb inter_cont inter_state)" using inter_conc valid_configuration_def
+            by (metis expr_all_sat_def get_state.simps list.pred_inject(1) state.simps(3))
+          then show ?thesis
+            by (metis \<open>is_final (inter_bb, inter_cont, inter_state)\<close> final_is_static_propagate inter_conc prod.sel(1) prod.sel(2) relpowp_imp_rtranclp rest0)
+        next
+          case (Goto x3)
+          thus ?thesis using assms(4) Some by blast
+      qed
+    qed
+  qed
+next
+  case (Cons) 
+  hence "cs1 \<noteq> []" using ast_cfg_rel.simps syn_rel assms(3) by blast
+  thus ?thesis
+  proof (cases j)
+    case 0
+    from this j_step_ast_trace assms(3) have "(reached_bb, reached_cont, reached_state) = ((BigBlock name cs1 None any_tr), KStop, (Normal ns1))" by simp
+    then show ?thesis by (simp add: valid_configuration_def expr_all_sat_def)
+  next
+    case (Suc j')
+    from this j_step_ast_trace assms(3) obtain inter_bb inter_cont inter_state where
+      step: "A,M,\<Lambda>,\<Gamma>,\<Omega>,T \<turnstile> \<langle>((BigBlock name cs1 None any_tr), KStop, (Normal ns1))\<rangle> \<longrightarrow> (inter_bb, inter_cont, inter_state)" and
+      rest: "A,M,\<Lambda>,\<Gamma>,\<Omega>,T \<turnstile> (inter_bb, inter_cont, inter_state) -n\<longrightarrow>^j' (reached_bb, reached_cont, reached_state)"
+      by (metis prod_cases3 relpowp_Suc_D2) 
+    then show ?thesis 
+    proof (cases any_tr)
+      case None
+      from step this have concrete_inter: "(inter_bb, inter_cont, inter_state) = (BigBlock name [] None None, KStop, inter_state)"
       proof cases
-        case RedSimpleCmds thus ?thesis using Return Some by blast
-      qed (auto simp add: assms(4))
+        case RedSimpleCmds thus ?thesis using None by (auto simp add: RedSimpleCmds)
+      qed auto
   
-      have Red_impl: "(\<And> s2'.((red_cmd_list A M \<Lambda> \<Gamma> \<Omega> cs2 (Normal ns1) s2') \<Longrightarrow> (s2' \<noteq> Failure)))" 
-        using dag_verifies_propagate_2  assms(6) cfg_is_correct by blast 
+      have Red_impl: "(\<And> s2'.((red_cmd_list A M \<Lambda> \<Gamma> \<Omega> cs2 (Normal ns1) s2') \<Longrightarrow> (s2' \<noteq> Failure)))"
+        using assms(5) cfg_is_correct dag_verifies_propagate_2 by blast
   
       from step have "inter_state \<noteq> Failure"
       proof cases
-        case RedSimpleCmds thus ?thesis using Red_impl using assms(5) block_local_rel_generic local.step syn_rel by blast
+        case RedSimpleCmds thus ?thesis using Red_impl block_local_rel_generic local.Cons local.step syn_rel assms(3) by blast
       qed auto
-
+  
+      hence valid_inter: "(valid_configuration A \<Lambda> \<Gamma> \<Omega> [] inter_bb inter_cont inter_state)" 
+        unfolding valid_configuration_def expr_all_sat_def
+        using concrete_inter get_state.simps is_final.simps by simp
+  
+      have "is_final (inter_bb, inter_cont, inter_state)" using concrete_inter by simp 
+      then show ?thesis by (metis Pair_inject concrete_inter final_is_static_propagate relpowp_imp_rtranclp rest valid_inter)
+    next
+      case (Some transfer)
       then show ?thesis
-      proof (cases inter_state)
-        case (Normal x1)
+      proof (cases transfer)
+        case (Goto x1)
+        then show ?thesis using Some assms(4) by blast
+      next
+        case (Return ret)
+        from step this Some have concrete_inter: "(inter_bb, inter_cont, inter_state) = (BigBlock name [] None (Some (Return ret)), KStop, inter_state)"
+        proof cases
+          case RedSimpleCmds thus ?thesis using Return Some by blast
+        qed (auto simp add: \<open>cs1 \<noteq> []\<close>)
+    
+        have Red_impl: "(\<And> s2'.((red_cmd_list A M \<Lambda> \<Gamma> \<Omega> cs2 (Normal ns1) s2') \<Longrightarrow> (s2' \<noteq> Failure)))" 
+          using dag_verifies_propagate_2  assms(5) cfg_is_correct by blast 
+    
+        from step have "inter_state \<noteq> Failure"
+        proof cases
+          case RedSimpleCmds thus ?thesis using Red_impl block_local_rel_generic local.Cons local.step syn_rel assms(3) by blast
+        qed auto
+  
         then show ?thesis
-        proof (cases j')
-          case 0
-          then show ?thesis using concrete_inter by (metis Ast.valid_configuration_def \<open>inter_state \<noteq> Failure\<close> get_state.simps is_final.simps(4) relpowp_0_E rest)
-        next
-          case (Suc j'')
-          from this rest obtain inter_bb2 inter_cont2 inter_state2 where
-            snd_step: "A,M,\<Lambda>,\<Gamma>,\<Omega>,T \<turnstile> \<langle>(inter_bb, inter_cont, inter_state)\<rangle> \<longrightarrow> (inter_bb2, inter_cont2, inter_state2)" and
-            snd_rest: "A,M,\<Lambda>,\<Gamma>,\<Omega>,T \<turnstile> (inter_bb2, inter_cont2, inter_state2) -n\<longrightarrow>^j'' (reached_bb, reached_cont, reached_state)"
-            by (metis get_state.cases relpowp_Suc_E2)
-          then have inter2_conc: "(inter_bb2, inter_cont2, inter_state2) = ((BigBlock name [] None None), KStop, inter_state)" 
-            using concrete_inter \<open>inter_state \<noteq> Failure\<close> Normal
-          proof cases
-            case RedReturn thus ?thesis using concrete_inter \<open>inter_state \<noteq> Failure\<close> Normal by blast
-          qed auto
-          hence "is_final (inter_bb2, inter_cont2, inter_state2)" by simp
+        proof (cases inter_state)
+          case (Normal x1)
           then show ?thesis
-            by (metis Ast.valid_configuration_def inter2_conc \<open>inter_state \<noteq> Failure\<close> expr_all_sat_def final_is_static_propagate get_state.simps list.pred_inject(1) rtranclp_power snd_rest)
+          proof (cases j')
+            case 0
+            then show ?thesis using concrete_inter by (metis Ast.valid_configuration_def \<open>inter_state \<noteq> Failure\<close> get_state.simps is_final.simps(4) relpowp_0_E rest)
+          next
+            case (Suc j'')
+            from this rest obtain inter_bb2 inter_cont2 inter_state2 where
+              snd_step: "A,M,\<Lambda>,\<Gamma>,\<Omega>,T \<turnstile> \<langle>(inter_bb, inter_cont, inter_state)\<rangle> \<longrightarrow> (inter_bb2, inter_cont2, inter_state2)" and
+              snd_rest: "A,M,\<Lambda>,\<Gamma>,\<Omega>,T \<turnstile> (inter_bb2, inter_cont2, inter_state2) -n\<longrightarrow>^j'' (reached_bb, reached_cont, reached_state)"
+              by (metis get_state.cases relpowp_Suc_E2)
+            then have inter2_conc: "(inter_bb2, inter_cont2, inter_state2) = ((BigBlock name [] None None), KStop, inter_state)" 
+              using concrete_inter \<open>inter_state \<noteq> Failure\<close> Normal
+            proof cases
+              case RedReturn thus ?thesis using concrete_inter \<open>inter_state \<noteq> Failure\<close> Normal by blast
+            qed auto
+            hence "is_final (inter_bb2, inter_cont2, inter_state2)" by simp
+            then show ?thesis
+              by (metis Ast.valid_configuration_def inter2_conc \<open>inter_state \<noteq> Failure\<close> expr_all_sat_def final_is_static_propagate get_state.simps list.pred_inject(1) rtranclp_power snd_rest)
+          qed
+        next
+          case Failure
+          then show ?thesis using \<open>inter_state \<noteq> Failure\<close> by simp
+        next
+          case Magic
+          then show ?thesis by (metis valid_configuration_def \<open>inter_state \<noteq> Failure\<close> get_state.simps magic_propagates rest state.simps(5))
         qed
-      next
-        case Failure
-        then show ?thesis using \<open>inter_state \<noteq> Failure\<close> by simp
-      next
-        case Magic
-        then show ?thesis by (metis valid_configuration_def \<open>inter_state \<noteq> Failure\<close> get_state.simps magic_propagates rest state.simps(5))
       qed
     qed
   qed
@@ -654,37 +996,77 @@ qed
 
 
 text \<open>Global lemma for an ast-bigblock with a non-empty set of simple commands that enters a loop after it executes its simple cmds.\<close>
+
+(*
+lemma inner_loop_head_global_rel_wrapped:
+  assumes j_step_ast_trace: 
+          "A,M,\<Lambda>1_local,\<Gamma>,\<Omega>,T \<turnstile> (BigBlock None [] (Some (WhileWrapper loop)) None, cont0, Normal ns1) -n\<longrightarrow>^j 
+                                 (reached_bb, reached_cont, reached_state)"
+  and cfg_is_correct: "\<And> m' s'. (red_cfg_multi A M \<Lambda>1_local \<Gamma> \<Omega> G ((Inl n),(Normal ns1)) (m',s')) \<Longrightarrow> (s' \<noteq> Failure)"
+  and loop_ih:
+        "\<And>k ns1'. k < j \<Longrightarrow>
+        (A,M,\<Lambda>1_local,\<Gamma>,\<Omega>,T \<turnstile>(bb0_unwrapped, KEndBlock KStop, Normal ns1') -n\<longrightarrow>^k (reached_bb, reached_cont, reached_state)) \<Longrightarrow>
+        (\<And> m' s'. (red_cfg_multi A M \<Lambda>1_local \<Gamma> \<Omega> nested_loop_before_cfg_to_dag_prog.proc_body ((Inl 1),(Normal ns1')) (m',s')) \<Longrightarrow> (s' \<noteq> Failure)) \<Longrightarrow>
+        (Ast.valid_configuration A \<Lambda>1_local \<Gamma> \<Omega> [] reached_bb reached_cont reached_state)" 
+  shows "(Ast.valid_configuration A \<Lambda>1_local \<Gamma> \<Omega> [] reached_bb reached_cont reached_state)"
+  using assms
+proof (cases j)
+  case 0
+  from this j_step_ast_trace have 
+    "(reached_bb, reached_cont, reached_state) = (outer_body_bb1, (KSeq outer_body_bb2 (KSeq bb0_unwrapped (KEndBlock KStop))), Normal ns1)" by auto
+  then show ?thesis by (simp add: Ast.valid_configuration_def)
+next
+  case (Suc j')
+  from assms this obtain inter_bb inter_cont inter_state where
+    step: "A,M,\<Lambda>1_local,\<Gamma>,\<Omega>,T \<turnstile> \<langle>(outer_body_bb1, (KSeq outer_body_bb2 (KSeq bb0_unwrapped (KEndBlock KStop))), Normal ns1)\<rangle> \<longrightarrow> (inter_bb, inter_cont, inter_state)" and
+    rest: "A,M,\<Lambda>1_local,\<Gamma>,\<Omega>,T \<turnstile>(inter_bb, inter_cont, inter_state) -n\<longrightarrow>^j' (reached_bb, reached_cont, reached_state)" 
+    by (metis (no_types, opaque_lifting) get_state.cases relpowp_Suc_D2)
+  hence "(inter_bb, inter_cont, inter_state) = (outer_body_bb1_unwrapped, KEndBlock (KSeq outer_body_bb2 (KSeq bb0_unwrapped (KEndBlock KStop))), Normal ns1)"
+    unfolding outer_body_bb1_unwrapped_def outer_body_bb1_def
+    by (cases) auto
+  hence rest_conc: "A,M,\<Lambda>1_local,\<Gamma>,\<Omega>,T \<turnstile> (outer_body_bb1_unwrapped, KEndBlock (KSeq outer_body_bb2 (KSeq bb0_unwrapped (KEndBlock KStop))), Normal ns1) -n\<longrightarrow>^j' (reached_bb, reached_cont, reached_state)" 
+    using rest by simp
+  show ?thesis 
+    apply (rule inner_loop_head_global_rel)
+      apply (rule rest_conc)
+     apply (rule cfg_is_correct)
+     apply simp
+    using Suc less_SucI loop_ih by blast
+qed
+*)
+
 lemma block_global_rel_while_successor:
   assumes j_step_ast_trace: 
-      "A,M,\<Lambda>,\<Gamma>,\<Omega>,T \<turnstile> ((BigBlock name cmds (Some (WhileWrapper (ParsedWhile guard invs (body_bb0#body_bbs)))) None), cont1, Normal ns1) -n\<longrightarrow>^j 
+      "A,M,\<Lambda>,\<Gamma>,\<Omega>,T \<turnstile> (bb, cont1, Normal ns1) -n\<longrightarrow>^j 
                       (reached_bb, reached_cont, reached_state)"
-  and syn_rel: "ast_cfg_rel None [] (BigBlock name cmds (Some (WhileWrapper (ParsedWhile guard invs (body_bb0#body_bbs)))) None) cmds"
+  and syn_rel: "ast_cfg_rel None [] bb cmds"
+  and "bb = (BigBlock name cmds (Some (WhileWrapper (ParsedWhile guard invs (body_bb0#body_bbs)))) None)"
   and "cmds \<noteq> []"
   and "node_to_block G ! n = cmds"
   and cfg_is_correct: "\<And> m' s'. (red_cfg_multi A M \<Lambda> \<Gamma> \<Omega> G ((Inl n),(Normal ns1)) (m',s')) \<Longrightarrow> (s' \<noteq> Failure)"
   and block_local_rel:
     "\<And> reached_bb_inter reached_cont_inter reached_state_inter. 
-    (red_bigblock A M \<Lambda> \<Gamma> \<Omega> T ((BigBlock name cmds (Some (WhileWrapper (ParsedWhile guard invs (body_bb0#body_bbs)))) None), cont1, (Normal ns1)) (reached_bb_inter, reached_cont_inter, reached_state_inter)) \<Longrightarrow> 
+    (red_bigblock A M \<Lambda> \<Gamma> \<Omega> T (bb, cont1, (Normal ns1)) (reached_bb_inter, reached_cont_inter, reached_state_inter)) \<Longrightarrow> 
     (\<And> s2'.((red_cmd_list A M \<Lambda> \<Gamma> \<Omega> cmds (Normal ns1) s2') \<Longrightarrow> (s2' \<noteq> Failure))) \<Longrightarrow>   
-    (reached_state_inter \<noteq> Failure  \<and> (\<forall>ns1'. reached_state_inter = Normal ns1' \<longrightarrow> (A,M,\<Lambda>,\<Gamma>,\<Omega> \<turnstile> \<langle>cmds, Normal ns1\<rangle> [\<rightarrow>] Normal ns1')))"
+    (reached_state_inter \<noteq> Failure  \<and> (\<forall>ns1'. reached_state_inter = Normal ns1' \<longrightarrow> (A,M,\<Lambda>,\<Gamma>,\<Omega> \<turnstile> \<langle>(node_to_block G ! n), Normal ns1\<rangle> [\<rightarrow>] Normal ns1')))"
   and global_rel_succ:
         "\<And> ns2 k.
          k < j \<Longrightarrow>
          (\<forall>msuc2. List.member (out_edges(G) ! n) msuc2 \<longrightarrow> (\<forall>m3 s3. (A,M,\<Lambda>,\<Gamma>,\<Omega>,G \<turnstile> (Inl msuc2, Normal ns2) -n\<rightarrow>* (m3, s3)) \<longrightarrow> s3 \<noteq> Failure)) \<Longrightarrow>
          A,M,\<Lambda>,\<Gamma>,\<Omega>,T \<turnstile> ((BigBlock name [] (Some (ParsedWhile guard invs (body_bb0#body_bbs))) None), KEndBlock cont1, Normal ns2) -n\<longrightarrow>^k 
                       (reached_bb, reached_cont, reached_state) \<Longrightarrow> 
-         (valid_configuration A \<Lambda> \<Gamma> \<Omega> [] reached_bb reached_cont reached_state)"
-  shows "(valid_configuration A \<Lambda> \<Gamma> \<Omega> [] reached_bb reached_cont reached_state)"
+         (valid_configuration A \<Lambda> \<Gamma> \<Omega> posts reached_bb reached_cont reached_state)"
+  shows "(valid_configuration A \<Lambda> \<Gamma> \<Omega> posts reached_bb reached_cont reached_state)"
   using assms
 proof cases
   assume "j = 0"
   then have "(reached_bb, reached_cont, reached_state) = 
-             ((BigBlock name cmds (Some (WhileWrapper (ParsedWhile guard invs (body_bb0#body_bbs)))) None), cont1, Normal ns1)" using j_step_ast_trace by auto
+             ((BigBlock name cmds (Some (WhileWrapper (ParsedWhile guard invs (body_bb0#body_bbs)))) None), cont1, Normal ns1)" using j_step_ast_trace assms(3) by auto
   thus ?thesis by (simp add: valid_configuration_def)
 next
   assume "j \<noteq> 0"
   from this obtain j' where "j = Suc j'" using not0_implies_Suc by blast
-  from this j_step_ast_trace obtain inter_bb inter_cont inter_state where
+  from this j_step_ast_trace assms(3) obtain inter_bb inter_cont inter_state where
     first_step: "A,M,\<Lambda>,\<Gamma>,\<Omega>,T \<turnstile> \<langle>((BigBlock name cmds (Some (WhileWrapper (ParsedWhile guard invs (body_bb0#body_bbs)))) None), cont1, Normal ns1)\<rangle> \<longrightarrow> (inter_bb, inter_cont, inter_state)" and 
     rest: "A,M,\<Lambda>,\<Gamma>,\<Omega>,T \<turnstile> (inter_bb, inter_cont, inter_state) -n\<longrightarrow>^j' (reached_bb, reached_cont, reached_state)"
     by (metis (no_types, opaque_lifting) get_state.cases relpowp_Suc_D2)
@@ -692,9 +1074,9 @@ next
   proof cases
     case RedSimpleCmds thus ?thesis by blast
   qed (auto simp add: \<open>cmds \<noteq> []\<close>)
-  have Red_impl: "(\<And> s2'.((red_cmd_list A M \<Lambda> \<Gamma> \<Omega> cmds (Normal ns1) s2') \<Longrightarrow> (s2' \<noteq> Failure)))" using dag_verifies_propagate_2 cfg_is_correct assms(4) by blast
+  have Red_impl: "(\<And> s2'.((red_cmd_list A M \<Lambda> \<Gamma> \<Omega> cmds (Normal ns1) s2') \<Longrightarrow> (s2' \<noteq> Failure)))" using dag_verifies_propagate_2 cfg_is_correct assms(5) by blast
   have local_conclusion: "inter_state \<noteq> Failure  \<and> (\<forall>ns1'. inter_state = Normal ns1' \<longrightarrow> (A,M,\<Lambda>,\<Gamma>,\<Omega> \<turnstile> \<langle>cmds, Normal ns1\<rangle> [\<rightarrow>] Normal ns1'))" 
-    using Red_impl first_step assms(3) block_local_rel_generic syn_rel by blast 
+    using Red_impl first_step assms(3-4) block_local_rel_generic syn_rel by metis
   show ?thesis 
   proof (cases inter_state)
     case (Normal x1)
@@ -703,16 +1085,15 @@ next
     proof (cases j')
       case 0
       then show ?thesis 
-        by (metis (full_types, opaque_lifting) Ast.valid_configuration_def expr_all_sat_def get_state.simps list.pred_inject(1) local_conclusion relpowp.simps(1) rest)
+        by (metis Normal a1 nat.discI rest wrapper_to_endblock)
     next
       case 2: (Suc j'')
 
       hence Red_cfg_conc: 
         "(\<forall>msuc2. List.member (out_edges(G) ! n) msuc2 \<longrightarrow> (\<forall>m3 s3. (A,M,\<Lambda>,\<Gamma>,\<Omega>,G \<turnstile> (Inl msuc2, inter_state) -n\<rightarrow>* (m3, s3)) \<longrightarrow> s3 \<noteq> Failure))" 
-        using dag_verifies_propagate Normal \<open>A,M,\<Lambda>,\<Gamma>,\<Omega> \<turnstile> \<langle>cmds,Normal ns1\<rangle> [\<rightarrow>] inter_state\<close> assms(4) cfg_is_correct 
-        by blast
+        using dag_verifies_propagate Normal \<open>A,M,\<Lambda>,\<Gamma>,\<Omega> \<turnstile> \<langle>cmds,Normal ns1\<rangle> [\<rightarrow>] inter_state\<close> assms(5) cfg_is_correct by blast
 
-      from 2 j_step_ast_trace obtain inter_bb2 inter_cont2 inter_state2 where
+      from 2 j_step_ast_trace assms(3) obtain inter_bb2 inter_cont2 inter_state2 where
         first_step_2: "A,M,\<Lambda>,\<Gamma>,\<Omega>,T \<turnstile> \<langle>(inter_bb, inter_cont, inter_state)\<rangle> \<longrightarrow> (inter_bb2, inter_cont2, inter_state2)" and 
         rest_2: "A,M,\<Lambda>,\<Gamma>,\<Omega>,T \<turnstile> (inter_bb2, inter_cont2, inter_state2) -n\<longrightarrow>^j'' (reached_bb, reached_cont, reached_state)"
         by (metis get_state.cases relpowp_Suc_E2 rest)
@@ -724,7 +1105,7 @@ next
       qed auto 
 
       have "j'' < j" by (simp add: "2" \<open>j = Suc j'\<close>)
-      then show ?thesis using a3 rest_2 Normal Red_cfg_conc assms(7) by blast
+      then show ?thesis using a3 rest_2 Normal Red_cfg_conc assms(8) by blast 
     qed
   next
     case Failure
@@ -735,19 +1116,41 @@ next
   qed
 qed
 
+lemma ending_directly_after_loop_exit:
+  assumes "A,M,\<Lambda>,\<Gamma>,\<Omega>,T \<turnstile> (bb, KEndBlock KStop, (Normal ns1'')) -n\<longrightarrow>^j (reached_bb, reached_cont, reached_state)"
+      and "bb = (BigBlock name [] None None)"
+  shows "(Ast.valid_configuration A \<Lambda> \<Gamma> \<Omega> [] reached_bb reached_cont reached_state)"
+  using assms
+proof (cases j)
+  case 0
+  hence "(reached_bb, reached_cont, reached_state) = ((BigBlock name [] None None), KEndBlock KStop, (Normal ns1''))" using assms by auto
+  then show ?thesis by (simp add: Ast.valid_configuration_def)
+next
+  case (Suc j')
+  from assms(1-2) obtain inter_bb inter_cont inter_state where
+    step: "A,M,\<Lambda>,\<Gamma>,\<Omega>,T \<turnstile> \<langle>((BigBlock name [] None None), KEndBlock KStop, (Normal ns1''))\<rangle> \<longrightarrow> (inter_bb, inter_cont, inter_state)" and
+    rest: "A,M,\<Lambda>,\<Gamma>,\<Omega>,T \<turnstile> (inter_bb, inter_cont, inter_state) -n\<longrightarrow>^j' (reached_bb, reached_cont, reached_state)"
+    by (metis (full_types) Suc prod_cases3 relpowp_Suc_E2)
+  hence conc_inter: "(inter_bb, inter_cont, inter_state) = ((BigBlock name [] None None), KStop, (Normal ns1''))" 
+    by (cases) auto
+  hence "is_final (inter_bb, inter_cont, inter_state)" by simp 
+  moreover have "(Ast.valid_configuration A \<Lambda> \<Gamma> \<Omega> [] inter_bb inter_cont inter_state)" 
+    using valid_configuration_def conc_inter by (metis expr_all_sat_def get_state.simps list.pred_inject(1) state.simps(3))  
+  ultimately show ?thesis using rest by (metis conc_inter final_is_static_propagate prod.sel(1) prod.sel(2) relpowp_imp_rtranclp)
+qed
+
 text \<open>Global lemma for a loop-head ast-bigblock with non-empty invariants. The loop is also required to be non-empty.\<close>
 lemma block_global_rel_loop_head:
-  assumes block_rel: "ast_cfg_rel None assertions (BigBlock name [] any_str any_tr) assertions"
-  and ast_trace: "A,M,\<Lambda>,\<Gamma>,\<Omega>,T \<turnstile> ((BigBlock name [] any_str any_tr), KEndBlock cont1, (Normal ns1)) -n\<longrightarrow>^j (reached_bb, reached_cont, reached_state)"
+  assumes block_rel: "ast_cfg_rel None assertions bb assertions"
+  and ast_trace: "A,M,\<Lambda>,\<Gamma>,\<Omega>,T \<turnstile> (bb, KEndBlock cont1, (Normal ns1)) -n\<longrightarrow>^j (reached_bb, reached_cont, reached_state)"
   and cfg_correct: "(\<And> m2 s2. ((red_cfg_multi A M \<Lambda> \<Gamma> \<Omega> G (Inl n, Normal ns1) (m2, s2)) \<Longrightarrow> (s2 \<noteq> Failure)))"
+  and "bb = (BigBlock name [] any_str any_tr)"
   (* TODO: You're requiring that the loop isn't empty! What if it is? *)
   and bb_successor_while: "any_str = Some (ParsedWhile cont_guard invs (bb0#body_bbs))"
   and block_local_rel:
-    "\<And> reached_bb_inter reached_cont_inter reached_state_inter. (red_bigblock A M \<Lambda> \<Gamma> \<Omega> T ((BigBlock name [] any_str any_tr), KEndBlock cont1, (Normal ns1)) (reached_bb_inter, reached_cont_inter, reached_state_inter)) \<Longrightarrow> 
+    "\<And> reached_bb_inter reached_cont_inter reached_state_inter. (red_bigblock A M \<Lambda> \<Gamma> \<Omega> T (bb, KEndBlock cont1, (Normal ns1)) (reached_bb_inter, reached_cont_inter, reached_state_inter)) \<Longrightarrow> 
     (\<And> s2'.((red_cmd_list A M \<Lambda> \<Gamma> \<Omega> assertions (Normal ns1) s2') \<Longrightarrow> (s2' \<noteq> Failure))) \<Longrightarrow>   
     (reached_state_inter \<noteq> Failure  \<and> (\<forall>ns1'. reached_state_inter = Normal ns1' \<longrightarrow> (A,M,\<Lambda>,\<Gamma>,\<Omega> \<turnstile> \<langle>assertions, Normal ns1\<rangle> [\<rightarrow>] Normal ns1')))"
-  (* TODO: The following is a sketchy assumption! Fix it!*)
-  and "assertions \<noteq> []" 
   and "node_to_block(G) ! n = assertions"
   and succ_correct: 
    "\<And> ns1'' loop_guard j'. 
@@ -755,28 +1158,28 @@ lemma block_global_rel_loop_head:
     (\<forall>msuc2.  List.member (out_edges(G) ! n) msuc2 \<longrightarrow> (\<forall>m3 s3. ((A,M,\<Lambda>,\<Gamma>,\<Omega>,G \<turnstile> (Inl(msuc2), Normal ns1'') -n\<rightarrow>* (m3, s3)) \<longrightarrow> s3 \<noteq> Failure))) \<Longrightarrow>
     ((cont_guard = Some loop_guard) \<and> 
       (red_expr A \<Lambda> \<Gamma> \<Omega> loop_guard ns1'' (BoolV True)) \<and> 
-      A,M,\<Lambda>,\<Gamma>,\<Omega>,T \<turnstile> (bb0, convert_list_to_cont (rev ((BigBlock name [] any_str any_tr)#body_bbs)) (KEndBlock cont1), (Normal ns1'')) -n\<longrightarrow>^j' (reached_bb, reached_cont, reached_state)) \<or> 
+      A,M,\<Lambda>,\<Gamma>,\<Omega>,T \<turnstile> (bb0, convert_list_to_cont (bb#(rev body_bbs)) (KEndBlock cont1), (Normal ns1'')) -n\<longrightarrow>^j' (reached_bb, reached_cont, reached_state)) \<or> 
     ((cont_guard = Some loop_guard) \<and> 
       (red_expr A \<Lambda> \<Gamma> \<Omega> loop_guard ns1'' (BoolV False)) \<and> 
       A,M,\<Lambda>,\<Gamma>,\<Omega>,T \<turnstile> ((BigBlock name [] None None), KEndBlock cont1, (Normal ns1'')) -n\<longrightarrow>^j' (reached_bb, reached_cont, reached_state)) \<or>
     ((cont_guard = None) \<and> 
      ((A,M,\<Lambda>,\<Gamma>,\<Omega>,T \<turnstile> ((BigBlock name [] None None), KEndBlock cont1, (Normal ns1'')) -n\<longrightarrow>^j' (reached_bb, reached_cont, reached_state)) \<or>
-      (A,M,\<Lambda>,\<Gamma>,\<Omega>,T \<turnstile> (bb0, convert_list_to_cont (rev ((BigBlock name [] any_str any_tr)#body_bbs)) (KEndBlock cont1), (Normal ns1'')) -n\<longrightarrow>^j' (reached_bb, reached_cont, reached_state))))  \<Longrightarrow>  
+      (A,M,\<Lambda>,\<Gamma>,\<Omega>,T \<turnstile> (bb0, convert_list_to_cont (bb#(rev body_bbs)) (KEndBlock cont1), (Normal ns1'')) -n\<longrightarrow>^j' (reached_bb, reached_cont, reached_state))))  \<Longrightarrow>  
     (Ast.valid_configuration A \<Lambda> \<Gamma> \<Omega> posts reached_bb reached_cont reached_state)"
   shows "(Ast.valid_configuration A \<Lambda> \<Gamma> \<Omega> posts reached_bb reached_cont reached_state)" 
   using assms
 proof cases
-    case (Rel_Invs)
+    case Rel_Invs
     thus ?thesis 
     proof cases
       assume "j = 0"
-      hence "(reached_bb, reached_cont, reached_state) = ((BigBlock name [] any_str any_tr), KEndBlock cont1, (Normal ns1))" using ast_trace by simp 
+      hence "(reached_bb, reached_cont, reached_state) = ((BigBlock name [] any_str any_tr), KEndBlock cont1, (Normal ns1))" using ast_trace assms(4) by simp 
       thus ?thesis by (simp add: Ast.valid_configuration_def)
     next
       assume "j \<noteq> 0" 
       from this obtain j' where "j = Suc j'" using not0_implies_Suc by blast
   
-      from ast_trace this obtain inter_bb inter_cont inter_state where
+      from ast_trace this assms(4) obtain inter_bb inter_cont inter_state where
         first_step: "A,M,\<Lambda>,\<Gamma>,\<Omega>,T \<turnstile> \<langle>((BigBlock name [] any_str any_tr), KEndBlock cont1, (Normal ns1))\<rangle> \<longrightarrow> (inter_bb, inter_cont, inter_state)" and
         rest: "A,M,\<Lambda>,\<Gamma>,\<Omega>,T \<turnstile> (inter_bb, inter_cont, inter_state) -n\<longrightarrow>^j' (reached_bb, reached_cont, reached_state)"
         by (metis prod_cases3 relpowp_Suc_D2)
@@ -787,25 +1190,25 @@ proof cases
         from first_step show ?thesis using bb_successor_while
         proof cases
           case RedParsedWhileTrue
-          hence concrete_inter1: "(inter_bb, inter_cont, inter_state) = (bb0, convert_list_to_cont (rev ((BigBlock name [] any_str any_tr)#body_bbs)) (KEndBlock cont1), (Normal ns1))"
+          hence concrete_inter1: "(inter_bb, inter_cont, inter_state) = (bb0, convert_list_to_cont ((BigBlock name [] any_str any_tr)#(rev body_bbs)) (KEndBlock cont1), (Normal ns1))"
             using bb_successor_while None by blast
   
           from first_step
           have succ_cfg_correct: "(\<forall>msuc2.  List.member (out_edges(G) ! n) msuc2 \<longrightarrow> (\<forall>m3 s3. ((A,M,\<Lambda>,\<Gamma>,\<Omega>,G \<turnstile> (Inl(msuc2), inter_state) -n\<rightarrow>* (m3, s3)) \<longrightarrow> s3 \<noteq> Failure)))"
-            by (metis Pair_inject assms(7) block_local_rel cfg_correct concrete_inter1 dag_verifies_propagate dag_verifies_propagate_2)
+            by (metis Pair_inject assms(4) assms(7) block_local_rel cfg_correct concrete_inter1 dag_verifies_propagate dag_verifies_propagate_2)
   
-          show ?thesis using \<open>j = Suc j'\<close> succ_cfg_correct None rest concrete_inter1 succ_correct by blast 
+          show ?thesis using \<open>j = Suc j'\<close> succ_cfg_correct None rest concrete_inter1 succ_correct assms(4) by blast 
         next 
           case RedParsedWhileFalse
           hence concrete_inter2: "(inter_bb, inter_cont, inter_state) = ((BigBlock name [] None None), KEndBlock cont1, (Normal ns1))" by simp
   
           from first_step
           have succ_cfg_correct: "(\<forall>msuc2.  List.member (out_edges(G) ! n) msuc2 \<longrightarrow> (\<forall>m3 s3. ((A,M,\<Lambda>,\<Gamma>,\<Omega>,G \<turnstile> (Inl(msuc2), inter_state) -n\<rightarrow>* (m3, s3)) \<longrightarrow> s3 \<noteq> Failure)))"
-            by (metis assms(7) block_local_rel cfg_correct dag_verifies_propagate dag_verifies_propagate_2 local.RedParsedWhileFalse(5))
+            by (metis assms(4) assms(7) block_local_rel cfg_correct dag_verifies_propagate dag_verifies_propagate_2 local.RedParsedWhileFalse(5))
   
           show ?thesis using \<open>j = Suc j'\<close> succ_cfg_correct None rest concrete_inter2 succ_correct by blast
         next 
-          case RedParsedWhile_InvFail thus ?thesis using assms(7) block_local_rel cfg_correct dag_verifies_propagate_2 first_step by blast
+          case RedParsedWhile_InvFail thus ?thesis using assms(7) block_local_rel cfg_correct dag_verifies_propagate_2 first_step assms(4) by blast
         qed auto
       next
         case (Some concrete_loop_guard)
@@ -817,16 +1220,16 @@ proof cases
           from first_step show ?thesis 
           proof cases
             case RedParsedWhileTrue
-            hence concrete_inter3: "(inter_bb, inter_cont, inter_state) = (bb0, convert_list_to_cont (rev ((BigBlock name [] any_str any_tr)#body_bbs)) (KEndBlock cont1), (Normal ns1))"
+            hence concrete_inter3: "(inter_bb, inter_cont, inter_state) = (bb0, convert_list_to_cont ((BigBlock name [] any_str any_tr)#(rev body_bbs)) (KEndBlock cont1), (Normal ns1))"
               using bb_successor_while Some by blast
   
             from first_step
             have succ_cfg_correct: "(\<forall>msuc2.  List.member (out_edges(G) ! n) msuc2 \<longrightarrow> (\<forall>m3 s3. ((A,M,\<Lambda>,\<Gamma>,\<Omega>,G \<turnstile> (Inl(msuc2), inter_state) -n\<rightarrow>* (m3, s3)) \<longrightarrow> s3 \<noteq> Failure)))"
-              by (metis Pair_inject assms(7) block_local_rel cfg_correct concrete_inter3 dag_verifies_propagate dag_verifies_propagate_2)
+              by (metis Pair_inject assms(4) assms(7) block_local_rel cfg_correct concrete_inter3 dag_verifies_propagate dag_verifies_propagate_2)
   
-            show ?thesis using \<open>j = Suc j'\<close> succ_cfg_correct Some guard_true rest concrete_inter3 succ_correct by blast 
+            show ?thesis using \<open>j = Suc j'\<close> succ_cfg_correct Some guard_true rest concrete_inter3 succ_correct assms(4) by blast 
         next 
-            case RedParsedWhile_InvFail thus ?thesis using assms(7) block_local_rel cfg_correct dag_verifies_propagate_2 first_step by blast
+            case RedParsedWhile_InvFail thus ?thesis using assms(7) block_local_rel cfg_correct dag_verifies_propagate_2 first_step assms(4) by blast
         qed (auto simp add: bb_successor_while Some guard_not_false)
       next
         assume guard_not_true: "\<not> (red_expr A \<Lambda> \<Gamma> \<Omega> concrete_loop_guard ns1 (BoolV True))"
@@ -841,7 +1244,7 @@ proof cases
 
           from first_step
           have succ_cfg_correct: "(\<forall>msuc2.  List.member (out_edges(G) ! n) msuc2 \<longrightarrow> (\<forall>m3 s3. ((A,M,\<Lambda>,\<Gamma>,\<Omega>,G \<turnstile> (Inl(msuc2), inter_state) -n\<rightarrow>* (m3, s3)) \<longrightarrow> s3 \<noteq> Failure)))"
-            by (metis assms(7) block_local_rel cfg_correct dag_verifies_propagate dag_verifies_propagate_2 local.RedParsedWhileFalse(5))
+            by (metis assms(4) assms(7) block_local_rel cfg_correct dag_verifies_propagate dag_verifies_propagate_2 local.RedParsedWhileFalse(5))
   
             show ?thesis using \<open>j = Suc j'\<close> succ_cfg_correct Some guard_false rest concrete_inter4 succ_correct by blast
           next
@@ -857,20 +1260,112 @@ proof cases
       qed
     qed
   qed
-qed auto
+next 
+  case Rel_Main_test 
+  thus ?thesis
+    proof cases
+      assume "j = 0"
+      hence "(reached_bb, reached_cont, reached_state) = ((BigBlock name [] any_str any_tr), KEndBlock cont1, (Normal ns1))" using ast_trace assms(4) by simp 
+      thus ?thesis by (simp add: Ast.valid_configuration_def)
+    next
+      assume "j \<noteq> 0" 
+      from this obtain j' where "j = Suc j'" using not0_implies_Suc by blast
+  
+      from ast_trace this assms(4) obtain inter_bb inter_cont inter_state where
+        first_step: "A,M,\<Lambda>,\<Gamma>,\<Omega>,T \<turnstile> \<langle>((BigBlock name [] any_str any_tr), KEndBlock cont1, (Normal ns1))\<rangle> \<longrightarrow> (inter_bb, inter_cont, inter_state)" and
+        rest: "A,M,\<Lambda>,\<Gamma>,\<Omega>,T \<turnstile> (inter_bb, inter_cont, inter_state) -n\<longrightarrow>^j' (reached_bb, reached_cont, reached_state)"
+        by (metis prod_cases3 relpowp_Suc_D2)
+  
+      show ?thesis
+      proof (cases cont_guard)
+        case None
+        from first_step show ?thesis using bb_successor_while
+        proof cases
+          case RedParsedWhileTrue
+          hence concrete_inter1: "(inter_bb, inter_cont, inter_state) = (bb0, convert_list_to_cont ((BigBlock name [] any_str any_tr)#(rev body_bbs)) (KEndBlock cont1), (Normal ns1))"
+            using bb_successor_while None by blast
+  
+          from first_step
+          have succ_cfg_correct: "(\<forall>msuc2.  List.member (out_edges(G) ! n) msuc2 \<longrightarrow> (\<forall>m3 s3. ((A,M,\<Lambda>,\<Gamma>,\<Omega>,G \<turnstile> (Inl(msuc2), inter_state) -n\<rightarrow>* (m3, s3)) \<longrightarrow> s3 \<noteq> Failure)))"
+            by (metis Pair_inject assms(4) assms(7) block_local_rel cfg_correct concrete_inter1 dag_verifies_propagate dag_verifies_propagate_2)
+  
+          show ?thesis using \<open>j = Suc j'\<close> succ_cfg_correct None rest concrete_inter1 succ_correct assms(4) by blast 
+        next 
+          case RedParsedWhileFalse
+          hence concrete_inter2: "(inter_bb, inter_cont, inter_state) = ((BigBlock name [] None None), KEndBlock cont1, (Normal ns1))" by simp
+  
+          from first_step
+          have succ_cfg_correct: "(\<forall>msuc2.  List.member (out_edges(G) ! n) msuc2 \<longrightarrow> (\<forall>m3 s3. ((A,M,\<Lambda>,\<Gamma>,\<Omega>,G \<turnstile> (Inl(msuc2), inter_state) -n\<rightarrow>* (m3, s3)) \<longrightarrow> s3 \<noteq> Failure)))"
+            by (metis assms(4) assms(7) block_local_rel cfg_correct dag_verifies_propagate dag_verifies_propagate_2 local.RedParsedWhileFalse(5))
+  
+          show ?thesis using \<open>j = Suc j'\<close> succ_cfg_correct None rest concrete_inter2 succ_correct by blast
+        next 
+          case RedParsedWhile_InvFail thus ?thesis using assms(7) block_local_rel cfg_correct dag_verifies_propagate_2 first_step assms(4) by blast
+        qed auto
+      next
+        case (Some concrete_loop_guard)
+        then show ?thesis 
+        proof cases
+          assume guard_true: "(red_expr A \<Lambda> \<Gamma> \<Omega> concrete_loop_guard ns1 (BoolV True))"
+          hence guard_not_false: "\<not> (red_expr A \<Lambda> \<Gamma> \<Omega> concrete_loop_guard ns1 (BoolV False))" using expr_eval_determ by blast
+  
+          from first_step show ?thesis 
+          proof cases
+            case RedParsedWhileTrue
+            hence concrete_inter3: "(inter_bb, inter_cont, inter_state) = (bb0, convert_list_to_cont ((BigBlock name [] any_str any_tr)#(rev body_bbs)) (KEndBlock cont1), (Normal ns1))"
+              using bb_successor_while Some by blast
+  
+            from first_step
+            have succ_cfg_correct: "(\<forall>msuc2.  List.member (out_edges(G) ! n) msuc2 \<longrightarrow> (\<forall>m3 s3. ((A,M,\<Lambda>,\<Gamma>,\<Omega>,G \<turnstile> (Inl(msuc2), inter_state) -n\<rightarrow>* (m3, s3)) \<longrightarrow> s3 \<noteq> Failure)))"
+              by (metis Pair_inject assms(4) assms(7) block_local_rel cfg_correct concrete_inter3 dag_verifies_propagate dag_verifies_propagate_2)
+  
+            show ?thesis using \<open>j = Suc j'\<close> succ_cfg_correct Some guard_true rest concrete_inter3 succ_correct assms(4) by blast 
+        next 
+            case RedParsedWhile_InvFail thus ?thesis using assms(7) block_local_rel cfg_correct dag_verifies_propagate_2 first_step assms(4) by blast
+        qed (auto simp add: bb_successor_while Some guard_not_false)
+      next
+        assume guard_not_true: "\<not> (red_expr A \<Lambda> \<Gamma> \<Omega> concrete_loop_guard ns1 (BoolV True))"
+        thus ?thesis 
+        proof cases
+          assume guard_false: "(red_expr A \<Lambda> \<Gamma> \<Omega> concrete_loop_guard ns1 (BoolV False))"
+  
+          from first_step show ?thesis 
+          proof cases
+            case RedParsedWhileFalse
+            hence concrete_inter4: "(inter_bb, inter_cont, inter_state) = ((BigBlock name [] None None), KEndBlock cont1, (Normal ns1))" by simp
+
+          from first_step
+          have succ_cfg_correct: "(\<forall>msuc2.  List.member (out_edges(G) ! n) msuc2 \<longrightarrow> (\<forall>m3 s3. ((A,M,\<Lambda>,\<Gamma>,\<Omega>,G \<turnstile> (Inl(msuc2), inter_state) -n\<rightarrow>* (m3, s3)) \<longrightarrow> s3 \<noteq> Failure)))"
+            by (metis assms(4) assms(7) block_local_rel cfg_correct dag_verifies_propagate dag_verifies_propagate_2 local.RedParsedWhileFalse(5))
+  
+            show ?thesis using \<open>j = Suc j'\<close> succ_cfg_correct Some guard_false rest concrete_inter4 succ_correct by blast
+          next
+            case RedParsedWhile_InvFail thus ?thesis using Some bb_successor_while guard_not_true by blast
+          qed (auto simp add: bb_successor_while Some guard_not_true)
+        next
+          assume guard_not_false: "\<not> (red_expr A \<Lambda> \<Gamma> \<Omega> concrete_loop_guard ns1 (BoolV False))"
+          from first_step show ?thesis
+          proof cases
+            case RedParsedWhile_InvFail thus ?thesis using Some bb_successor_while guard_not_true by blast
+          qed (auto simp add: bb_successor_while Some guard_not_true guard_not_false)
+        qed
+      qed
+    qed
+  qed
+qed 
 
 text \<open>Global lemma for an ast-bigblock with a non-empty set of simple cmds which enters an if-statement after executing its simple cmds.\<close>
 lemma block_global_rel_if_successor:
-  assumes block_rel: "ast_cfg_rel None [] (BigBlock name cs1 any_str any_tr) cs2"
-  and ast_trace: "A,M,\<Lambda>,\<Gamma>,\<Omega>,T \<turnstile> ((BigBlock name cs1 any_str any_tr), cont0, (Normal ns1)) -n\<longrightarrow>^j (reached_bb, reached_cont, reached_state)"
-  and "cs1 \<noteq> Nil"
-  and "cs2 \<noteq> Nil"
+  assumes block_rel: "ast_cfg_rel None [] bb cs2"
+  and ast_trace: "A,M,\<Lambda>,\<Gamma>,\<Omega>,T \<turnstile> (bb, cont0, (Normal ns1)) -n\<longrightarrow>^j (reached_bb, reached_cont, reached_state)"
+  and "bb = (BigBlock name cs1 any_str any_tr)"
   and "node_to_block(G) ! n = cs2"
   and cfg_correct: "(\<And> m2 s2. ((red_cfg_multi A M \<Lambda> \<Gamma> \<Omega> G (Inl n, Normal ns1) (m2, s2)) \<Longrightarrow> (s2 \<noteq> Failure)))"
   and bb_successor_if: "any_str = Some (ParsedIf cont_guard (then0#then_bbs) (else0#else_bbs))"
   and block_local_rel:
         "\<And> reached_bb_inter reached_cont_inter reached_state_inter. (red_bigblock A M \<Lambda> \<Gamma> \<Omega> T ((BigBlock name cs1 any_str any_tr), cont0, (Normal ns1)) (reached_bb_inter, reached_cont_inter, reached_state_inter)) \<Longrightarrow> 
-        (\<And> s2'.((red_cmd_list A M \<Lambda> \<Gamma> \<Omega> cs2 (Normal ns1) s2') \<Longrightarrow> (s2' \<noteq> Failure))) \<Longrightarrow>   
+        (\<And> s2'.((red_cmd_list A M \<Lambda> \<Gamma> \<Omega> cs2 (Normal ns1) s2') \<Longrightarrow> (s2' \<noteq> Failure))) \<Longrightarrow> 
+        cs1 \<noteq> [] \<Longrightarrow> cs2 \<noteq> [] \<Longrightarrow>  
         (reached_state_inter \<noteq> Failure  \<and> (\<forall>ns1'. reached_state_inter = Normal ns1' \<longrightarrow> (A,M,\<Lambda>,\<Gamma>,\<Omega> \<turnstile> \<langle>cs2, Normal ns1\<rangle> [\<rightarrow>] Normal ns1')))"
   and succ_correct: 
        "\<And> ns1'' block_guard k.
@@ -891,123 +1386,88 @@ lemma block_global_rel_if_successor:
 proof cases
   case Rel_Main_test
   have not_end: "(cont0 \<noteq> KStop) \<or> any_str \<noteq> None \<or> any_tr \<noteq> None" using bb_successor_if by simp
-  from ast_trace show ?thesis
-  proof (cases j)
-    case 0
-    hence "(reached_bb, reached_cont, reached_state) = ((BigBlock name cs1 any_str any_tr), cont0, (Normal ns1))" using ast_trace by auto
-    then show ?thesis by (simp add: Ast.valid_configuration_def bb_successor_if) 
-  next
-    case 1: (Suc j')
-    from this obtain inter_bb inter_cont inter_state where
-      first_step: "red_bigblock A M \<Lambda> \<Gamma> \<Omega> T ((BigBlock name cs1 any_str any_tr), cont0, (Normal ns1)) (inter_bb, inter_cont, inter_state)" and
-      rest_of_steps: "A,M,\<Lambda>,\<Gamma>,\<Omega>,T \<turnstile> (inter_bb, inter_cont, inter_state) -n\<longrightarrow>^j' (reached_bb, reached_cont, reached_state)" 
-      by (metis ast_trace get_state.cases relpowp_Suc_E2)
-
-    from cfg_correct \<open>cs2 \<noteq> Nil\<close> \<open>node_to_block(G) ! n = cs2\<close> 
-    have local_rel_corr: "(\<And> s2'.((red_cmd_list A M \<Lambda> \<Gamma> \<Omega> (cs2) (Normal ns1) s2') \<Longrightarrow> (s2' \<noteq> Failure)))"
-      using dag_verifies_propagate_2 by blast
-
-    from local_rel_corr first_step 
-    have a2: "(inter_state \<noteq> Failure  \<and> (\<forall>ns1'. inter_state = Normal ns1' \<longrightarrow> (A,M,\<Lambda>,\<Gamma>,\<Omega> \<turnstile> \<langle>cs2, Normal ns1\<rangle> [\<rightarrow>] Normal ns1')))" 
-      using block_local_rel by simp
-
-    from first_step \<open>cs1 \<noteq> Nil\<close> 
-    have a1: "(inter_bb, inter_cont, inter_state) = ((BigBlock name [] any_str any_tr), cont0, inter_state)"
-    proof cases
-      case RedSimpleCmds then show ?thesis by (auto simp add: RedSimpleCmds)
-    qed auto
-
-    show ?thesis 
-    proof (cases inter_state)
-      case 2: (Normal x1)
-      from rest_of_steps show ?thesis 
-      proof (cases j')
-        case 0
-        then show ?thesis 
-          by (metis Ast.valid_configuration_def a1 a2 bb_successor_if get_state.simps is_final.simps(3) relpowp_0_E rest_of_steps) 
-      next
-        case 3: (Suc j'')
-        from this rest_of_steps obtain snd_inter_bb snd_inter_cont snd_inter_state where
-          snd_step: "red_bigblock A M \<Lambda> \<Gamma> \<Omega> T ((BigBlock name [] any_str any_tr), cont0, inter_state)  (snd_inter_bb, snd_inter_cont, snd_inter_state)" and
-          snd_rest_of_steps: "A,M,\<Lambda>,\<Gamma>,\<Omega>,T \<turnstile> (snd_inter_bb, snd_inter_cont, snd_inter_state) -n\<longrightarrow>^j'' (reached_bb, reached_cont, reached_state)"
-          by (metis a1 get_state.cases relpowp_Suc_D2)
-
+  show ?thesis
+  proof (cases cs2)
+    case Nil 
+    thus ?thesis
+    proof (cases j)
+      case 0
+      hence "(reached_bb, reached_cont, reached_state) = ((BigBlock name cs1 any_str any_tr), cont0, (Normal ns1))" using ast_trace assms(3) by auto
+      then show ?thesis by (simp add: Ast.valid_configuration_def bb_successor_if) 
+    next
+      case 1: (Suc j')
+        from this assms(3) obtain snd_inter_bb snd_inter_cont snd_inter_state where
+          snd_step: "red_bigblock A M \<Lambda> \<Gamma> \<Omega> T ((BigBlock name [] any_str any_tr), cont0, (Normal ns1))  (snd_inter_bb, snd_inter_cont, snd_inter_state)" and
+          snd_rest_of_steps: "A,M,\<Lambda>,\<Gamma>,\<Omega>,T \<turnstile> (snd_inter_bb, snd_inter_cont, snd_inter_state) -n\<longrightarrow>^j' (reached_bb, reached_cont, reached_state)"
+          by (metis ast_trace bigblock.inject local.Nil local.Rel_Main_test relpowp_Suc_E2 surj_pair)
+  
         thus ?thesis 
         proof (cases cont_guard)
           case None
           from snd_step this show ?thesis
           proof cases
             case RedParsedIfTrue
-            hence eq: "(snd_inter_bb, snd_inter_cont, snd_inter_state) = (then0, convert_list_to_cont (rev then_bbs) cont0, inter_state)" using None bb_successor_if 1 by auto
-
-            from first_step 
-            have succ_cfg_correct: "(\<forall>msuc2.  List.member (out_edges(G) ! n) msuc2 \<longrightarrow> (\<forall>m3 s3. ((A,M,\<Lambda>,\<Gamma>,\<Omega>,G \<turnstile> (Inl(msuc2), inter_state) -n\<rightarrow>* (m3, s3)) \<longrightarrow> s3 \<noteq> Failure)))"
-            proof cases
-              case RedSimpleCmds show ?thesis using 2 eq RedSimpleCmds(3) dag_verifies_propagate assms(5) Rel_Main_test(1) cfg_correct by blast
-            qed (auto simp add: \<open>cs1 \<noteq> Nil\<close>)
-
-            have "j'' < j" using 1 3 using Suc_lessD by blast
+            hence eq: "(snd_inter_bb, snd_inter_cont, snd_inter_state) = (then0, convert_list_to_cont (rev then_bbs) cont0, (Normal ns1))" using None bb_successor_if 1 by auto
+  
+            have succ_cfg_correct: "(\<forall>msuc2.  List.member (out_edges(G) ! n) msuc2 \<longrightarrow> (\<forall>m3 s3. ((A,M,\<Lambda>,\<Gamma>,\<Omega>,G \<turnstile> (Inl(msuc2), (Normal ns1)) -n\<rightarrow>* (m3, s3)) \<longrightarrow> s3 \<noteq> Failure)))"
+              using assms(4) cfg_correct correctness_propagates_through_empty local.Nil by blast
+  
+            have "j' < j" using 1 using Suc_lessD by blast
             
-            thus ?thesis using eq snd_rest_of_steps succ_correct None 2 succ_cfg_correct by blast
+            thus ?thesis using eq snd_rest_of_steps succ_correct None succ_cfg_correct by blast
           next
             case RedParsedIfFalse
-            hence eq: "(snd_inter_bb, snd_inter_cont, snd_inter_state) = (else0, convert_list_to_cont (rev else_bbs) cont0, inter_state)" using None bb_successor_if 1 by auto
-
-            from first_step 
-            have succ_cfg_correct: "(\<forall>msuc2.  List.member (out_edges(G) ! n) msuc2 \<longrightarrow> (\<forall>m3 s3. ((A,M,\<Lambda>,\<Gamma>,\<Omega>,G \<turnstile> (Inl(msuc2), inter_state) -n\<rightarrow>* (m3, s3)) \<longrightarrow> s3 \<noteq> Failure)))"
-            proof cases
-              case RedSimpleCmds show ?thesis using 2 eq RedSimpleCmds(3) dag_verifies_propagate assms(5) Rel_Main_test(1) cfg_correct by blast
-            qed (auto simp add: \<open>cs1 \<noteq> Nil\<close>)
-
-            have "j'' < j" using 1 3 using Suc_lessD by blast
-
-            thus ?thesis using eq snd_rest_of_steps succ_correct None 2 succ_cfg_correct by blast
-          qed (auto simp add: bb_successor_if 2)
+            hence eq: "(snd_inter_bb, snd_inter_cont, snd_inter_state) = (else0, convert_list_to_cont (rev else_bbs) cont0, (Normal ns1))" using None bb_successor_if 1 by auto
+  
+            from snd_step 
+            have succ_cfg_correct: "(\<forall>msuc2.  List.member (out_edges(G) ! n) msuc2 \<longrightarrow> (\<forall>m3 s3. ((A,M,\<Lambda>,\<Gamma>,\<Omega>,G \<turnstile> (Inl(msuc2), (Normal ns1)) -n\<rightarrow>* (m3, s3)) \<longrightarrow> s3 \<noteq> Failure)))"
+              using assms(4) cfg_correct correctness_propagates_through_empty local.Nil by blast
+  
+            have "j' < j" using 1 using Suc_lessD by blast
+  
+            thus ?thesis using eq snd_rest_of_steps succ_correct None succ_cfg_correct by blast
+          qed (auto simp add: bb_successor_if)
         next
           case (Some block_guard)
           then show ?thesis 
           proof cases
-            assume guard_true: "(red_expr A \<Lambda> \<Gamma> \<Omega> block_guard x1 (BoolV True))"
-            hence guard_not_false: "\<not> (red_expr A \<Lambda> \<Gamma> \<Omega> block_guard x1 (BoolV False))" using expr_eval_determ by blast
-            from snd_step have eq: "(snd_inter_bb, snd_inter_cont, snd_inter_state) = (then0, convert_list_to_cont (rev then_bbs) cont0, inter_state)" 
+            assume guard_true: "(red_expr A \<Lambda> \<Gamma> \<Omega> block_guard ns1 (BoolV True))"
+            hence guard_not_false: "\<not> (red_expr A \<Lambda> \<Gamma> \<Omega> block_guard ns1 (BoolV False))" using expr_eval_determ by blast
+            from snd_step have eq: "(snd_inter_bb, snd_inter_cont, snd_inter_state) = (then0, convert_list_to_cont (rev then_bbs) cont0, Normal ns1)" 
             proof cases
               case RedParsedIfTrue thus ?thesis using guard_true bb_successor_if by (simp add: RedParsedIfTrue)
-            qed (auto simp add: guard_not_false bb_successor_if 2 Some)
-
-            from first_step 
-            have succ_cfg_correct: "(\<forall>msuc2.  List.member (out_edges(G) ! n) msuc2 \<longrightarrow> (\<forall>m3 s3. ((A,M,\<Lambda>,\<Gamma>,\<Omega>,G \<turnstile> (Inl(msuc2), inter_state) -n\<rightarrow>* (m3, s3)) \<longrightarrow> s3 \<noteq> Failure)))"
-            proof cases
-              case RedSimpleCmds show ?thesis using 2 eq RedSimpleCmds(3) dag_verifies_propagate assms(5) Rel_Main_test(1) cfg_correct by blast
-            qed (auto simp add: \<open>cs1 \<noteq> Nil\<close>)
-
-            have "j'' < j" using 1 3 using Suc_lessD by blast
+            qed (auto simp add: guard_not_false bb_successor_if Some)
+  
+            from snd_step 
+            have succ_cfg_correct: "(\<forall>msuc2.  List.member (out_edges(G) ! n) msuc2 \<longrightarrow> (\<forall>m3 s3. ((A,M,\<Lambda>,\<Gamma>,\<Omega>,G \<turnstile> (Inl(msuc2), Normal ns1) -n\<rightarrow>* (m3, s3)) \<longrightarrow> s3 \<noteq> Failure)))"
+              using assms(4) cfg_correct correctness_propagates_through_empty local.Nil by blast
+  
+            have "j' < j" using 1 using Suc_lessD by blast
             
-            thus ?thesis using eq guard_true snd_rest_of_steps succ_correct Some succ_cfg_correct 2 by blast
+            thus ?thesis using eq guard_true snd_rest_of_steps succ_correct Some succ_cfg_correct by blast
           next
-            assume guard_not_true: "\<not> (red_expr A \<Lambda> \<Gamma> \<Omega> block_guard x1 (BoolV True))"
+            assume guard_not_true: "\<not> (red_expr A \<Lambda> \<Gamma> \<Omega> block_guard ns1 (BoolV True))"
             thus ?thesis 
             proof cases
-              assume guard_false: "(red_expr A \<Lambda> \<Gamma> \<Omega> block_guard x1 (BoolV False))"
-              from snd_step have eq: "(snd_inter_bb, snd_inter_cont, snd_inter_state) = (else0, convert_list_to_cont (rev else_bbs) cont0, inter_state)" 
+              assume guard_false: "(red_expr A \<Lambda> \<Gamma> \<Omega> block_guard ns1 (BoolV False))"
+              from snd_step have eq: "(snd_inter_bb, snd_inter_cont, snd_inter_state) = (else0, convert_list_to_cont (rev else_bbs) cont0, Normal ns1)" 
               proof cases
                 case RedParsedIfFalse thus ?thesis using guard_false bb_successor_if by (simp add: RedParsedIfFalse)
-              qed (auto simp add: guard_not_true bb_successor_if 2 Some)
-
-              from first_step 
-              have succ_cfg_correct: "(\<forall>msuc2.  List.member (out_edges(G) ! n) msuc2 \<longrightarrow> (\<forall>m3 s3. ((A,M,\<Lambda>,\<Gamma>,\<Omega>,G \<turnstile> (Inl(msuc2), inter_state) -n\<rightarrow>* (m3, s3)) \<longrightarrow> s3 \<noteq> Failure)))"
-              proof cases
-                case RedSimpleCmds show ?thesis using 2 eq RedSimpleCmds(3) dag_verifies_propagate assms(5) Rel_Main_test(1) cfg_correct by blast
-              qed (auto simp add: \<open>cs1 \<noteq> Nil\<close>)              
-
-              have "j'' < j" using 1 3 using Suc_lessD by blast
+              qed (auto simp add: guard_not_true bb_successor_if Some)
+  
+              from snd_step 
+              have succ_cfg_correct: "(\<forall>msuc2.  List.member (out_edges(G) ! n) msuc2 \<longrightarrow> (\<forall>m3 s3. ((A,M,\<Lambda>,\<Gamma>,\<Omega>,G \<turnstile> (Inl(msuc2), Normal ns1) -n\<rightarrow>* (m3, s3)) \<longrightarrow> s3 \<noteq> Failure)))"
+                using assms(4) cfg_correct correctness_propagates_through_empty local.Nil by blast              
+  
+              have "j' < j" using 1 using Suc_lessD by blast
         
-              thus ?thesis using eq guard_false snd_rest_of_steps succ_correct Some 2 succ_cfg_correct by blast
+              thus ?thesis using eq guard_false snd_rest_of_steps succ_correct Some succ_cfg_correct by blast
             next
-              assume guard_not_false2: "(\<not> (red_expr A \<Lambda> \<Gamma> \<Omega> block_guard x1 (BoolV False)))" and  
-                     guard_not_true2: "(\<not> (red_expr A \<Lambda> \<Gamma> \<Omega> block_guard x1 (BoolV True)))"
+              assume guard_not_false2: "(\<not> (red_expr A \<Lambda> \<Gamma> \<Omega> block_guard ns1 (BoolV False)))" and  
+                     guard_not_true2: "(\<not> (red_expr A \<Lambda> \<Gamma> \<Omega> block_guard ns1 (BoolV True)))"
               thus ?thesis
               proof -
-                from snd_step have False using guard_not_false2 guard_not_true2 bb_successor_if Some 2 
+                from snd_step have False using guard_not_false2 guard_not_true2 bb_successor_if Some 
                   by (cases) auto
                 thus ?thesis by simp
               qed
@@ -1015,22 +1475,248 @@ proof cases
           qed 
         qed
       qed
+  next
+    case (Cons) 
+    hence "cs1 \<noteq> []" using assms(3) local.Rel_Main_test by auto
+    thus ?thesis
+    proof (cases j)
+      case 0
+      hence "(reached_bb, reached_cont, reached_state) = ((BigBlock name cs1 any_str any_tr), cont0, (Normal ns1))" using ast_trace assms(3) by auto
+      then show ?thesis by (simp add: Ast.valid_configuration_def bb_successor_if) 
     next
-      case Failure
-      then show ?thesis
-        using \<open>inter_state \<noteq> Failure \<and> (\<forall>ns1'. inter_state = Normal ns1' \<longrightarrow> A,M,\<Lambda>,\<Gamma>,\<Omega> \<turnstile> \<langle>cs2,Normal ns1\<rangle> [\<rightarrow>] Normal ns1')\<close> 
-        by linarith
-    next
-      case Magic
-      then show ?thesis by (metis Ast.valid_configuration_def a2 get_state.simps magic_propagates rest_of_steps state.distinct(3))
+      case 1: (Suc j')
+      from this assms(3) obtain inter_bb inter_cont inter_state where
+        first_step: "red_bigblock A M \<Lambda> \<Gamma> \<Omega> T ((BigBlock name cs1 any_str any_tr), cont0, (Normal ns1)) (inter_bb, inter_cont, inter_state)" and
+        rest_of_steps: "A,M,\<Lambda>,\<Gamma>,\<Omega>,T \<turnstile> (inter_bb, inter_cont, inter_state) -n\<longrightarrow>^j' (reached_bb, reached_cont, reached_state)" 
+        by (metis ast_trace get_state.cases relpowp_Suc_E2)
+  
+      from cfg_correct Cons \<open>node_to_block(G) ! n = cs2\<close> 
+      have local_rel_corr: "(\<And> s2'.((red_cmd_list A M \<Lambda> \<Gamma> \<Omega> (cs2) (Normal ns1) s2') \<Longrightarrow> (s2' \<noteq> Failure)))"
+        using dag_verifies_propagate_2 by blast
+  
+      from local_rel_corr first_step Cons
+      have a2: "(inter_state \<noteq> Failure  \<and> (\<forall>ns1'. inter_state = Normal ns1' \<longrightarrow> (A,M,\<Lambda>,\<Gamma>,\<Omega> \<turnstile> \<langle>cs2, Normal ns1\<rangle> [\<rightarrow>] Normal ns1')))" 
+        using block_local_rel local.Rel_Main_test assms(3) by blast
+  
+      from first_step Cons \<open>cs1 \<noteq> []\<close>
+      have a1: "(inter_bb, inter_cont, inter_state) = ((BigBlock name [] any_str any_tr), cont0, inter_state)"
+      proof cases
+        case RedSimpleCmds then show ?thesis by (auto simp add: RedSimpleCmds)
+      qed auto
+  
+      show ?thesis 
+      proof (cases inter_state)
+        case 2: (Normal x1)
+        from rest_of_steps show ?thesis 
+        proof (cases j')
+          case 0
+          then show ?thesis 
+            by (metis Ast.valid_configuration_def a1 a2 bb_successor_if get_state.simps is_final.simps(3) relpowp_0_E rest_of_steps) 
+        next
+          case 3: (Suc j'')
+          from this rest_of_steps obtain snd_inter_bb snd_inter_cont snd_inter_state where
+            snd_step: "red_bigblock A M \<Lambda> \<Gamma> \<Omega> T ((BigBlock name [] any_str any_tr), cont0, inter_state)  (snd_inter_bb, snd_inter_cont, snd_inter_state)" and
+            snd_rest_of_steps: "A,M,\<Lambda>,\<Gamma>,\<Omega>,T \<turnstile> (snd_inter_bb, snd_inter_cont, snd_inter_state) -n\<longrightarrow>^j'' (reached_bb, reached_cont, reached_state)"
+            by (metis a1 get_state.cases relpowp_Suc_D2)
+  
+          thus ?thesis 
+          proof (cases cont_guard)
+            case None
+            from snd_step this show ?thesis
+            proof cases
+              case RedParsedIfTrue
+              hence eq: "(snd_inter_bb, snd_inter_cont, snd_inter_state) = (then0, convert_list_to_cont (rev then_bbs) cont0, inter_state)" using None bb_successor_if 1 by auto
+  
+              from first_step 
+              have succ_cfg_correct: "(\<forall>msuc2.  List.member (out_edges(G) ! n) msuc2 \<longrightarrow> (\<forall>m3 s3. ((A,M,\<Lambda>,\<Gamma>,\<Omega>,G \<turnstile> (Inl(msuc2), inter_state) -n\<rightarrow>* (m3, s3)) \<longrightarrow> s3 \<noteq> Failure)))"
+              proof cases
+                case RedSimpleCmds show ?thesis using 2 eq RedSimpleCmds(3) dag_verifies_propagate assms(3-4) Rel_Main_test(1) cfg_correct by blast
+              qed (auto simp add: \<open>cs1 \<noteq> Nil\<close>)
+  
+              have "j'' < j" using 1 3 using Suc_lessD by blast
+              
+              thus ?thesis using eq snd_rest_of_steps succ_correct None 2 succ_cfg_correct by blast
+            next
+              case RedParsedIfFalse
+              hence eq: "(snd_inter_bb, snd_inter_cont, snd_inter_state) = (else0, convert_list_to_cont (rev else_bbs) cont0, inter_state)" using None bb_successor_if 1 by auto
+  
+              from first_step 
+              have succ_cfg_correct: "(\<forall>msuc2.  List.member (out_edges(G) ! n) msuc2 \<longrightarrow> (\<forall>m3 s3. ((A,M,\<Lambda>,\<Gamma>,\<Omega>,G \<turnstile> (Inl(msuc2), inter_state) -n\<rightarrow>* (m3, s3)) \<longrightarrow> s3 \<noteq> Failure)))"
+              proof cases
+                case RedSimpleCmds show ?thesis using 2 eq RedSimpleCmds(3) dag_verifies_propagate assms(3-4) Rel_Main_test(1) cfg_correct by blast
+              qed (auto simp add: \<open>cs1 \<noteq> Nil\<close>)
+  
+              have "j'' < j" using 1 3 using Suc_lessD by blast
+  
+              thus ?thesis using eq snd_rest_of_steps succ_correct None 2 succ_cfg_correct by blast
+            qed (auto simp add: bb_successor_if 2)
+          next
+            case (Some block_guard)
+            then show ?thesis 
+            proof cases
+              assume guard_true: "(red_expr A \<Lambda> \<Gamma> \<Omega> block_guard x1 (BoolV True))"
+              hence guard_not_false: "\<not> (red_expr A \<Lambda> \<Gamma> \<Omega> block_guard x1 (BoolV False))" using expr_eval_determ by blast
+              from snd_step have eq: "(snd_inter_bb, snd_inter_cont, snd_inter_state) = (then0, convert_list_to_cont (rev then_bbs) cont0, inter_state)" 
+              proof cases
+                case RedParsedIfTrue thus ?thesis using guard_true bb_successor_if by (simp add: RedParsedIfTrue)
+              qed (auto simp add: guard_not_false bb_successor_if 2 Some)
+  
+              from first_step 
+              have succ_cfg_correct: "(\<forall>msuc2.  List.member (out_edges(G) ! n) msuc2 \<longrightarrow> (\<forall>m3 s3. ((A,M,\<Lambda>,\<Gamma>,\<Omega>,G \<turnstile> (Inl(msuc2), inter_state) -n\<rightarrow>* (m3, s3)) \<longrightarrow> s3 \<noteq> Failure)))"
+              proof cases
+                case RedSimpleCmds show ?thesis using 2 eq RedSimpleCmds(3) dag_verifies_propagate assms(3-4) Rel_Main_test(1) cfg_correct by blast
+              qed (auto simp add: \<open>cs1 \<noteq> Nil\<close>)
+  
+              have "j'' < j" using 1 3 using Suc_lessD by blast
+              
+              thus ?thesis using eq guard_true snd_rest_of_steps succ_correct Some succ_cfg_correct 2 by blast
+            next
+              assume guard_not_true: "\<not> (red_expr A \<Lambda> \<Gamma> \<Omega> block_guard x1 (BoolV True))"
+              thus ?thesis 
+              proof cases
+                assume guard_false: "(red_expr A \<Lambda> \<Gamma> \<Omega> block_guard x1 (BoolV False))"
+                from snd_step have eq: "(snd_inter_bb, snd_inter_cont, snd_inter_state) = (else0, convert_list_to_cont (rev else_bbs) cont0, inter_state)" 
+                proof cases
+                  case RedParsedIfFalse thus ?thesis using guard_false bb_successor_if by (simp add: RedParsedIfFalse)
+                qed (auto simp add: guard_not_true bb_successor_if 2 Some)
+  
+                from first_step 
+                have succ_cfg_correct: "(\<forall>msuc2.  List.member (out_edges(G) ! n) msuc2 \<longrightarrow> (\<forall>m3 s3. ((A,M,\<Lambda>,\<Gamma>,\<Omega>,G \<turnstile> (Inl(msuc2), inter_state) -n\<rightarrow>* (m3, s3)) \<longrightarrow> s3 \<noteq> Failure)))"
+                proof cases
+                  case RedSimpleCmds show ?thesis using 2 eq RedSimpleCmds(3) dag_verifies_propagate assms(3-4) Rel_Main_test(1) cfg_correct by blast
+                qed (auto simp add: \<open>cs1 \<noteq> Nil\<close>)              
+  
+                have "j'' < j" using 1 3 using Suc_lessD by blast
+          
+                thus ?thesis using eq guard_false snd_rest_of_steps succ_correct Some 2 succ_cfg_correct by blast
+              next
+                assume guard_not_false2: "(\<not> (red_expr A \<Lambda> \<Gamma> \<Omega> block_guard x1 (BoolV False)))" and  
+                       guard_not_true2: "(\<not> (red_expr A \<Lambda> \<Gamma> \<Omega> block_guard x1 (BoolV True)))"
+                thus ?thesis
+                proof -
+                  from snd_step have False using guard_not_false2 guard_not_true2 bb_successor_if Some 2 
+                    by (cases) auto
+                  thus ?thesis by simp
+                qed
+              qed  
+            qed 
+          qed
+        qed
+      next
+        case Failure
+        then show ?thesis
+          using \<open>inter_state \<noteq> Failure \<and> (\<forall>ns1'. inter_state = Normal ns1' \<longrightarrow> A,M,\<Lambda>,\<Gamma>,\<Omega> \<turnstile> \<langle>cs2,Normal ns1\<rangle> [\<rightarrow>] Normal ns1')\<close> 
+          by linarith
+      next
+        case Magic
+        then show ?thesis by (metis Ast.valid_configuration_def a2 get_state.simps magic_propagates rest_of_steps state.distinct(3))
+      qed
     qed
   qed
-qed auto
+next
+  case Rel_Invs
+  hence "cs2 = []" by simp
+  have not_end: "(cont0 \<noteq> KStop) \<or> any_str \<noteq> None \<or> any_tr \<noteq> None" using bb_successor_if by simp
+  show ?thesis
+  proof (cases cs2)
+    case Nil 
+    thus ?thesis
+    proof (cases j)
+      case 0
+      hence "(reached_bb, reached_cont, reached_state) = ((BigBlock name cs1 any_str any_tr), cont0, (Normal ns1))" using ast_trace assms(3) by auto
+      then show ?thesis by (simp add: Ast.valid_configuration_def bb_successor_if) 
+    next
+      case 1: (Suc j')
+        from this assms(3) obtain snd_inter_bb snd_inter_cont snd_inter_state where
+          snd_step: "red_bigblock A M \<Lambda> \<Gamma> \<Omega> T ((BigBlock name [] any_str any_tr), cont0, (Normal ns1))  (snd_inter_bb, snd_inter_cont, snd_inter_state)" and
+          snd_rest_of_steps: "A,M,\<Lambda>,\<Gamma>,\<Omega>,T \<turnstile> (snd_inter_bb, snd_inter_cont, snd_inter_state) -n\<longrightarrow>^j' (reached_bb, reached_cont, reached_state)" 
+          using Rel_Invs
+          by (metis ast_trace bigblock.inject local.Rel_Invs(1) relpowp_Suc_E2 surj_pair)
+  
+        thus ?thesis 
+        proof (cases cont_guard)
+          case None
+          from snd_step this show ?thesis
+          proof cases
+            case RedParsedIfTrue
+            hence eq: "(snd_inter_bb, snd_inter_cont, snd_inter_state) = (then0, convert_list_to_cont (rev then_bbs) cont0, (Normal ns1))" using None bb_successor_if 1 by auto
+  
+            have succ_cfg_correct: "(\<forall>msuc2.  List.member (out_edges(G) ! n) msuc2 \<longrightarrow> (\<forall>m3 s3. ((A,M,\<Lambda>,\<Gamma>,\<Omega>,G \<turnstile> (Inl(msuc2), (Normal ns1)) -n\<rightarrow>* (m3, s3)) \<longrightarrow> s3 \<noteq> Failure)))"
+              using assms(4) cfg_correct correctness_propagates_through_empty local.Nil by blast
+  
+            have "j' < j" using 1 using Suc_lessD by blast
+            
+            thus ?thesis using eq snd_rest_of_steps succ_correct None succ_cfg_correct by blast
+          next
+            case RedParsedIfFalse
+            hence eq: "(snd_inter_bb, snd_inter_cont, snd_inter_state) = (else0, convert_list_to_cont (rev else_bbs) cont0, (Normal ns1))" using None bb_successor_if 1 by auto
+  
+            from snd_step 
+            have succ_cfg_correct: "(\<forall>msuc2.  List.member (out_edges(G) ! n) msuc2 \<longrightarrow> (\<forall>m3 s3. ((A,M,\<Lambda>,\<Gamma>,\<Omega>,G \<turnstile> (Inl(msuc2), (Normal ns1)) -n\<rightarrow>* (m3, s3)) \<longrightarrow> s3 \<noteq> Failure)))"
+              using assms(4) cfg_correct correctness_propagates_through_empty local.Nil by blast
+  
+            have "j' < j" using 1 using Suc_lessD by blast
+  
+            thus ?thesis using eq snd_rest_of_steps succ_correct None succ_cfg_correct by blast
+          qed (auto simp add: bb_successor_if)
+        next
+          case (Some block_guard)
+          then show ?thesis 
+          proof cases
+            assume guard_true: "(red_expr A \<Lambda> \<Gamma> \<Omega> block_guard ns1 (BoolV True))"
+            hence guard_not_false: "\<not> (red_expr A \<Lambda> \<Gamma> \<Omega> block_guard ns1 (BoolV False))" using expr_eval_determ by blast
+            from snd_step have eq: "(snd_inter_bb, snd_inter_cont, snd_inter_state) = (then0, convert_list_to_cont (rev then_bbs) cont0, Normal ns1)" 
+            proof cases
+              case RedParsedIfTrue thus ?thesis using guard_true bb_successor_if by (simp add: RedParsedIfTrue)
+            qed (auto simp add: guard_not_false bb_successor_if Some)
+  
+            from snd_step 
+            have succ_cfg_correct: "(\<forall>msuc2.  List.member (out_edges(G) ! n) msuc2 \<longrightarrow> (\<forall>m3 s3. ((A,M,\<Lambda>,\<Gamma>,\<Omega>,G \<turnstile> (Inl(msuc2), Normal ns1) -n\<rightarrow>* (m3, s3)) \<longrightarrow> s3 \<noteq> Failure)))"
+              using assms(4) cfg_correct correctness_propagates_through_empty local.Nil by blast
+  
+            have "j' < j" using 1 using Suc_lessD by blast
+            
+            thus ?thesis using eq guard_true snd_rest_of_steps succ_correct Some succ_cfg_correct by blast
+          next
+            assume guard_not_true: "\<not> (red_expr A \<Lambda> \<Gamma> \<Omega> block_guard ns1 (BoolV True))"
+            thus ?thesis 
+            proof cases
+              assume guard_false: "(red_expr A \<Lambda> \<Gamma> \<Omega> block_guard ns1 (BoolV False))"
+              from snd_step have eq: "(snd_inter_bb, snd_inter_cont, snd_inter_state) = (else0, convert_list_to_cont (rev else_bbs) cont0, Normal ns1)" 
+              proof cases
+                case RedParsedIfFalse thus ?thesis using guard_false bb_successor_if by (simp add: RedParsedIfFalse)
+              qed (auto simp add: guard_not_true bb_successor_if Some)
+  
+              from snd_step 
+              have succ_cfg_correct: "(\<forall>msuc2.  List.member (out_edges(G) ! n) msuc2 \<longrightarrow> (\<forall>m3 s3. ((A,M,\<Lambda>,\<Gamma>,\<Omega>,G \<turnstile> (Inl(msuc2), Normal ns1) -n\<rightarrow>* (m3, s3)) \<longrightarrow> s3 \<noteq> Failure)))"
+                using assms(4) cfg_correct correctness_propagates_through_empty local.Nil by blast              
+  
+              have "j' < j" using 1 using Suc_lessD by blast
+        
+              thus ?thesis using eq guard_false snd_rest_of_steps succ_correct Some succ_cfg_correct by blast
+            next
+              assume guard_not_false2: "(\<not> (red_expr A \<Lambda> \<Gamma> \<Omega> block_guard ns1 (BoolV False)))" and  
+                     guard_not_true2: "(\<not> (red_expr A \<Lambda> \<Gamma> \<Omega> block_guard ns1 (BoolV True)))"
+              thus ?thesis
+              proof -
+                from snd_step have False using guard_not_false2 guard_not_true2 bb_successor_if Some 
+                  by (cases) auto
+                thus ?thesis by simp
+              qed
+            qed  
+          qed 
+        qed
+      qed
+  next
+    case (Cons) thus ?thesis using \<open>cs2 = []\<close> by simp
+  qed
+qed
 
 text \<open>Global lemma for an ast-bigblock with a non-empty set of simple cmds which is the first bigblock in the else-branch of an if-statement.\<close>
 lemma block_global_rel_if_false:
-  assumes block_rel: "ast_cfg_rel None [] (BigBlock name cs1 any_str any_tr) cs2"
-  and ast_trace: "A,M,\<Lambda>,\<Gamma>,\<Omega>,T \<turnstile> ((BigBlock name cs1 any_str any_tr), cont0, (Normal ns1)) -n\<longrightarrow>^j (reached_bb, reached_cont, reached_state)"
+  assumes block_rel: "ast_cfg_rel None [] bb cs2"
+  and ast_trace: "A,M,\<Lambda>,\<Gamma>,\<Omega>,T \<turnstile> (bb, cont0, (Normal ns1)) -n\<longrightarrow>^j (reached_bb, reached_cont, reached_state)"
+  and "bb = (BigBlock name cs1 any_str any_tr)"
   and "cs1 \<noteq> Nil"
   and "cs2 \<noteq> Nil"
   and "node_to_block(G) ! n = cs3"
@@ -1041,7 +1727,7 @@ lemma block_global_rel_if_false:
   and "(UnOp Not block_guard) \<sim> some_cmd"
   and trace_is_possible: "A,\<Lambda>,\<Gamma>,\<Omega> \<turnstile> \<langle>(UnOp Not block_guard), ns1\<rangle> \<Down> LitV (LBool True)"
   and block_local_rel: 
-        "\<And> reached_bb_inter reached_cont_inter reached_state_inter. (red_bigblock A M \<Lambda> \<Gamma> \<Omega> T ((BigBlock name cs1 any_str any_tr), cont0, (Normal ns1)) (reached_bb_inter, reached_cont_inter, reached_state_inter)) \<Longrightarrow> 
+        "\<And> reached_bb_inter reached_cont_inter reached_state_inter. (red_bigblock A M \<Lambda> \<Gamma> \<Omega> T (bb, cont0, (Normal ns1)) (reached_bb_inter, reached_cont_inter, reached_state_inter)) \<Longrightarrow> 
         (\<And> s2'.((red_cmd_list A M \<Lambda> \<Gamma> \<Omega> cs3 (Normal ns1) s2') \<Longrightarrow> (s2' \<noteq> Failure))) \<Longrightarrow>   
         (reached_state_inter \<noteq> Failure  \<and> (\<forall>ns1'. reached_state_inter = Normal ns1' \<longrightarrow> (A,M,\<Lambda>,\<Gamma>,\<Omega> \<turnstile> \<langle>cs3, Normal ns1\<rangle> [\<rightarrow>] Normal ns1')))"
   and succ_correct: 
@@ -1058,11 +1744,11 @@ proof cases
   from ast_trace show ?thesis
   proof (cases j)
     case 0
-    hence "(reached_bb, reached_cont, reached_state) = ((BigBlock name cs1 any_str any_tr), cont0, (Normal ns1))" using ast_trace by fastforce
+    hence "(reached_bb, reached_cont, reached_state) = ((BigBlock name cs1 any_str any_tr), cont0, (Normal ns1))" using ast_trace assms(3) by fastforce
     then show ?thesis unfolding Ast.valid_configuration_def by (simp add: trivial_bb_successor)
   next
     case succ_0: (Suc j')
-    from this obtain inter_bb inter_cont inter_state where
+    from this assms(3) obtain inter_bb inter_cont inter_state where
       first_step: "red_bigblock A M \<Lambda> \<Gamma> \<Omega> T ((BigBlock name cs1 any_str any_tr), cont0, (Normal ns1)) (inter_bb, inter_cont, inter_state)" and
       rest_of_steps: "A,M,\<Lambda>,\<Gamma>,\<Omega>,T \<turnstile> (inter_bb, inter_cont, inter_state) -n\<longrightarrow>^j' (reached_bb, reached_cont, reached_state)" 
       by (metis ast_trace prod_cases3 relpowp_Suc_D2)
@@ -1073,7 +1759,7 @@ proof cases
 
     from local_rel_corr first_step 
     have a2: "(inter_state \<noteq> Failure  \<and> (\<forall>ns1'. inter_state = Normal ns1' \<longrightarrow> (A,M,\<Lambda>,\<Gamma>,\<Omega> \<turnstile> \<langle>cs3, Normal ns1\<rangle> [\<rightarrow>] Normal ns1')))" 
-      using block_local_rel by simp
+      using block_local_rel assms(3) by simp
 
     from first_step \<open>cs1 \<noteq> Nil\<close> 
     have a1: "(inter_bb, inter_cont, inter_state) = ((BigBlock name [] any_str any_tr), cont0, inter_state)"
@@ -1105,9 +1791,9 @@ proof cases
         proof cases
           case RedSimpleCmds 
           hence cmds_red: "A,M,\<Lambda>,\<Gamma>,\<Omega> \<turnstile> \<langle>c#cs2, Normal ns1\<rangle> [\<rightarrow>] inter_state" 
-            using Rel_Main_test(1) \<open>c = Assume some_cmd\<close> \<open>(UnOp Not block_guard) \<sim> some_cmd\<close> equiv_preserves_value trace_is_possible RedAssumeOk RedCmdListCons 
-            by metis
-          show ?thesis by (metis (no_types, lifting) "1" RedNormalSucc assms(5) assms(6) cfg_correct cmds_red converse_rtranclp_into_rtranclp)
+            using  "1" a2 assms(7) 
+            by blast
+          show ?thesis by (metis (no_types, lifting) "1" RedNormalSucc assms(6-7) cfg_correct cmds_red converse_rtranclp_into_rtranclp)
         qed (auto simp add: \<open>cs1 \<noteq> Nil\<close>) 
 
         have "j'' < j" using succ_0 2 by simp
@@ -1128,8 +1814,9 @@ qed auto
 
 text \<open>Global lemma for an ast-bigblock with a non-empty set of simple cmds which is the first bigblock in the then-branch of an if-statement.\<close>
 lemma block_global_rel_if_true:
-  assumes block_rel: "ast_cfg_rel None [] (BigBlock name cs1 any_str any_tr) cs2"
-  and ast_trace: "A,M,\<Lambda>,\<Gamma>,\<Omega>,T \<turnstile> ((BigBlock name cs1 any_str any_tr), cont0, (Normal ns1)) -n\<longrightarrow>^j (reached_bb, reached_cont, reached_state)"
+  assumes block_rel: "ast_cfg_rel None [] bb cs2"
+  and ast_trace: "A,M,\<Lambda>,\<Gamma>,\<Omega>,T \<turnstile> (bb, cont0, (Normal ns1)) -n\<longrightarrow>^j (reached_bb, reached_cont, reached_state)"
+  and "bb = (BigBlock name cs1 any_str any_tr)"
   and "cs1 \<noteq> Nil"
   and "cs2 \<noteq> Nil"
   and "node_to_block(G) ! n = cs3"
@@ -1139,7 +1826,7 @@ lemma block_global_rel_if_true:
   and "c = Assume block_guard"
   and trace_is_possible: "A,\<Lambda>,\<Gamma>,\<Omega> \<turnstile> \<langle>block_guard, ns1\<rangle> \<Down> LitV (LBool True)"
   and block_local_rel: 
-        "\<And> reached_bb_inter reached_cont_inter reached_state_inter. (red_bigblock A M \<Lambda> \<Gamma> \<Omega> T ((BigBlock name cs1 any_str any_tr), cont0, (Normal ns1)) (reached_bb_inter, reached_cont_inter, reached_state_inter)) \<Longrightarrow> 
+        "\<And> reached_bb_inter reached_cont_inter reached_state_inter. (red_bigblock A M \<Lambda> \<Gamma> \<Omega> T (bb, cont0, (Normal ns1)) (reached_bb_inter, reached_cont_inter, reached_state_inter)) \<Longrightarrow> 
         (\<And> s2'.((red_cmd_list A M \<Lambda> \<Gamma> \<Omega> cs3 (Normal ns1) s2') \<Longrightarrow> (s2' \<noteq> Failure))) \<Longrightarrow>   
         (reached_state_inter \<noteq> Failure  \<and> (\<forall>ns1'. reached_state_inter = Normal ns1' \<longrightarrow> (A,M,\<Lambda>,\<Gamma>,\<Omega> \<turnstile> \<langle>cs3, Normal ns1\<rangle> [\<rightarrow>] Normal ns1')))"
   and succ_correct: 
@@ -1156,11 +1843,11 @@ proof cases
   from ast_trace show ?thesis
   proof (cases j)
     case 0
-    hence "(reached_bb, reached_cont, reached_state) = ((BigBlock name cs1 any_str any_tr), cont0, (Normal ns1))" using ast_trace by auto
-    then show ?thesis unfolding Ast.valid_configuration_def by (metis assms(3) get_state.simps is_final.simps(2) neq_Nil_conv state.distinct(1))
+    hence "(reached_bb, reached_cont, reached_state) = ((BigBlock name cs1 any_str any_tr), cont0, (Normal ns1))" using ast_trace assms(3) by auto
+    then show ?thesis unfolding Ast.valid_configuration_def by (metis assms(4) get_state.simps is_final.simps(2) neq_Nil_conv state.distinct(1))
   next
     case succ_0: (Suc j')
-    from this obtain inter_bb inter_cont inter_state where
+    from this assms(3) obtain inter_bb inter_cont inter_state where
       first_step: "red_bigblock A M \<Lambda> \<Gamma> \<Omega> T ((BigBlock name cs1 any_str any_tr), cont0, (Normal ns1)) (inter_bb, inter_cont, inter_state)" and
       rest_of_steps: "A,M,\<Lambda>,\<Gamma>,\<Omega>,T \<turnstile> (inter_bb, inter_cont, inter_state) -n\<longrightarrow>^j' (reached_bb, reached_cont, reached_state)" 
       by (metis ast_trace get_state.cases relpowp_Suc_D2)
@@ -1171,7 +1858,7 @@ proof cases
 
     from local_rel_corr first_step 
     have a2: "(inter_state \<noteq> Failure  \<and> (\<forall>ns1'. inter_state = Normal ns1' \<longrightarrow> (A,M,\<Lambda>,\<Gamma>,\<Omega> \<turnstile> \<langle>cs3, Normal ns1\<rangle> [\<rightarrow>] Normal ns1')))" 
-      using block_local_rel by simp
+      using block_local_rel assms(3) by simp
 
     from first_step \<open>cs1 \<noteq> Nil\<close> 
     have a1: "(inter_bb, inter_cont, inter_state) = ((BigBlock name [] any_str any_tr), cont0, inter_state)"
@@ -1204,8 +1891,8 @@ proof cases
         proof cases
           case RedSimpleCmds 
           hence cmds_red: "A,M,\<Lambda>,\<Gamma>,\<Omega> \<turnstile> \<langle>c#cs2, Normal ns1\<rangle> [\<rightarrow>] inter_state" 
-            using Rel_Main_test(1) \<open>c = Assume block_guard\<close> trace_is_possible RedAssumeOk RedCmdListCons by blast
-          show ?thesis using "1" assms(5) assms(6) cfg_correct cmds_red dag_verifies_propagate by blast
+            using Rel_Main_test(1) \<open>c = Assume block_guard\<close> trace_is_possible RedAssumeOk RedCmdListCons assms(3) by blast
+          show ?thesis using "1" assms(6-7) cfg_correct cmds_red dag_verifies_propagate by blast
         qed (auto simp add: \<open>cs1 \<noteq> Nil\<close>) 
 
         have "j'' < j" using succ_0 2 by simp
@@ -1226,15 +1913,16 @@ qed auto
 
 text \<open>Global lemma for a generic ast-bigblock with a non-empty set of simple cmds.\<close>
 lemma block_global_rel_generic:
-  assumes block_rel: "ast_cfg_rel None [] (BigBlock name cs1 any_str any_tr) cs2"
-  and ast_trace: "A,M,\<Lambda>,\<Gamma>,\<Omega>,T \<turnstile> ((BigBlock name cs1 any_str any_tr), cont0, (Normal ns1)) -n\<longrightarrow>^j (reached_bb, reached_cont, reached_state)"
+  assumes block_rel: "ast_cfg_rel None [] bb cs2"
+  and ast_trace: "A,M,\<Lambda>,\<Gamma>,\<Omega>,T \<turnstile> (bb, cont0, (Normal ns1)) -n\<longrightarrow>^j (reached_bb, reached_cont, reached_state)"
+  and "bb = (BigBlock name cs1 any_str any_tr)"
   and "cs1 \<noteq> Nil"
   and "cs2 \<noteq> Nil"
   and "node_to_block(G) ! n = cs2"
   and cfg_correct: "(\<And> m2 s2. ((red_cfg_multi A M \<Lambda> \<Gamma> \<Omega> G (Inl n, Normal ns1) (m2, s2)) \<Longrightarrow> (s2 \<noteq> Failure)))"
   and trivial_bb_successor: "(cont0 = KSeq bb1 cont1) \<and> any_str = None \<and> any_tr = None"
   and block_local_rel: 
-        "\<And> reached_bb_inter reached_cont_inter reached_state_inter. (red_bigblock A M \<Lambda> \<Gamma> \<Omega> T ((BigBlock name cs1 any_str any_tr), cont0, (Normal ns1)) (reached_bb_inter, reached_cont_inter, reached_state_inter)) \<Longrightarrow> 
+        "\<And> reached_bb_inter reached_cont_inter reached_state_inter. (red_bigblock A M \<Lambda> \<Gamma> \<Omega> T (bb, cont0, (Normal ns1)) (reached_bb_inter, reached_cont_inter, reached_state_inter)) \<Longrightarrow> 
         (\<And> s2'.((red_cmd_list A M \<Lambda> \<Gamma> \<Omega> cs2 (Normal ns1) s2') \<Longrightarrow> (s2' \<noteq> Failure))) \<Longrightarrow>   
         (reached_state_inter \<noteq> Failure  \<and> (\<forall>ns1'. reached_state_inter = Normal ns1' \<longrightarrow> (A,M,\<Lambda>,\<Gamma>,\<Omega> \<turnstile> \<langle>cs2, Normal ns1\<rangle> [\<rightarrow>] Normal ns1')))"
   and succ_correct: 
@@ -1251,11 +1939,11 @@ proof cases
   from ast_trace show ?thesis
   proof (cases j)
     case 0
-    hence "(reached_bb, reached_cont, reached_state) = ((BigBlock name cs1 any_str any_tr), cont0, (Normal ns1))" using ast_trace by auto
+    hence "(reached_bb, reached_cont, reached_state) = ((BigBlock name cs1 any_str any_tr), cont0, (Normal ns1))" using ast_trace assms(3) by auto
     then show ?thesis unfolding Ast.valid_configuration_def by (simp add: trivial_bb_successor)
   next
     case succ_0: (Suc j')
-    from this obtain inter_bb inter_cont inter_state where
+    from this assms(3) obtain inter_bb inter_cont inter_state where
       first_step: "red_bigblock A M \<Lambda> \<Gamma> \<Omega> T ((BigBlock name cs1 any_str any_tr), cont0, (Normal ns1)) (inter_bb, inter_cont, inter_state)" and
       rest_of_steps: "A,M,\<Lambda>,\<Gamma>,\<Omega>,T \<turnstile> (inter_bb, inter_cont, inter_state) -n\<longrightarrow>^j' (reached_bb, reached_cont, reached_state)"
       by (metis ast_trace get_state.cases relpowp_Suc_D2)
@@ -1266,7 +1954,7 @@ proof cases
 
     from local_rel_corr first_step 
     have a2: "(inter_state \<noteq> Failure  \<and> (\<forall>ns1'. inter_state = Normal ns1' \<longrightarrow> (A,M,\<Lambda>,\<Gamma>,\<Omega> \<turnstile> \<langle>cs2, Normal ns1\<rangle> [\<rightarrow>] Normal ns1')))" 
-      using block_local_rel by simp
+      using block_local_rel assms(3) by simp
 
     from first_step \<open>cs1 \<noteq> Nil\<close> 
     have a1: "(inter_bb, inter_cont, inter_state) = ((BigBlock name [] any_str any_tr), cont0, inter_state)"
@@ -1297,7 +1985,7 @@ proof cases
         from first_step 
         have succ_cfg_correct: "(\<forall>msuc2.  List.member (out_edges(G) ! n) msuc2 \<longrightarrow> (\<forall>m3 s3. ((A,M,\<Lambda>,\<Gamma>,\<Omega>,G \<turnstile> (Inl(msuc2), inter_state) -n\<rightarrow>* (m3, s3)) \<longrightarrow> s3 \<noteq> Failure)))"
         proof cases
-          case RedSimpleCmds show ?thesis using 1 snd_step_equiv  RedSimpleCmds(3) dag_verifies_propagate Rel_Main_test(1) cfg_correct assms(5) by blast
+          case RedSimpleCmds show ?thesis using 1 snd_step_equiv  RedSimpleCmds(3) dag_verifies_propagate Rel_Main_test(1) cfg_correct assms(6) assms(3) by blast
         qed (auto simp add: \<open>cs1 \<noteq> Nil\<close>) 
 
         have "j'' < j" using succ_0 2 by simp
