BoogieLang/generated_example_proofs/empty_branch_if_proofs/empty_branch_if_proofs/empty_branch_if_before_ast_cfg.thy
@@ -1,0 +1,89 @@
+theory empty_branch_if_before_ast_cfg
+  imports Main
+          "Boogie_Lang.Ast"
+          "Boogie_Lang.Semantics"
+          "../global_data"
+
+begin
+
+definition bigblock0
+  where "bigblock0 \<equiv> 
+          (BigBlock None [(Havoc 0)] 
+            (Some (ParsedIf (Some (BinOp (Var 0) Gt (Lit (LInt 5)))) 
+                  [BigBlock None [] None None] [BigBlock None [(Assign 0 (Lit (LInt 6)))] None None])) 
+             None)"
+
+definition bigblock1
+  where "bigblock1 \<equiv> 
+          (BigBlock None [(Assert (BinOp (Var 0) Gt (Lit (LInt 5))))] None None)"
+
+definition proc_body
+  where
+    "proc_body = bigblock0 #  bigblock1  # []"
+
+definition pres
+  where
+    "pres  = []"
+definition post
+  where
+    "post  = []"
+definition params_vdecls :: "(vdecls)"
+  where
+    "params_vdecls  = []"
+definition locals_vdecls :: "(vdecls)"
+  where
+    "locals_vdecls  = [(0,(TPrim TInt),(None ))]"
+lemma locals_min_aux:
+shows "(((map fst (append empty_branch_if_before_ast_cfg.params_vdecls empty_branch_if_before_ast_cfg.locals_vdecls)) \<noteq> []) \<longrightarrow> ((Min (set (map fst (append empty_branch_if_before_ast_cfg.params_vdecls empty_branch_if_before_ast_cfg.locals_vdecls)))) \<ge> 0))"
+unfolding empty_branch_if_before_ast_cfg.params_vdecls_def empty_branch_if_before_ast_cfg.locals_vdecls_def
+by simp
+
+lemma locals_min:
+shows "(\<forall> x. ((Set.member x (set (map fst (append empty_branch_if_before_ast_cfg.params_vdecls empty_branch_if_before_ast_cfg.locals_vdecls)))) \<longrightarrow> (x \<ge> 0)))"
+using locals_min_aux helper_min
+by blast
+
+lemma globals_locals_disj:
+shows "((Set.inter (set (map fst (append global_data.constants_vdecls global_data.globals_vdecls))) (set (map fst (append empty_branch_if_before_ast_cfg.params_vdecls empty_branch_if_before_ast_cfg.locals_vdecls)))) = {})"
+unfolding global_data.constants_vdecls_def global_data.globals_vdecls_def
+by simp
+
+lemma consts_wf:
+shows "((list_all (comp (wf_ty 0) (comp fst snd)) global_data.constants_vdecls) )"
+unfolding global_data.constants_vdecls_def
+by simp
+
+lemma globals_wf:
+shows "((list_all (comp (wf_ty 0) (comp fst snd)) global_data.globals_vdecls) )"
+unfolding global_data.globals_vdecls_def
+by simp
+
+lemma params_wf:
+shows "((list_all (comp (wf_ty 0) (comp fst snd)) empty_branch_if_before_ast_cfg.params_vdecls) )"
+unfolding empty_branch_if_before_ast_cfg.params_vdecls_def
+by simp
+
+lemma locals_wf:
+shows "((list_all (comp (wf_ty 0) (comp fst snd)) empty_branch_if_before_ast_cfg.locals_vdecls) )"
+unfolding empty_branch_if_before_ast_cfg.locals_vdecls_def
+by simp
+
+lemma var_context_wf:
+shows "(\<forall> x \<tau>. (((lookup_var_ty ((append global_data.constants_vdecls global_data.globals_vdecls),(append empty_branch_if_before_ast_cfg.params_vdecls empty_branch_if_before_ast_cfg.locals_vdecls)) x) = (Some \<tau>)) \<longrightarrow> ((wf_ty 0) \<tau>)))"
+apply (rule lookup_ty_pred_2)
+by ((simp_all add:consts_wf globals_wf params_wf locals_wf))
+
+lemma m_x:
+shows "((map_of (append empty_branch_if_before_ast_cfg.params_vdecls empty_branch_if_before_ast_cfg.locals_vdecls) 0) = (Some ((TPrim TInt),(None ))))"
+by (simp add:params_vdecls_def locals_vdecls_def)
+
+lemma l_x:
+shows "((lookup_var_decl ((append global_data.constants_vdecls global_data.globals_vdecls),(append empty_branch_if_before_ast_cfg.params_vdecls empty_branch_if_before_ast_cfg.locals_vdecls)) 0) = (Some ((TPrim TInt),(None ))))" and "((lookup_var_ty ((append global_data.constants_vdecls global_data.globals_vdecls),(append empty_branch_if_before_ast_cfg.params_vdecls empty_branch_if_before_ast_cfg.locals_vdecls)) 0) = (Some (TPrim TInt)))"
+using globals_locals_disj m_x
+by (simp_all add: lookup_var_decl_global_2 lookup_var_decl_local lookup_var_decl_ty_Some)
+
+definition proc_ast :: "(ast_procedure)"
+  where
+    "proc_ast  = (|proc_ty_args = 0,proc_args = empty_branch_if_before_ast_cfg.params_vdecls,proc_rets = [],proc_modifs = [],proc_pres = (exprs_to_only_checked_spec empty_branch_if_before_ast_cfg.pres),proc_posts = (exprs_to_only_checked_spec empty_branch_if_before_ast_cfg.post),proc_body = (Some (empty_branch_if_before_ast_cfg.locals_vdecls,empty_branch_if_before_ast_cfg.proc_body))|)"
+
+end
