BoogieLang/generated_example_proofs/goto_example_proofs/q_proofs/q_passive_prog.thy
@@ -1,0 +1,77 @@
+theory q_passive_prog
+imports Boogie_Lang.Semantics Boogie_Lang.Util q_before_passive_prog
+begin
+definition block_0
+  where
+    "block_0  = [(Assert (BinOp (Lit (LInt 0)) Eq (Lit (LInt 0))))]"
+definition block_1
+  where
+    "block_1  = []"
+definition block_2
+  where
+    "block_2  = []"
+definition outEdges
+  where
+    "outEdges  = [[],[0],[1]]"
+definition node_to_blocks
+  where
+    "node_to_blocks  = [block_0,block_1,block_2]"
+definition proc_body
+  where
+    "proc_body  = (|entry = 2,out_edges = outEdges,node_to_block = node_to_blocks|)"
+lemma node_0:
+shows "((nth (node_to_block proc_body) 0) = block_0)"
+by (simp add:proc_body_def node_to_blocks_def)
+
+lemma node_1:
+shows "((nth (node_to_block proc_body) 1) = block_1)"
+by (simp add:proc_body_def node_to_blocks_def)
+
+lemma node_2:
+shows "((nth (node_to_block proc_body) 2) = block_2)"
+by (simp add:proc_body_def node_to_blocks_def)
+
+lemma outEdges_0:
+shows "((nth (out_edges proc_body) 0) = [])"
+by (simp add:proc_body_def outEdges_def)
+
+lemma outEdges_1:
+shows "((nth (out_edges proc_body) 1) = [0])"
+by (simp add:proc_body_def outEdges_def)
+
+lemma outEdges_2:
+shows "((nth (out_edges proc_body) 2) = [1])"
+by (simp add:proc_body_def outEdges_def)
+
+definition params_vdecls :: "(vdecls)"
+  where
+    "params_vdecls  = []"
+definition locals_vdecls :: "(vdecls)"
+  where
+    "locals_vdecls  = [(0,(TPrim TInt),(None ))]"
+lemma locals_min_aux:
+shows "(((map fst (append q_passive_prog.params_vdecls q_passive_prog.locals_vdecls)) \<noteq> []) \<longrightarrow> ((Min (set (map fst (append q_passive_prog.params_vdecls q_passive_prog.locals_vdecls)))) \<ge> 0))"
+unfolding q_passive_prog.params_vdecls_def q_passive_prog.locals_vdecls_def
+by simp
+
+lemma locals_min:
+shows "(\<forall> x. ((Set.member x (set (map fst (append q_passive_prog.params_vdecls q_passive_prog.locals_vdecls)))) \<longrightarrow> (x \<ge> 0)))"
+using locals_min_aux helper_min
+by blast
+
+lemma globals_locals_disj:
+shows "((Set.inter (set (map fst (append global_data.constants_vdecls global_data.globals_vdecls))) (set (map fst (append q_passive_prog.params_vdecls q_passive_prog.locals_vdecls)))) = {})"
+unfolding global_data.constants_vdecls_def global_data.globals_vdecls_def
+by simp
+
+lemma m_x:
+shows "((map_of (append q_passive_prog.params_vdecls q_passive_prog.locals_vdecls) 0) = (Some ((TPrim TInt),(None ))))"
+by (simp add:params_vdecls_def locals_vdecls_def)
+
+lemma l_x:
+shows "((lookup_var_decl ((append global_data.constants_vdecls global_data.globals_vdecls),(append q_passive_prog.params_vdecls q_passive_prog.locals_vdecls)) 0) = (Some ((TPrim TInt),(None ))))" and "((lookup_var_ty ((append global_data.constants_vdecls global_data.globals_vdecls),(append q_passive_prog.params_vdecls q_passive_prog.locals_vdecls)) 0) = (Some (TPrim TInt)))"
+using globals_locals_disj m_x
+by (simp_all add: lookup_var_decl_global_2 lookup_var_decl_local lookup_var_decl_ty_Some)
+
+
+end
