BoogieLang/generated_example_proofs/goto_example_proofs/q_proofs/q_vcphase_proof.thy
@@ -1,0 +1,148 @@
+theory q_vcphase_proof
+imports Boogie_Lang.Semantics Boogie_Lang.Util Boogie_Lang.VCHints Boogie_Lang.VCPhaseML q_passive_prog q_before_passive_prog
+begin
+locale vc
+begin
+
+definition vc_anon0
+  where
+    "vc_anon0  = ((0::int) = (0::int))"
+definition vc_PreconditionGeneratedEntry
+  where
+    "vc_PreconditionGeneratedEntry  = (vc_anon0 )"
+
+end
+
+locale passification = 
+fixes A :: "(('a)absval_ty_fun)" and \<Lambda> :: "(var_context)" and \<Gamma> :: "(('a)fun_interp)" and n_s :: "(('a)nstate)" and vc_x :: "int"
+assumes 
+G0: "((lookup_var \<Lambda> n_s 0) = (Some (IntV vc_x)))" and 
+G1: "(\<And> v. (closed ((type_of_val A) v)))"
+begin
+
+lemmas global_assms = G0 G1
+lemmas forall_poly_thm = forall_vc_type[OF G1]
+lemmas exists_poly_thm = exists_vc_type[OF G1]
+declare Nat.One_nat_def[simp del]
+
+ML\<open>
+val block_anon0_hints = [
+(AssertNoConj,NONE)]
+\<close>
+lemma block_anon0AA0:
+shows "((red_cmd_list A M \<Lambda> \<Gamma> \<Omega> q_passive_prog.block_0 (Normal n_s) s') \<Longrightarrow> ((vc.vc_anon0 ) \<Longrightarrow> ((s' \<noteq> Failure) \<and> (\<forall> n_s'. ((s' = (Normal n_s')) \<longrightarrow> (n_s' = n_s))))))"
+unfolding q_passive_prog.block_0_def vc.vc_anon0_def
+apply (tactic \<open> boogie_vc_tac @{context} @{thms global_assms} (@{thm forall_poly_thm}, @{thm exists_poly_thm}) block_anon0_hints \<close>)
+by (auto?)
+
+lemma block_0:
+assumes 
+"(red_cmd_list A M \<Lambda> \<Gamma> \<Omega> q_passive_prog.block_1 (Normal n_s) s')" and 
+"(vc.vc_anon0 )"
+shows "((s' \<noteq> Failure) \<and> (\<forall> n_s'. ((s' = (Normal n_s')) \<longrightarrow> ((n_s' = n_s) \<and> (vc.vc_anon0 )))))"
+using assms
+unfolding q_passive_prog.block_1_def
+apply cases
+by auto
+
+lemma block_PreconditionGeneratedEntry:
+shows "((red_cmd_list A M \<Lambda> \<Gamma> \<Omega> q_passive_prog.block_2 (Normal n_s) s') \<Longrightarrow> ((vc.vc_PreconditionGeneratedEntry ) \<Longrightarrow> ((s' \<noteq> Failure) \<and> (\<forall> n_s'. ((s' = (Normal n_s')) \<longrightarrow> ((n_s' = n_s) \<and> (vc.vc_anon0 )))))))"
+apply (erule red_cmd_list.cases)
+using global_assms
+unfolding q_passive_prog.block_2_def vc.vc_PreconditionGeneratedEntry_def
+apply (handle_cmd_list_full?)
+by (auto?)
+
+lemma cfg_block_anon0:
+assumes 
+"(red_cfg_multi A M \<Lambda> \<Gamma> \<Omega> q_passive_prog.proc_body ((Inl 0),(Normal n_s)) (m',s'))" and 
+"(vc.vc_anon0 )"
+shows "(s' \<noteq> Failure)"
+apply (rule converse_rtranclpE2[OF assms(1)], fastforce)
+apply (rule red_cfg_multi_backwards_step_no_succ[OF assms(1) q_passive_prog.node_0 q_passive_prog.outEdges_0])
+using block_anon0AA0[OF _ assms(2)] by blast
+
+lemma cfg_block_0:
+assumes 
+"(red_cfg_multi A M \<Lambda> \<Gamma> \<Omega> q_passive_prog.proc_body ((Inl 1),(Normal n_s)) (m',s'))" and 
+"(vc.vc_anon0 )"
+shows "(s' \<noteq> Failure)"
+apply (rule converse_rtranclpE2[OF assms(1)], fastforce)
+apply (rule red_cfg_multi_backwards_step[OF assms(1) q_passive_prog.node_1])
+apply (erule block_0[OF _ assms(2)])
+apply ((simp add:q_passive_prog.outEdges_1))
+apply (erule member_elim, simp)
+apply (erule cfg_block_anon0, simp?)
+by (simp add: member_rec(2))
+
+lemma cfg_PreconditionGeneratedEntry:
+assumes 
+"(red_cfg_multi A M \<Lambda> \<Gamma> \<Omega> q_passive_prog.proc_body ((Inl 2),(Normal n_s)) (m',s'))" and 
+"(vc.vc_PreconditionGeneratedEntry )"
+shows "(s' \<noteq> Failure)"
+apply (rule converse_rtranclpE2[OF assms(1)], fastforce)
+apply (rule red_cfg_multi_backwards_step[OF assms(1) q_passive_prog.node_2])
+apply (erule block_PreconditionGeneratedEntry[OF _ assms(2)])
+apply ((simp add:q_passive_prog.outEdges_2))
+apply (erule member_elim, simp)
+apply (erule cfg_block_0, simp?)
+by (simp add: member_rec(2))
+
+
+end
+
+locale axioms = 
+fixes A :: "(('a)absval_ty_fun)" and \<Lambda> :: "(var_context)" and \<Gamma> :: "(('a)fun_interp)" and n_s :: "(('a)nstate)"
+assumes 
+G0: "(\<And> v. (closed ((type_of_val A) v)))"
+begin
+
+lemmas global_assms = G0
+lemmas forall_poly_thm = forall_vc_type[OF G0]
+lemmas exists_poly_thm = exists_vc_type[OF G0]
+declare Nat.One_nat_def[simp del]
+
+
+end
+
+definition ctor_list
+  where
+    "ctor_list  = []"
+fun ctor :: "((closed_ty) => int)"
+  where
+    "ctor (TConC s _) = (the (map_of ctor_list s))"
+declare One_nat_def[simp del]
+
+lemma end_to_end:
+assumes 
+Red: "(red_cfg_multi A M ((append global_data.constants_vdecls global_data.globals_vdecls),(append q_passive_prog.params_vdecls q_passive_prog.locals_vdecls)) \<Gamma> [] q_passive_prog.proc_body ((Inl 2),(Normal n_s)) (m',s'))" and 
+VC: "(\<And> (vc_x::int). (vc.vc_PreconditionGeneratedEntry ))" and 
+Closed: "(\<And> v. (closed ((type_of_val A) v)))" and 
+NonEmptyTypes: "(\<And> t. ((closed t) \<Longrightarrow> (\<exists> v. (((type_of_val A) v) = t))))" and 
+FInterp: "(fun_interp_wf A global_data.fdecls \<Gamma>)" and 
+Axioms: "(axiom_assm A \<Gamma> global_data.constants_vdecls (n_s::(('a)nstate)) global_data.axioms)" and 
+ParamsLocal: "(state_typ_wf A [] (local_state n_s) (append q_passive_prog.params_vdecls q_passive_prog.locals_vdecls))" and 
+ConstsGlobal: "(state_typ_wf A [] (global_state n_s) (append global_data.constants_vdecls global_data.globals_vdecls))"
+shows "(s' \<noteq> Failure)"
+proof -
+let ?n_s_c = "(nstate_global_restriction n_s global_data.constants_vdecls)"
+let ?\<Lambda> = "((append global_data.constants_vdecls global_data.globals_vdecls),(append q_passive_prog.params_vdecls q_passive_prog.locals_vdecls))"
+let ?\<Lambda>c = "((global_data.constants_vdecls,[])::(var_context))"
+from ParamsLocal have sc_x:"(((lookup_var ?\<Lambda> n_s 0) = (Some (IntV (convert_val_to_int (the (lookup_var ?\<Lambda> n_s 0)))))) \<and> (((type_of_val A) (the (lookup_var ?\<Lambda> n_s 0))) = (TPrim TInt)))"
+apply (simp only:state_typ_wf_def)
+apply (erule allE, erule allE, erule impE, rule map_of_lookup_vdecls_ty[OF q_passive_prog.m_x])
+apply (subst lookup_var_local[OF q_passive_prog.m_x])+
+by (fastforce dest: tint_intv tbool_boolv)
+show "(s' \<noteq> Failure)"
+apply (rule passification.cfg_PreconditionGeneratedEntry[OF _ Red])
+apply (simp only:passification_def)
+apply (intro conjI)?
+apply (rule HOL.conjunct1[OF sc_x])
+apply (simp add:Closed)
+apply (rule VC)
+done
+qed
+
+
+
+end
