BoogieLang/generated_example_proofs/if_example_proofs/p_proofs/p_passive_prog.thy
@@ -1,0 +1,128 @@
+theory p_passive_prog
+imports Boogie_Lang.Semantics Boogie_Lang.Util p_before_passive_prog
+begin
+definition block_0
+  where
+    "block_0  = [(Assert (BinOp (Var 2) Gt (Lit (LInt 0))))]"
+definition block_1
+  where
+    "block_1  = [(Assume (BinOp (Var 1) Gt (Lit (LInt 5)))),(Assume (BinOp (Var 2) Eq (Lit (LInt 10))))]"
+definition block_2
+  where
+    "block_2  = [(Assume (BinOp (Lit (LInt 5)) Ge (Var 1))),(Assume (BinOp (Var 2) Eq (Lit (LInt 1))))]"
+definition block_3
+  where
+    "block_3  = []"
+definition block_4
+  where
+    "block_4  = []"
+definition block_5
+  where
+    "block_5  = []"
+definition outEdges
+  where
+    "outEdges  = [[],[0],[0],[1,2],[3],[4]]"
+definition node_to_blocks
+  where
+    "node_to_blocks  = [block_0,block_1,block_2,block_3,block_4,block_5]"
+definition proc_body
+  where
+    "proc_body  = (|entry = 5,out_edges = outEdges,node_to_block = node_to_blocks|)"
+lemma node_0:
+shows "((nth (node_to_block proc_body) 0) = block_0)"
+by (simp add:proc_body_def node_to_blocks_def)
+
+lemma node_1:
+shows "((nth (node_to_block proc_body) 1) = block_1)"
+by (simp add:proc_body_def node_to_blocks_def)
+
+lemma node_2:
+shows "((nth (node_to_block proc_body) 2) = block_2)"
+by (simp add:proc_body_def node_to_blocks_def)
+
+lemma node_3:
+shows "((nth (node_to_block proc_body) 3) = block_3)"
+by (simp add:proc_body_def node_to_blocks_def)
+
+lemma node_4:
+shows "((nth (node_to_block proc_body) 4) = block_4)"
+by (simp add:proc_body_def node_to_blocks_def)
+
+lemma node_5:
+shows "((nth (node_to_block proc_body) 5) = block_5)"
+by (simp add:proc_body_def node_to_blocks_def)
+
+lemma outEdges_0:
+shows "((nth (out_edges proc_body) 0) = [])"
+by (simp add:proc_body_def outEdges_def)
+
+lemma outEdges_1:
+shows "((nth (out_edges proc_body) 1) = [0])"
+by (simp add:proc_body_def outEdges_def)
+
+lemma outEdges_2:
+shows "((nth (out_edges proc_body) 2) = [0])"
+by (simp add:proc_body_def outEdges_def)
+
+lemma outEdges_3:
+shows "((nth (out_edges proc_body) 3) = [1,2])"
+by (simp add:proc_body_def outEdges_def)
+
+lemma outEdges_4:
+shows "((nth (out_edges proc_body) 4) = [3])"
+by (simp add:proc_body_def outEdges_def)
+
+lemma outEdges_5:
+shows "((nth (out_edges proc_body) 5) = [4])"
+by (simp add:proc_body_def outEdges_def)
+
+definition params_vdecls :: "(vdecls)"
+  where
+    "params_vdecls  = []"
+definition locals_vdecls :: "(vdecls)"
+  where
+    "locals_vdecls  = [(0,(TPrim TInt),(None )),(1,(TPrim TInt),(None )),(2,(TPrim TInt),(None ))]"
+lemma locals_min_aux:
+shows "(((map fst (append p_passive_prog.params_vdecls p_passive_prog.locals_vdecls)) \<noteq> []) \<longrightarrow> ((Min (set (map fst (append p_passive_prog.params_vdecls p_passive_prog.locals_vdecls)))) \<ge> 0))"
+unfolding p_passive_prog.params_vdecls_def p_passive_prog.locals_vdecls_def
+by simp
+
+lemma locals_min:
+shows "(\<forall> x. ((Set.member x (set (map fst (append p_passive_prog.params_vdecls p_passive_prog.locals_vdecls)))) \<longrightarrow> (x \<ge> 0)))"
+using locals_min_aux helper_min
+by blast
+
+lemma globals_locals_disj:
+shows "((Set.inter (set (map fst (append global_data.constants_vdecls global_data.globals_vdecls))) (set (map fst (append p_passive_prog.params_vdecls p_passive_prog.locals_vdecls)))) = {})"
+unfolding global_data.constants_vdecls_def global_data.globals_vdecls_def
+by simp
+
+lemma m_x:
+shows "((map_of (append p_passive_prog.params_vdecls p_passive_prog.locals_vdecls) 0) = (Some ((TPrim TInt),(None ))))"
+by (simp add:params_vdecls_def locals_vdecls_def)
+
+lemma m_x_0:
+shows "((map_of (append p_passive_prog.params_vdecls p_passive_prog.locals_vdecls) 1) = (Some ((TPrim TInt),(None ))))"
+by (simp add:params_vdecls_def locals_vdecls_def)
+
+lemma m_x_1:
+shows "((map_of (append p_passive_prog.params_vdecls p_passive_prog.locals_vdecls) 2) = (Some ((TPrim TInt),(None ))))"
+by (simp add:params_vdecls_def locals_vdecls_def)
+
+lemma l_x:
+shows "((lookup_var_decl ((append global_data.constants_vdecls global_data.globals_vdecls),(append p_passive_prog.params_vdecls p_passive_prog.locals_vdecls)) 0) = (Some ((TPrim TInt),(None ))))" and "((lookup_var_ty ((append global_data.constants_vdecls global_data.globals_vdecls),(append p_passive_prog.params_vdecls p_passive_prog.locals_vdecls)) 0) = (Some (TPrim TInt)))"
+using globals_locals_disj m_x
+by (simp_all add: lookup_var_decl_global_2 lookup_var_decl_local lookup_var_decl_ty_Some)
+
+lemma l_x_0:
+shows "((lookup_var_decl ((append global_data.constants_vdecls global_data.globals_vdecls),(append p_passive_prog.params_vdecls p_passive_prog.locals_vdecls)) 1) = (Some ((TPrim TInt),(None ))))" and "((lookup_var_ty ((append global_data.constants_vdecls global_data.globals_vdecls),(append p_passive_prog.params_vdecls p_passive_prog.locals_vdecls)) 1) = (Some (TPrim TInt)))"
+using globals_locals_disj m_x_0
+by (simp_all add: lookup_var_decl_global_2 lookup_var_decl_local lookup_var_decl_ty_Some)
+
+lemma l_x_1:
+shows "((lookup_var_decl ((append global_data.constants_vdecls global_data.globals_vdecls),(append p_passive_prog.params_vdecls p_passive_prog.locals_vdecls)) 2) = (Some ((TPrim TInt),(None ))))" and "((lookup_var_ty ((append global_data.constants_vdecls global_data.globals_vdecls),(append p_passive_prog.params_vdecls p_passive_prog.locals_vdecls)) 2) = (Some (TPrim TInt)))"
+using globals_locals_disj m_x_1
+by (simp_all add: lookup_var_decl_global_2 lookup_var_decl_local lookup_var_decl_ty_Some)
+
+
+end
