BoogieLang/generated_example_proofs/no_guard_if_proofs/no_guard_if_proofs/no_guard_if_ast_cfg_proof.thy
@@ -1,0 +1,158 @@
+theory no_guard_if_ast_cfg_proof
+  imports Main
+          Boogie_Lang.Ast
+          Boogie_Lang.Semantics
+          Boogie_Lang.Ast_Cfg_Transformation
+          "../global_data" 
+          no_guard_if_before_cfg_to_dag_prog 
+          no_guard_if_before_ast_cfg
+          no_guard_if_cfgtodag_proof
+          "/home/alex/Isabelle_10-Nov-2021/lib/Apply_Trace_Cmd"
+
+begin
+
+definition bigblock_then 
+  where "bigblock_then \<equiv> BigBlock None [(Assign 0 (Lit (LInt 0)))] None None"
+
+definition bigblock_else
+  where "bigblock_else \<equiv> BigBlock None [(Assign 0 (Lit (LInt 1)))] None None"
+
+lemma bigblock0_local_rel:
+  assumes Red_bb0_to: 
+      "red_bigblock A M \<Lambda> \<Gamma> \<Omega> T (bigblock0, KStop, (Normal ns1)) (reached_bb, reached_cont, reached_state)" 
+  and Red0_impl: "(\<And> s2'.(red_cmd_list A M \<Lambda> \<Gamma> \<Omega> no_guard_if_before_cfg_to_dag_prog.block_0 (Normal ns1) s2') \<Longrightarrow> s2' \<noteq> Failure)" 
+  shows "reached_state \<noteq> Failure \<and> 
+         (\<forall>ns1'. reached_state = Normal ns1' \<longrightarrow> (A,M,\<Lambda>,\<Gamma>,\<Omega> \<turnstile> \<langle>no_guard_if_before_cfg_to_dag_prog.block_0, Normal ns1\<rangle> [\<rightarrow>] Normal ns1'))"
+proof -
+  show ?thesis
+    apply (rule block_local_rel_generic)
+           apply (rule Rel_Main_test[of bigblock0])
+           apply (simp add: bigblock0_def no_guard_if_before_cfg_to_dag_prog.block_0_def)
+          apply simp
+         apply simp
+        apply (rule Red_bb0_to)
+       apply (rule Red0_impl, simp)
+      apply (simp add: bigblock0_def)
+     apply (simp)
+    apply (simp add: no_guard_if_before_cfg_to_dag_prog.block_0_def)
+    done
+qed
+
+
+lemma bigblock_then_local_rel:
+  assumes Red_bb0_to: "red_bigblock A M \<Lambda> \<Gamma> \<Omega> T (bigblock_then, KSeq bigblock1 KStop, (Normal ns1)) (reached_bb, reached_cont, reached_state)" 
+  and Red0_impl: "(\<And> s2'.(red_cmd_list A M \<Lambda> \<Gamma> \<Omega> no_guard_if_before_cfg_to_dag_prog.block_2 (Normal ns1) s2') \<Longrightarrow> s2' \<noteq> Failure)" 
+  shows "reached_state \<noteq> Failure \<and> 
+         (\<forall>ns1'. reached_state = Normal ns1' \<longrightarrow> (A,M,\<Lambda>,\<Gamma>,\<Omega> \<turnstile> \<langle>no_guard_if_before_cfg_to_dag_prog.block_2, Normal ns1\<rangle> [\<rightarrow>] Normal ns1'))" 
+proof -
+  show ?thesis
+    unfolding no_guard_if_before_cfg_to_dag_prog.block_2_def 
+    apply (rule block_local_rel_generic)
+           apply (rule Rel_Main_test[of bigblock_then])
+           apply (simp add: bigblock_then_def)
+          apply simp
+         apply simp
+        apply (rule Red_bb0_to)
+       apply (rule Red0_impl)
+       apply (simp add: no_guard_if_before_cfg_to_dag_prog.block_2_def)
+      apply (simp add: bigblock_then_def)
+    by simp_all
+qed
+
+lemma bigblock_else_local_rel:
+  assumes Red_bb0_to: "red_bigblock A M \<Lambda> \<Gamma> \<Omega> T (bigblock_else, KSeq bigblock1 KStop, (Normal ns1)) (reached_bb, reached_cont, reached_state)" 
+  and Red0_impl: "(\<And> s2'.(red_cmd_list A M \<Lambda> \<Gamma> \<Omega> no_guard_if_before_cfg_to_dag_prog.block_1 (Normal ns1) s2') \<Longrightarrow> s2' \<noteq> Failure)" 
+  shows "reached_state \<noteq> Failure \<and> 
+         (\<forall>ns1'. reached_state = Normal ns1' \<longrightarrow> (A,M,\<Lambda>,\<Gamma>,\<Omega> \<turnstile> \<langle>no_guard_if_before_cfg_to_dag_prog.block_1, Normal ns1\<rangle> [\<rightarrow>] Normal ns1'))"
+proof -
+  show ?thesis
+    unfolding no_guard_if_before_cfg_to_dag_prog.block_1_def 
+    apply (rule block_local_rel_generic)
+           apply (rule Rel_Main_test[of bigblock_else])
+           apply (simp add: bigblock_else_def)
+          apply simp
+         apply simp
+        apply (rule Red_bb0_to)
+       apply (rule Red0_impl)
+       apply (simp add: no_guard_if_before_cfg_to_dag_prog.block_1_def)
+      apply (simp add: bigblock_else_def)
+    by simp_all
+qed
+
+
+lemma block_then_global_rel:
+  assumes "A,M,\<Lambda>,\<Gamma>,\<Omega>,T \<turnstile> (bigblock_then, KStop, (Normal ns1)) -n\<longrightarrow>^j (reached_bb, reached_cont, reached_state)"
+  and  "\<And> m' s'. (red_cfg_multi A M \<Lambda> \<Gamma> \<Omega> no_guard_if_before_cfg_to_dag_prog.proc_body ((Inl 2),(Normal ns1)) (m',s')) \<Longrightarrow> (s' \<noteq> Failure)"
+  shows "(Ast.valid_configuration A \<Lambda> \<Gamma> \<Omega> [] reached_bb reached_cont reached_state)" 
+proof -
+  show ?thesis 
+    apply (rule generic_ending_block_global_rel)
+         apply (rule Rel_Main_test[of bigblock_then _ no_guard_if_before_cfg_to_dag_prog.block_2])
+         apply (simp add: bigblock_then_def no_guard_if_before_cfg_to_dag_prog.block_2_def)
+        apply (rule assms(1))
+       apply (simp add: bigblock_then_def)
+      apply simp
+     apply (rule no_guard_if_before_cfg_to_dag_prog.node_2)
+    apply (rule assms(2))
+    apply simp
+    done
+qed
+
+
+lemma block_else_global_rel:
+  assumes "A,M,\<Lambda>,\<Gamma>,\<Omega>,T \<turnstile> (bigblock_else, KStop, (Normal ns1)) -n\<longrightarrow>^j (reached_bb, reached_cont, reached_state)"
+  and  "\<And> m' s'. (red_cfg_multi A M \<Lambda> \<Gamma> \<Omega> no_guard_if_before_cfg_to_dag_prog.proc_body ((Inl 1),(Normal ns1)) (m',s')) \<Longrightarrow> (s' \<noteq> Failure)"
+  shows "(Ast.valid_configuration A \<Lambda> \<Gamma> \<Omega> [] reached_bb reached_cont reached_state)" 
+proof -
+  show ?thesis
+    apply (rule generic_ending_block_global_rel)
+           apply (rule Rel_Main_test[of bigblock_else _ no_guard_if_before_cfg_to_dag_prog.block_1])
+         apply (simp add: bigblock_else_def no_guard_if_before_cfg_to_dag_prog.block_1_def)
+        apply (rule assms(1))
+       apply (simp add: bigblock_else_def)
+      apply simp
+     apply (rule no_guard_if_before_cfg_to_dag_prog.node_1)
+    apply (rule assms(2))
+    apply simp
+    done
+qed
+
+
+lemma block0_global_rel:
+  assumes  "\<And> m' s'. (red_cfg_multi A M \<Lambda> \<Gamma> \<Omega> no_guard_if_before_cfg_to_dag_prog.proc_body ((Inl 0),(Normal ns1)) (m',s')) \<Longrightarrow> (s' \<noteq> Failure)"
+  and ast_trace: "A,M,\<Lambda>,\<Gamma>,\<Omega>,T \<turnstile> (bigblock0, KStop, (Normal ns1)) -n\<longrightarrow>^j (reached_bb, reached_cont, reached_state)"
+  shows "(valid_configuration A \<Lambda> \<Gamma> \<Omega> no_guard_if_before_cfg_to_dag_prog.post reached_bb reached_cont reached_state)" 
+proof -
+  show ?thesis 
+    apply (rule block_global_rel_if_successor)
+           apply (rule Rel_Main_test[of bigblock0 _ no_guard_if_before_cfg_to_dag_prog.block_0])
+           apply (simp add: bigblock0_def no_guard_if_before_cfg_to_dag_prog.block_0_def)
+          apply (rule ast_trace)
+         apply (simp add: bigblock0_def)
+        apply (rule no_guard_if_before_cfg_to_dag_prog.node_0)
+       apply (rule assms(1))
+       apply simp
+      apply simp
+     apply (rule bigblock0_local_rel)
+      apply (simp add: bigblock0_def)
+     apply assumption
+    apply simp
+    apply (rule disjE)
+      apply assumption
+
+     apply (erule allE[where x=2])
+     apply (simp add:no_guard_if_before_cfg_to_dag_prog.outEdges_0)
+     apply (simp add:member_rec(1))
+    unfolding no_guard_if_before_cfg_to_dag_prog.post_def
+     apply (rule block_then_global_rel)
+      apply (simp add: bigblock_then_def)
+    apply simp
+   
+    apply (erule allE[where x=1])
+    apply (simp del: Nat.One_nat_def add:no_guard_if_before_cfg_to_dag_prog.outEdges_0)
+    apply (simp del: Nat.One_nat_def add:member_rec(1))
+    apply (rule block_else_global_rel)
+      apply (simp add: bigblock_else_def)
+    apply simp
+    done
+qed
