BoogieLang/generated_example_proofs/while_example_proofs/m_proofs/m_before_passive_prog.thy
@@ -1,0 +1,106 @@
+theory m_before_passive_prog
+imports Boogie_Lang.Semantics Boogie_Lang.Util m_before_cfg_to_dag_prog
+begin
+definition block_0
+  where
+    "block_0  = []"
+definition block_1
+  where
+    "block_1  = [(Assume (BinOp (Var 1) Le (Var 0))),(Assert (BinOp (Var 0) Ge (Var 1)))]"
+definition block_2
+  where
+    "block_2  = [(Assume (BinOp (Var 0) Lt (Var 1))),(Assign 0 (BinOp (Var 0) Add (Lit (LInt 1)))),(Assert (BinOp (Var 0) Le (Var 1))),(Assume (Lit (LBool False)))]"
+definition block_3
+  where
+    "block_3  = [(Havoc 0),(Assume (BinOp (Var 0) Le (Var 1)))]"
+definition block_4
+  where
+    "block_4  = [(Assign 0 (Lit (LInt 0))),(Assume (BinOp (Var 1) Gt (Lit (LInt 0)))),(Assert (BinOp (Var 0) Le (Var 1)))]"
+definition block_5
+  where
+    "block_5  = []"
+definition block_6
+  where
+    "block_6  = []"
+definition outEdges
+  where
+    "outEdges  = [[],[0],[0],[1,2],[3],[4],[5]]"
+definition node_to_blocks
+  where
+    "node_to_blocks  = [block_0,block_1,block_2,block_3,block_4,block_5,block_6]"
+definition proc_body
+  where
+    "proc_body  = (|entry = 6,out_edges = outEdges,node_to_block = node_to_blocks|)"
+lemma node_0:
+shows "((nth (node_to_block proc_body) 0) = block_0)"
+by (simp add:proc_body_def node_to_blocks_def)
+
+lemma node_1:
+shows "((nth (node_to_block proc_body) 1) = block_1)"
+by (simp add:proc_body_def node_to_blocks_def)
+
+lemma node_2:
+shows "((nth (node_to_block proc_body) 2) = block_2)"
+by (simp add:proc_body_def node_to_blocks_def)
+
+lemma node_3:
+shows "((nth (node_to_block proc_body) 3) = block_3)"
+by (simp add:proc_body_def node_to_blocks_def)
+
+lemma node_4:
+shows "((nth (node_to_block proc_body) 4) = block_4)"
+by (simp add:proc_body_def node_to_blocks_def)
+
+lemma node_5:
+shows "((nth (node_to_block proc_body) 5) = block_5)"
+by (simp add:proc_body_def node_to_blocks_def)
+
+lemma node_6:
+shows "((nth (node_to_block proc_body) 6) = block_6)"
+by (simp add:proc_body_def node_to_blocks_def)
+
+lemma outEdges_0:
+shows "((nth (out_edges proc_body) 0) = [])"
+by (simp add:proc_body_def outEdges_def)
+
+lemma outEdges_1:
+shows "((nth (out_edges proc_body) 1) = [0])"
+by (simp add:proc_body_def outEdges_def)
+
+lemma outEdges_2:
+shows "((nth (out_edges proc_body) 2) = [0])"
+by (simp add:proc_body_def outEdges_def)
+
+lemma outEdges_3:
+shows "((nth (out_edges proc_body) 3) = [1,2])"
+by (simp add:proc_body_def outEdges_def)
+
+lemma outEdges_4:
+shows "((nth (out_edges proc_body) 4) = [3])"
+by (simp add:proc_body_def outEdges_def)
+
+lemma outEdges_5:
+shows "((nth (out_edges proc_body) 5) = [4])"
+by (simp add:proc_body_def outEdges_def)
+
+lemma outEdges_6:
+shows "((nth (out_edges proc_body) 6) = [5])"
+by (simp add:proc_body_def outEdges_def)
+
+lemma locals_min_aux:
+shows "(((map fst (append m_before_cfg_to_dag_prog.params_vdecls m_before_cfg_to_dag_prog.locals_vdecls)) \<noteq> []) \<longrightarrow> ((Min (set (map fst (append m_before_cfg_to_dag_prog.params_vdecls m_before_cfg_to_dag_prog.locals_vdecls)))) \<ge> 0))"
+unfolding m_before_cfg_to_dag_prog.params_vdecls_def m_before_cfg_to_dag_prog.locals_vdecls_def
+by simp
+
+lemma locals_min:
+shows "(\<forall> x. ((Set.member x (set (map fst (append m_before_cfg_to_dag_prog.params_vdecls m_before_cfg_to_dag_prog.locals_vdecls)))) \<longrightarrow> (x \<ge> 0)))"
+using locals_min_aux helper_min
+by blast
+
+lemma globals_locals_disj:
+shows "((Set.inter (set (map fst (append global_data.constants_vdecls global_data.globals_vdecls))) (set (map fst (append m_before_cfg_to_dag_prog.params_vdecls m_before_cfg_to_dag_prog.locals_vdecls)))) = {})"
+unfolding global_data.constants_vdecls_def global_data.globals_vdecls_def
+by simp
+
+
+end
