BoogieLang/generated_example_proofs/while_example_proofs/m_proofs/while_example_ast_cfg_proof.thy
@@ -1,0 +1,5 @@
+theory while_example_ast_cfg_proof
+  imports Main Boogie_Lang.Ast Boogie_Lang.Semantics "../global_data" while_example_before_ast_cfg m_before_cfg_to_dag_prog
+
+begin
+end
